@prefix : <http://latuli.no/terminalCapacityOnto#> .
@prefix dc: <http://purl.org/dc/elements/1.1/> .
@prefix owl: <http://www.w3.org/2002/07/owl#> .
@prefix rdf: <http://www.w3.org/1999/02/22-rdf-syntax-ns#> .
@prefix xml: <http://www.w3.org/XML/1998/namespace> .
@prefix xsd: <http://www.w3.org/2001/XMLSchema#> .
@prefix rdfs: <http://www.w3.org/2000/01/rdf-schema#> .
@prefix skos: <http://www.w3.org/2004/02/skos/core#> .
@prefix terms: <http://purl.org/dc/terms/> .
@base <https://w3id.org/latuli/ontology/tcm#> .

<https://w3id.org/latuli/ontology/tcm#> rdf:type owl:Ontology ;
                                         owl:imports <http://www.opengis.net/ont/geosparql> ,
                                                     <http://www.w3.org/2006/time#2016> .

#################################################################
#    Object Properties
#################################################################

###  https://w3id.org/latuli/ontology/tcm#combinedDoor
:combinedDoor rdf:type owl:ObjectProperty ;
              rdfs:domain :Terminal ;
              rdfs:range :Door ;
              rdfs:comment "A door, or a dock, which can be used both for receiving unloaded goods and for sending goods to be loaded onto a transport means." .


###  https://w3id.org/latuli/ontology/tcm#dimensionMeasurementType
:dimensionMeasurementType rdf:type owl:ObjectProperty ;
                          rdfs:domain :Dimension ;
                          rdfs:range :MeasurementType ;
                          rdfs:comment "Relates a Dimension with a MeasurementType (e.g., metre, cubic or kilogram)." .


###  https://w3id.org/latuli/ontology/tcm#distanceToMainRoad
:distanceToMainRoad rdf:type owl:ObjectProperty ;
                    rdfs:domain :Connectivity ;
                    rdfs:range :Dimension ;
                    rdfs:comment "Describes the distance to main roads, e.g. in terms of kilometres." .


###  https://w3id.org/latuli/ontology/tcm#doorServiceMode
:doorServiceMode rdf:type owl:ObjectProperty ;
                 rdfs:domain :Terminal ;
                 rdfs:range :ServiceMode ;
                 rdfs:comment "Relates a terminal to a ServiceMode." .


###  https://w3id.org/latuli/ontology/tcm#handlingAreaSize
:handlingAreaSize rdf:type owl:ObjectProperty ;
                  rdfs:domain :Terminal ;
                  rdfs:range :Dimension ;
                  rdfs:comment "Describes the size (physical characteristics) of the handling area in a terminal" .


###  https://w3id.org/latuli/ontology/tcm#hasDoorType
:hasDoorType rdf:type owl:ObjectProperty ;
             rdfs:domain :Door ;
             rdfs:range :DoorType .


###  https://w3id.org/latuli/ontology/tcm#hasGateCharacteristics
:hasGateCharacteristics rdf:type owl:ObjectProperty ;
                        rdfs:domain :Gate ;
                        rdfs:range :GateCharacteristics .


###  https://w3id.org/latuli/ontology/tcm#hasInternalTransportation
:hasInternalTransportation rdf:type owl:ObjectProperty ;
                           rdfs:domain :Terminal ;
                           rdfs:range :InternalTransportation ;
                           rdfs:comment "Describes what type of internal transportation a terminal uses for moving goods." .


###  https://w3id.org/latuli/ontology/tcm#hasMeasurementLimit
:hasMeasurementLimit rdf:type owl:ObjectProperty ;
                     rdfs:domain :PeriodicMeasurement ;
                     rdfs:range :MeasurementLimit ;
                     rdfs:comment "Relates a PeriodicMeasurement to a MeasurementLimit in order to specify the type of measurement made (average, min, max, etc.)" .


###  https://w3id.org/latuli/ontology/tcm#hasNetworkConnectivity
:hasNetworkConnectivity rdf:type owl:ObjectProperty ;
                        rdfs:domain :Terminal ;
                        rdfs:range :Connectivity ;
                        rdfs:comment "Describes how well-connected a terminal is, e.g. to main roads, main cities, etc." .


###  https://w3id.org/latuli/ontology/tcm#hasPeriodicMeasurement
:hasPeriodicMeasurement rdf:type owl:ObjectProperty ;
                        rdfs:domain :Throughput ;
                        rdfs:range :PeriodicMeasurement .


###  https://w3id.org/latuli/ontology/tcm#inboundDoor
:inboundDoor rdf:type owl:ObjectProperty ;
             rdfs:domain :Terminal ;
             rdfs:range :Door ;
             rdfs:comment "A door, or a dock, which can be used for receiving unloaded goods from a transport means." .


###  https://w3id.org/latuli/ontology/tcm#inboundTransportMeansFillRate
:inboundTransportMeansFillRate rdf:type owl:ObjectProperty ;
                               rdfs:domain :Terminal ;
                               rdfs:range :PeriodicMeasurement ;
                               rdfs:comment "A ratio describing how often (on average) transport means depart from the terminal without full load" .


###  https://w3id.org/latuli/ontology/tcm#intermediatePalletStorageCapacity
:intermediatePalletStorageCapacity rdf:type owl:ObjectProperty ;
                                   rdfs:domain :Terminal ;
                                   rdfs:range :Dimension ;
                                   rdfs:comment "Describes the capacity in terms of space (e.g. cubic or square meters) available for storing pallets intermediately." .


###  https://w3id.org/latuli/ontology/tcm#internalResourceCapacity
:internalResourceCapacity rdf:type owl:ObjectProperty ;
                          rdfs:domain :Terminal ;
                          rdfs:range :Dimension ;
                          rdfs:comment "The capacity of the conveyor belts network in an automated transportation mode, or the maximum number of workers available if the transportation is done manually, can be either considered limited or unlimited." .


###  https://w3id.org/latuli/ontology/tcm#isTerminalEquipmentType
:isTerminalEquipmentType rdf:type owl:ObjectProperty ;
                         rdfs:domain :TerminalEquipment ;
                         rdfs:range :TerminalEquipmentType .


###  https://w3id.org/latuli/ontology/tcm#loadingTime
:loadingTime rdf:type owl:ObjectProperty ;
             rdfs:domain :Terminal ;
             rdfs:range :PeriodicMeasurement ;
             rdfs:comment "The time it takes to load a transport means at the terminal." .


###  https://w3id.org/latuli/ontology/tcm#numInboundTransportMeansProcessed
:numInboundTransportMeansProcessed rdf:type owl:ObjectProperty ;
                                   rdfs:domain :Terminal ;
                                   rdfs:range :PeriodicMeasurement ;
                                   rdfs:comment "The number of inbound transport means processed in a given period of time" .


###  https://w3id.org/latuli/ontology/tcm#numMissedOrders
:numMissedOrders rdf:type owl:ObjectProperty ;
                 rdfs:domain :Terminal ;
                 rdfs:range :PeriodicMeasurement ;
                 rdfs:comment "The number of products that could not be loaded, or the corresponding lost profit." .


###  https://w3id.org/latuli/ontology/tcm#numOutboundTransportMeansProcessed
:numOutboundTransportMeansProcessed rdf:type owl:ObjectProperty ;
                                    rdfs:domain :Terminal ;
                                    rdfs:range :PeriodicMeasurement ;
                                    rdfs:comment "A measure specifying the number of loaded transport means (e.g. Trucks) processed at a terminal in a given period of time" .


###  https://w3id.org/latuli/ontology/tcm#numWorkers
:numWorkers rdf:type owl:ObjectProperty ;
            rdfs:domain :Terminal ;
            rdfs:range :PeriodicMeasurement .


###  https://w3id.org/latuli/ontology/tcm#numberOfLoadingUnitsProcessed
:numberOfLoadingUnitsProcessed rdf:type owl:ObjectProperty ;
                               rdfs:domain :Terminal ;
                               rdfs:range :PeriodicMeasurement ;
                               rdfs:comment "A measure specifying the number of loading units processed at a terminal in a given period of time" .


###  https://w3id.org/latuli/ontology/tcm#numberOfMovedPalletsPerHourCapacity
:numberOfMovedPalletsPerHourCapacity rdf:type owl:ObjectProperty ;
                                     rdfs:domain :Terminal ;
                                     rdfs:range :PeriodicMeasurement .


###  https://w3id.org/latuli/ontology/tcm#outboundDoor
:outboundDoor rdf:type owl:ObjectProperty ;
              rdfs:domain :Terminal ;
              rdfs:range :Door ;
              rdfs:comment "A door, or a dock, which can be used for sending goods to be loaded onto a transport means." .


###  https://w3id.org/latuli/ontology/tcm#outboundTransportMeansFillRate
:outboundTransportMeansFillRate rdf:type owl:ObjectProperty ;
                                rdfs:domain :Terminal ;
                                rdfs:range :PeriodicMeasurement .


###  https://w3id.org/latuli/ontology/tcm#overallThroughput
:overallThroughput rdf:type owl:ObjectProperty ;
                   rdfs:domain :Terminal ;
                   rdfs:range :Throughput .


###  https://w3id.org/latuli/ontology/tcm#percentTrailersDeclinedEntrance
:percentTrailersDeclinedEntrance rdf:type owl:ObjectProperty ;
                                 rdfs:domain :Terminal ;
                                 rdfs:range :PeriodicMeasurement ;
                                 rdfs:comment "Describes the percentage of trailers declined entrance upon arrival" .


###  https://w3id.org/latuli/ontology/tcm#percentTransportMeansDeclinedEntrance
:percentTransportMeansDeclinedEntrance rdf:type owl:ObjectProperty ;
                                       rdfs:domain :Terminal ;
                                       rdfs:range :PeriodicMeasurement ;
                                       rdfs:comment "Describes the percentage of transport means declined entrance upon arrival" .


###  https://w3id.org/latuli/ontology/tcm#periodicMeasurementDurationType
:periodicMeasurementDurationType rdf:type owl:ObjectProperty ;
                                 rdfs:domain :PeriodicMeasurement ;
                                 rdfs:range <http://www.w3.org/2006/time#TemporalUnit> ;
                                 rdfs:comment "Describes a specific duration of a PeriodicMeasurement" .


###  https://w3id.org/latuli/ontology/tcm#productType
:productType rdf:type owl:ObjectProperty ;
             rdfs:range :GoodsType ;
             rdfs:comment "Relates an Inventory with a GoodsType" .


###  https://w3id.org/latuli/ontology/tcm#splitShipmentHandlingIncidence
:splitShipmentHandlingIncidence rdf:type owl:ObjectProperty ;
                                rdfs:domain :Terminal ;
                                rdfs:range :PeriodicMeasurement .


###  https://w3id.org/latuli/ontology/tcm#storageCapacity
:storageCapacity rdf:type owl:ObjectProperty ;
                 rdfs:domain :Terminal ;
                 rdfs:range :Dimension ;
                 rdfs:comment "Describes the capacity (physical characteristics) of the storage function in a terminal" .


###  https://w3id.org/latuli/ontology/tcm#supportedGoodsType
:supportedGoodsType rdf:type owl:ObjectProperty ;
                    rdfs:domain :Terminal ;
                    rdfs:range :GoodsType ;
                    rdfs:comment "Describes the types of goods supported by the terminal." .


###  https://w3id.org/latuli/ontology/tcm#supportedLogisticsUnitType
:supportedLogisticsUnitType rdf:type owl:ObjectProperty ;
                            rdfs:domain :Terminal ;
                            rdfs:range :LogisticsUnit ;
                            rdfs:comment "Describes the types of logistics units supported at the terminal (e.g., containers, pallets, parcels, etc.)" .


###  https://w3id.org/latuli/ontology/tcm#supportedTransportMeansType
:supportedTransportMeansType rdf:type owl:ObjectProperty ;
                             rdfs:domain :Terminal ;
                             rdfs:range :TransportMeans ;
                             rdfs:comment "Describes the types of transport means supported at the terminal." .


###  https://w3id.org/latuli/ontology/tcm#supportedTransportMode
:supportedTransportMode rdf:type owl:ObjectProperty ;
                        rdfs:domain :Terminal ;
                        rdfs:range :TransportMode ;
                        rdfs:comment "Describes the types of transport modes supported at the terminal." .


###  https://w3id.org/latuli/ontology/tcm#temperatureControlledAreaSize
:temperatureControlledAreaSize rdf:type owl:ObjectProperty ;
                               rdfs:domain :Terminal ;
                               rdfs:range :Dimension ;
                               rdfs:comment "Describes the size of area within the terminal used for storing temperature controlled goods." .


###  https://w3id.org/latuli/ontology/tcm#terminalTotalSize
:terminalTotalSize rdf:type owl:ObjectProperty ;
                   rdfs:domain :Terminal ;
                   rdfs:range :Dimension ;
                   rdfs:comment "Describes the total size (physical characteristics) of a terminal." .


###  https://w3id.org/latuli/ontology/tcm#transhipmentTime
:transhipmentTime rdf:type owl:ObjectProperty ;
                  rdfs:domain :Terminal ;
                  rdfs:range :PeriodicMeasurement ;
                  rdfs:comment "The processing time  (e.g. for a shipment or a consignment) from it arrives at the terminal until it leaves the terminal." .


###  https://w3id.org/latuli/ontology/tcm#transitCenterSize
:transitCenterSize rdf:type owl:ObjectProperty ;
                   rdfs:domain :Terminal ;
                   rdfs:range :Dimension ;
                   rdfs:comment "Describes the size (physical characteristics) of the transit center in a terminal" .


###  https://w3id.org/latuli/ontology/tcm#typeOfGate
:typeOfGate rdf:type owl:ObjectProperty ;
            rdfs:domain :Terminal ;
            rdfs:range :Gate .


###  https://w3id.org/latuli/ontology/tcm#unloadingTime
:unloadingTime rdf:type owl:ObjectProperty ;
               rdfs:domain :Terminal ;
               rdfs:range :PeriodicMeasurement ;
               rdfs:comment "The time it takes to unload a transport means at the terminal." .


###  https://w3id.org/latuli/ontology/tcm#usedTerminalEquipment
:usedTerminalEquipment rdf:type owl:ObjectProperty ;
                       rdfs:domain :Terminal ;
                       rdfs:range :TerminalEquipment ;
                       rdfs:comment "Describes what type of terminal equipment is used by the terminal." .


###  https://w3id.org/latuli/ontology/tcm#waitingTimeInboundTransportMeans
:waitingTimeInboundTransportMeans rdf:type owl:ObjectProperty ;
                                  rdfs:domain :Terminal ;
                                  rdfs:range :PeriodicMeasurement ;
                                  rdfs:comment "Time spent at docks waiting to unload goods." .


###  https://w3id.org/latuli/ontology/tcm#waitingTimeOutboundTransportMeans
:waitingTimeOutboundTransportMeans rdf:type owl:ObjectProperty ;
                                   rdfs:domain :Terminal ;
                                   rdfs:range :PeriodicMeasurement ;
                                   rdfs:comment "Time spent at docks waiting to transport goods from terminal." .


#################################################################
#    Data properties
#################################################################

###  https://w3id.org/latuli/ontology/tcm#amount
:amount rdf:type owl:DatatypeProperty ;
        rdfs:domain :TerminalEquipment ;
        rdfs:range xsd:int .


###  https://w3id.org/latuli/ontology/tcm#automatedAccessControl
:automatedAccessControl rdf:type owl:DatatypeProperty ;
                        rdfs:domain :GateCharacteristics ;
                        rdfs:range xsd:boolean .


###  https://w3id.org/latuli/ontology/tcm#averageNumberOfWorkingHours
:averageNumberOfWorkingHours rdf:type owl:DatatypeProperty ;
                             rdfs:subPropertyOf owl:topDataProperty ;
                             rdfs:domain :Terminal ;
                             rdfs:range xsd:decimal ;
                             rdfs:comment "The average number of working hours per week at the terminal" .


###  https://w3id.org/latuli/ontology/tcm#bonded
:bonded rdf:type owl:DatatypeProperty ;
        rdfs:domain :GateCharacteristics ;
        rdfs:range xsd:boolean .


###  https://w3id.org/latuli/ontology/tcm#city
:city rdf:type owl:DatatypeProperty ;
      rdfs:domain :Terminal ;
      rdfs:range xsd:string .


###  https://w3id.org/latuli/ontology/tcm#closeAdherenceToSchedule
:closeAdherenceToSchedule rdf:type owl:DatatypeProperty ;
                          rdfs:domain :Terminal ;
                          rdfs:range xsd:boolean ;
                          rdfs:comment "A flag stating whether the terminal adheres to the schedule." .


###  https://w3id.org/latuli/ontology/tcm#combinedManualAndAutomatedInternalTransportation
:combinedManualAndAutomatedInternalTransportation rdf:type owl:DatatypeProperty ;
                                                  rdfs:subPropertyOf owl:topDataProperty ;
                                                  rdfs:domain :InternalTransportation ;
                                                  rdfs:range xsd:boolean ;
                                                  rdfs:comment "A flag that defines whether the internal transportation at the terminal is a combination of automated and manual (true) or not (false)" .


###  https://w3id.org/latuli/ontology/tcm#country
:country rdf:type owl:DatatypeProperty ;
         rdfs:domain :Terminal ;
         rdfs:range xsd:string .


###  https://w3id.org/latuli/ontology/tcm#cutOffTime
:cutOffTime rdf:type owl:DatatypeProperty ;
            rdfs:domain :Terminal ;
            rdfs:range xsd:string .


###  https://w3id.org/latuli/ontology/tcm#dimensionMeasurementValue
:dimensionMeasurementValue rdf:type owl:DatatypeProperty ;
                           rdfs:domain :Dimension ;
                           rdfs:range xsd:int ;
                           rdfs:comment "A value that specifies a dimension measurement (e.g. The total size of a terminal has a value of 1000 (square metres))." .


###  https://w3id.org/latuli/ontology/tcm#doorUtilisationRate
:doorUtilisationRate rdf:type owl:DatatypeProperty ;
                     rdfs:domain :Terminal ;
                     rdfs:range xsd:decimal ;
                     rdfs:comment "Describes the occupation time of doors at the terminal." .


###  https://w3id.org/latuli/ontology/tcm#gateNumber
:gateNumber rdf:type owl:DatatypeProperty ;
            rdfs:domain :Gate ;
            rdfs:range xsd:string .


###  https://w3id.org/latuli/ontology/tcm#geographicalCoordinateSystem
:geographicalCoordinateSystem rdf:type owl:DatatypeProperty ;
                              rdfs:domain :Terminal ;
                              rdfs:range xsd:string .


###  https://w3id.org/latuli/ontology/tcm#numDoors
:numDoors rdf:type owl:DatatypeProperty ;
          rdfs:domain :Door ;
          rdfs:range xsd:int .


###  https://w3id.org/latuli/ontology/tcm#numberOfInboundDoors
:numberOfInboundDoors rdf:type owl:DatatypeProperty ;
                      rdfs:subPropertyOf owl:topDataProperty ;
                      rdfs:domain :Terminal ;
                      rdfs:range xsd:int ;
                      rdfs:comment "The number of inbound doors available at a terminal." .


###  https://w3id.org/latuli/ontology/tcm#numberOfLanes
:numberOfLanes rdf:type owl:DatatypeProperty ;
               rdfs:domain :Terminal ;
               rdfs:range xsd:int .


###  https://w3id.org/latuli/ontology/tcm#numberOfOutboundDoors
:numberOfOutboundDoors rdf:type owl:DatatypeProperty ;
                       rdfs:subPropertyOf owl:topDataProperty ;
                       rdfs:domain :Terminal ;
                       rdfs:range xsd:int ;
                       rdfs:comment "The number of outbound doors available at a terminal." .


###  https://w3id.org/latuli/ontology/tcm#numberOfParkingBaysInBuffer
:numberOfParkingBaysInBuffer rdf:type owl:DatatypeProperty ;
                             rdfs:subPropertyOf owl:topDataProperty ;
                             rdfs:domain :Terminal ;
                             rdfs:range xsd:int ;
                             rdfs:comment "Describes the number of transport mode parking bays in a buffer zone." .


###  https://w3id.org/latuli/ontology/tcm#numberOfReeferContainerParkingBays
:numberOfReeferContainerParkingBays rdf:type owl:DatatypeProperty ;
                                    rdfs:domain :Terminal ;
                                    rdfs:range xsd:int .


###  https://w3id.org/latuli/ontology/tcm#numberOfShifts
:numberOfShifts rdf:type owl:DatatypeProperty ;
                rdfs:domain :Terminal ;
                rdfs:range xsd:int .


###  https://w3id.org/latuli/ontology/tcm#numberOfSwitchBays
:numberOfSwitchBays rdf:type owl:DatatypeProperty ;
                    rdfs:subPropertyOf owl:topDataProperty ;
                    rdfs:domain :Terminal ;
                    rdfs:range xsd:int ;
                    rdfs:comment "A location where logistics units (e.g., containers) are transferred between different transport means (e.g., rail to road)" .


###  https://w3id.org/latuli/ontology/tcm#numberOfTrailerParkingBays
:numberOfTrailerParkingBays rdf:type owl:DatatypeProperty ;
                            rdfs:subPropertyOf owl:topDataProperty ;
                            rdfs:domain :Terminal ;
                            rdfs:range xsd:int ;
                            rdfs:comment "Describes the number of parking bays allocated to trailers" .


###  https://w3id.org/latuli/ontology/tcm#numberOfTransportMeansParkingBays
:numberOfTransportMeansParkingBays rdf:type owl:DatatypeProperty ;
                                   rdfs:subPropertyOf owl:topDataProperty ;
                                   rdfs:domain :Terminal ;
                                   rdfs:range xsd:int ;
                                   rdfs:comment "Describes the number of parking bays allocated to transport means" .


###  https://w3id.org/latuli/ontology/tcm#onlyAutomatedInternalTransportation
:onlyAutomatedInternalTransportation rdf:type owl:DatatypeProperty ;
                                     rdfs:subPropertyOf owl:topDataProperty ;
                                     rdfs:domain :InternalTransportation ;
                                     rdfs:range xsd:boolean ;
                                     rdfs:comment "A flag that defines whether the internal transportation at the terminal is only automated (true) or not (false)" .


###  https://w3id.org/latuli/ontology/tcm#onlyManualInternalTransportation
:onlyManualInternalTransportation rdf:type owl:DatatypeProperty ;
                                  rdfs:subPropertyOf owl:topDataProperty ;
                                  rdfs:domain :InternalTransportation ;
                                  rdfs:range xsd:boolean ;
                                  rdfs:comment "A flag that defines whether the internal transportation at the terminal is only manual (true) or not (false)" .


###  https://w3id.org/latuli/ontology/tcm#periodicMeasurementValue
:periodicMeasurementValue rdf:type owl:DatatypeProperty ;
                          rdfs:domain :PeriodicMeasurement ;
                          rdfs:range xsd:int ;
                          rdfs:comment "A value that specifies a periodic measurement (e.g. the average unloading time at terminal X is 30 (minutes))." .


###  https://w3id.org/latuli/ontology/tcm#postalCode
:postalCode rdf:type owl:DatatypeProperty ;
            rdfs:domain :Terminal ;
            rdfs:range xsd:string .


###  https://w3id.org/latuli/ontology/tcm#preemptionAllowed
:preemptionAllowed rdf:type owl:DatatypeProperty ;
                   rdfs:domain :Terminal ;
                   rdfs:range xsd:boolean ;
                   rdfs:comment "Describes whether the loading or unloading of a truck can be interrupted and must be completed later." .


###  https://w3id.org/latuli/ontology/tcm#streetAddress
:streetAddress rdf:type owl:DatatypeProperty ;
               rdfs:domain :Terminal ;
               rdfs:range xsd:string .


###  https://w3id.org/latuli/ontology/tcm#twentyFourHoursService
:twentyFourHoursService rdf:type owl:DatatypeProperty ;
                        rdfs:domain :Terminal ;
                        rdfs:range xsd:boolean .


#################################################################
#    Classes
#################################################################

###  https://w3id.org/latuli/ontology/tcm#Connectivity
:Connectivity rdf:type owl:Class ;
              rdfs:comment "Describes how well-connected a terminal is, for example in terms of connectivity to main cities, main roads, etc." .


###  https://w3id.org/latuli/ontology/tcm#Dimension
:Dimension rdf:type owl:Class ;
           rdfs:comment "Defines a measurable dimension (length, mass, weight, volume, or area) of an item." .


###  https://w3id.org/latuli/ontology/tcm#Door
:Door rdf:type owl:Class ;
      rdfs:comment "A Door, or a dock, which is used to receive unloaded goods from transport means and to load goods onto transport means." .


###  https://w3id.org/latuli/ontology/tcm#DoorType
:DoorType rdf:type owl:Class ;
          rdfs:comment "Describes a type of door or dock at the terminal." .


###  https://w3id.org/latuli/ontology/tcm#Gate
:Gate rdf:type owl:Class ;
      rdfs:comment "A Gate is a facility for performing access control at a terminal." .


###  https://w3id.org/latuli/ontology/tcm#GateCharacteristics
:GateCharacteristics rdf:type owl:Class ;
                     rdfs:comment "Describes different types of characteristics for a gate." .


###  https://w3id.org/latuli/ontology/tcm#GoodsType
:GoodsType rdf:type owl:Class ;
           rdfs:comment "Describes a classification of goods being managed during a freight logistics operation." .


###  https://w3id.org/latuli/ontology/tcm#InternalTransportation
:InternalTransportation rdf:type owl:Class ;
                        rdfs:comment "Describes how the internal transportation of goods is performed within a terminal." .


###  https://w3id.org/latuli/ontology/tcm#LogisticsUnit
:LogisticsUnit rdf:type owl:Class ;
               rdfs:comment "Describes a uniquely identifiable unit consisting of one or more packages, goods items, or pieces of transport equipment." .


###  https://w3id.org/latuli/ontology/tcm#MeasurementLimit
:MeasurementLimit rdf:type owl:Class ;
                  rdfs:comment "Describes the type of periodic measurement being made. Examples are average, maximum, minimum, median and standard deviation." .


###  https://w3id.org/latuli/ontology/tcm#MeasurementType
:MeasurementType rdf:type owl:Class ;
                 rdfs:comment "Describes different types of measurement units. Examples are metre, cubic and gram." .


###  https://w3id.org/latuli/ontology/tcm#PeriodicMeasurement
:PeriodicMeasurement rdf:type owl:Class ;
                     rdfs:comment "Describes a periodic measurement of some performance indicator related to a freight terminal." .


###  https://w3id.org/latuli/ontology/tcm#ServiceMode
:ServiceMode rdf:type owl:Class ;
             rdfs:comment "Describes whether the door mode at a terminal is exclusive or mixed. The door mode is exclusive if each door is dedicated either to inbound trucks or outbound trucks exclusively. The door mode is mixed if a truck can be docked at any door." .


###  https://w3id.org/latuli/ontology/tcm#Terminal
:Terminal rdf:type owl:Class ;
          rdfs:subClassOf <http://www.opengis.net/ont/geosparql#Feature> ;
          rdfs:comment "A freight terminal is a processing node for freight. They may include airports, seaports, railroad terminals, and trucking terminals." .


###  https://w3id.org/latuli/ontology/tcm#TerminalEquipment
:TerminalEquipment rdf:type owl:Class ;
                   rdfs:comment "Terminal equipment used by the terminal." .


###  https://w3id.org/latuli/ontology/tcm#TerminalEquipmentType
:TerminalEquipmentType rdf:type owl:Class ;
                       rdfs:comment "Type of terminal equipment, such as forklifts, conveyor belts, etc." .


###  https://w3id.org/latuli/ontology/tcm#Throughput
:Throughput rdf:type owl:Class ;
            rdfs:comment "Describes the throughput of goods at a terminal for a particular period of time." .


###  https://w3id.org/latuli/ontology/tcm#TransportMeans
:TransportMeans rdf:type owl:Class ;
                rdfs:comment "A transport means is a particular device (with its own engine/power) used to convey goods or other objects from place to place during logistics cargo movements." .


###  https://w3id.org/latuli/ontology/tcm#TransportMode
:TransportMode rdf:type owl:Class ;
               rdfs:comment "Describes the mode of transportation being used on a transportation segment. Examples are AirTransport, RoadTransport, RailTransport and MaritimeTransport." .


#################################################################
#    Individuals
#################################################################

###  https://w3id.org/latuli/ontology/tcm#Aircraft
:Aircraft rdf:type owl:NamedIndividual ,
                   :TransportMeans .


###  https://w3id.org/latuli/ontology/tcm#Carton
:Carton rdf:type owl:NamedIndividual ,
                 :LogisticsUnit .


###  https://w3id.org/latuli/ontology/tcm#CubicMeter
:CubicMeter rdf:type owl:NamedIndividual ,
                     :MeasurementType .


###  https://w3id.org/latuli/ontology/tcm#Meter
:Meter rdf:type owl:NamedIndividual ,
                :MeasurementType .


###  https://w3id.org/latuli/ontology/tcm#Multimodal
:Multimodal rdf:type owl:NamedIndividual ,
                     :TransportMode .


###  https://w3id.org/latuli/ontology/tcm#Pallet
:Pallet rdf:type owl:NamedIndividual ,
                 :LogisticsUnit .


###  https://w3id.org/latuli/ontology/tcm#Ship
:Ship rdf:type owl:NamedIndividual ,
               :TransportMeans .


###  https://w3id.org/latuli/ontology/tcm#SquareMeter
:SquareMeter rdf:type owl:NamedIndividual ,
                      :MeasurementType .


###  https://w3id.org/latuli/ontology/tcm#Train
:Train rdf:type owl:NamedIndividual ,
                :TransportMeans .


###  https://w3id.org/latuli/ontology/tcm#Truck
:Truck rdf:type owl:NamedIndividual ,
                :TransportMeans .


###  https://w3id.org/latuli/ontology/tcm#UniModal
:UniModal rdf:type owl:NamedIndividual ,
                   :TransportMode .


###  https://w3id.org/latuli/ontology/tcm#avg
:avg rdf:type owl:NamedIndividual ,
              :MeasurementLimit .


###  https://w3id.org/latuli/ontology/tcm#max
:max rdf:type owl:NamedIndividual ,
              :MeasurementLimit .


###  https://w3id.org/latuli/ontology/tcm#min
:min rdf:type owl:NamedIndividual ,
              :MeasurementLimit .


###  Generated by the OWL API (version 4.5.9.2019-02-01T07:24:44Z) https://github.com/owlcs/owlapi
