<?xml version="1.0"?>
<rdf:RDF xmlns="https://w3id.org/latuli/ontology/m3#"
     xml:base="https://w3id.org/latuli/ontology/m3"
     xmlns:dc="http://purl.org/dc/elements/1.1/"
     xmlns:owl="http://www.w3.org/2002/07/owl#"
     xmlns:rdf="http://www.w3.org/1999/02/22-rdf-syntax-ns#"
     xmlns:xml="http://www.w3.org/XML/1998/namespace"
     xmlns:xsd="http://www.w3.org/2001/XMLSchema#"
     xmlns:rdfs="http://www.w3.org/2000/01/rdf-schema#"
     xmlns:skos="http://www.w3.org/2004/02/skos/core#"
     xmlns:terms="http://purl.org/dc/terms/">
    <owl:Ontology rdf:about="https://w3id.org/latuli/ontology/m3#">
        <owl:imports rdf:resource="http://www.opengis.net/ont/geosparql"/>
    </owl:Ontology>
    


    <!-- 
    ///////////////////////////////////////////////////////////////////////////////////////
    //
    // Annotation properties
    //
    ///////////////////////////////////////////////////////////////////////////////////////
     -->


    


    <!-- http://www.w3.org/2004/02/skos/core#prefLabel -->


    <owl:AnnotationProperty rdf:about="http://www.w3.org/2004/02/skos/core#prefLabel"/>
    


    <!-- 
    ///////////////////////////////////////////////////////////////////////////////////////
    //
    // Datatypes
    //
    ///////////////////////////////////////////////////////////////////////////////////////
     -->


    


    <!-- http://www.opengis.net/ont/geosparql#gmlLiteral -->


    <rdfs:Datatype rdf:about="http://www.opengis.net/ont/geosparql#gmlLiteral">
        <dc:contributor>Matthew Perry</dc:contributor>
        <dc:creator>OGC GeoSPARQL 1.0 Standard Working Group</dc:creator>
        <dc:date rdf:datatype="http://www.w3.org/2001/XMLSchema#date">2011-06-16</dc:date>
        <dc:description xml:lang="en">
      A GML serialization of a geometry object.
    </dc:description>
        <rdfs:comment xml:lang="en">
      A GML serialization of a geometry object.
    </rdfs:comment>
        <rdfs:isDefinedBy rdf:resource="http://www.opengis.net/ont/geosparql"/>
        <rdfs:isDefinedBy rdf:resource="http://www.opengis.net/spec/geosparql/1.0"/>
        <rdfs:label xml:lang="en">GML Literal</rdfs:label>
        <skos:definition xml:lang="en">
      A GML serialization of a geometry object.
    </skos:definition>
        <skos:prefLabel xml:lang="en">GML Literal</skos:prefLabel>
    </rdfs:Datatype>
    


    <!-- http://www.opengis.net/ont/geosparql#wktLiteral -->


    <rdfs:Datatype rdf:about="http://www.opengis.net/ont/geosparql#wktLiteral">
        <dc:contributor>Matthew Perry</dc:contributor>
        <dc:creator>OGC GeoSPARQL 1.0 Standard Working Group</dc:creator>
        <dc:date rdf:datatype="http://www.w3.org/2001/XMLSchema#date">2011-06-16</dc:date>
        <dc:description xml:lang="en">
      A Well-known Text serialization of a geometry object.
    </dc:description>
        <rdfs:comment xml:lang="en">
      A Well-known Text serialization of a geometry object.
    </rdfs:comment>
        <rdfs:isDefinedBy rdf:resource="http://www.opengis.net/ont/geosparql"/>
        <rdfs:isDefinedBy rdf:resource="http://www.opengis.net/spec/geosparql/1.0"/>
        <rdfs:label xml:lang="en">Well-known Text Literal</rdfs:label>
        <skos:definition xml:lang="en">
      A Well-known Text serialization of a geometry object.
    </skos:definition>
        <skos:prefLabel xml:lang="en">Well-known Text Literal</skos:prefLabel>
    </rdfs:Datatype>
    


    <!-- 
    ///////////////////////////////////////////////////////////////////////////////////////
    //
    // Object Properties
    //
    ///////////////////////////////////////////////////////////////////////////////////////
     -->


    


    <!-- http://www.opengis.net/ont/geosparql#defaultGeometry -->


    <owl:ObjectProperty rdf:about="http://www.opengis.net/ont/geosparql#defaultGeometry">
        <rdfs:subPropertyOf rdf:resource="http://www.opengis.net/ont/geosparql#hasGeometry"/>
        <rdfs:domain rdf:resource="http://www.opengis.net/ont/geosparql#Feature"/>
        <rdfs:range rdf:resource="http://www.opengis.net/ont/geosparql#Geometry"/>
        <dc:contributor>Matthew Perry</dc:contributor>
        <dc:creator>OGC GeoSPARQL 1.0 Standard Working Group</dc:creator>
        <dc:date rdf:datatype="http://www.w3.org/2001/XMLSchema#date">2011-06-16</dc:date>
        <dc:description xml:lang="en">
      The default geometry to be used in spatial calculations.
      It is Usually the most detailed geometry.
    </dc:description>
        <rdfs:comment xml:lang="en">
      The default geometry to be used in spatial calculations.
      It is Usually the most detailed geometry.
    </rdfs:comment>
        <rdfs:isDefinedBy rdf:resource="http://www.opengis.net/ont/geosparql"/>
        <rdfs:isDefinedBy rdf:resource="http://www.opengis.net/spec/geosparql/1.0"/>
        <rdfs:label xml:lang="en">defaultGeometry</rdfs:label>
        <skos:definition xml:lang="en">
      The default geometry to be used in spatial calculations.
      It is Usually the most detailed geometry.
    </skos:definition>
        <skos:prefLabel xml:lang="en">defaultGeometry</skos:prefLabel>
    </owl:ObjectProperty>
    


    <!-- http://www.opengis.net/ont/geosparql#ehContains -->


    <owl:ObjectProperty rdf:about="http://www.opengis.net/ont/geosparql#ehContains">
        <rdfs:domain rdf:resource="http://www.opengis.net/ont/geosparql#SpatialObject"/>
        <rdfs:range rdf:resource="http://www.opengis.net/ont/geosparql#SpatialObject"/>
        <dc:contributor>Matthew Perry</dc:contributor>
        <dc:creator>OGC GeoSPARQL 1.0 Standard Working Group</dc:creator>
        <dc:date rdf:datatype="http://www.w3.org/2001/XMLSchema#date">2011-06-16</dc:date>
        <dc:description xml:lang="en">
      Exists if the subject SpatialObject spatially contains the 
      object SpatialObject. DE-9IM: T*TFF*FF*
    </dc:description>
        <rdfs:comment xml:lang="en">
      Exists if the subject SpatialObject spatially contains the 
      object SpatialObject. DE-9IM: T*TFF*FF*
    </rdfs:comment>
        <rdfs:isDefinedBy rdf:resource="http://www.opengis.net/ont/geosparql"/>
        <rdfs:isDefinedBy rdf:resource="http://www.opengis.net/spec/geosparql/1.0"/>
        <rdfs:label xml:lang="en">contains</rdfs:label>
        <skos:definition xml:lang="en">
      Exists if the subject SpatialObject spatially contains the 
      object SpatialObject. DE-9IM: T*TFF*FF*
    </skos:definition>
        <skos:prefLabel xml:lang="en">contains</skos:prefLabel>
    </owl:ObjectProperty>
    


    <!-- http://www.opengis.net/ont/geosparql#ehCoveredBy -->


    <owl:ObjectProperty rdf:about="http://www.opengis.net/ont/geosparql#ehCoveredBy">
        <rdfs:domain rdf:resource="http://www.opengis.net/ont/geosparql#SpatialObject"/>
        <rdfs:range rdf:resource="http://www.opengis.net/ont/geosparql#SpatialObject"/>
        <dc:contributor>Matthew Perry</dc:contributor>
        <dc:creator>OGC GeoSPARQL 1.0 Standard Working Group</dc:creator>
        <dc:date rdf:datatype="http://www.w3.org/2001/XMLSchema#date">2011-06-16</dc:date>
        <dc:description xml:lang="en">
      Exists if the subject SpatialObject is spatially covered 
      by the object SpatialObject. DE-9IM: TFF*TFT**
    </dc:description>
        <rdfs:comment xml:lang="en">
      Exists if the subject SpatialObject is spatially covered 
      by the object SpatialObject. DE-9IM: TFF*TFT**
    </rdfs:comment>
        <rdfs:isDefinedBy rdf:resource="http://www.opengis.net/ont/geosparql"/>
        <rdfs:isDefinedBy rdf:resource="http://www.opengis.net/spec/geosparql/1.0"/>
        <rdfs:label xml:lang="en">coveredBy</rdfs:label>
        <skos:definition xml:lang="en">
      Exists if the subject SpatialObject is spatially covered 
      by the object SpatialObject. DE-9IM: TFF*TFT**
    </skos:definition>
        <skos:prefLabel xml:lang="en">coveredBy</skos:prefLabel>
    </owl:ObjectProperty>
    


    <!-- http://www.opengis.net/ont/geosparql#ehCovers -->


    <owl:ObjectProperty rdf:about="http://www.opengis.net/ont/geosparql#ehCovers">
        <rdfs:domain rdf:resource="http://www.opengis.net/ont/geosparql#SpatialObject"/>
        <rdfs:range rdf:resource="http://www.opengis.net/ont/geosparql#SpatialObject"/>
        <dc:contributor>Matthew Perry</dc:contributor>
        <dc:creator>OGC GeoSPARQL 1.0 Standard Working Group</dc:creator>
        <dc:date rdf:datatype="http://www.w3.org/2001/XMLSchema#date">2011-06-16</dc:date>
        <dc:description xml:lang="en">
      Exists if the subject SpatialObject spatially covers the 
      object SpatialObject. DE-9IM: T*TFT*FF*
    </dc:description>
        <rdfs:comment xml:lang="en">
      Exists if the subject SpatialObject spatially covers the 
      object SpatialObject. DE-9IM: T*TFT*FF*
    </rdfs:comment>
        <rdfs:isDefinedBy rdf:resource="http://www.opengis.net/ont/geosparql"/>
        <rdfs:isDefinedBy rdf:resource="http://www.opengis.net/spec/geosparql/1.0"/>
        <rdfs:label xml:lang="en">covers</rdfs:label>
        <skos:definition xml:lang="en">
      Exists if the subject SpatialObject spatially covers the 
      object SpatialObject. DE-9IM: T*TFT*FF*
    </skos:definition>
        <skos:prefLabel xml:lang="en">covers</skos:prefLabel>
    </owl:ObjectProperty>
    


    <!-- http://www.opengis.net/ont/geosparql#ehDisjoint -->


    <owl:ObjectProperty rdf:about="http://www.opengis.net/ont/geosparql#ehDisjoint">
        <rdfs:domain rdf:resource="http://www.opengis.net/ont/geosparql#SpatialObject"/>
        <rdfs:range rdf:resource="http://www.opengis.net/ont/geosparql#SpatialObject"/>
        <dc:contributor>Matthew Perry</dc:contributor>
        <dc:creator>OGC GeoSPARQL 1.0 Standard Working Group</dc:creator>
        <dc:date rdf:datatype="http://www.w3.org/2001/XMLSchema#date">2011-06-16</dc:date>
        <dc:description xml:lang="en">
      Exists if the subject SpatialObject is spatially disjoint
      from the object SpatialObject. DE-9IM: FF*FF****
    </dc:description>
        <rdfs:comment xml:lang="en">
      Exists if the subject SpatialObject is spatially disjoint
      from the object SpatialObject. DE-9IM: FF*FF****
    </rdfs:comment>
        <rdfs:isDefinedBy rdf:resource="http://www.opengis.net/ont/geosparql"/>
        <rdfs:isDefinedBy rdf:resource="http://www.opengis.net/spec/geosparql/1.0"/>
        <rdfs:label xml:lang="en">disjoint</rdfs:label>
        <skos:definition xml:lang="en">
      Exists if the subject SpatialObject is spatially disjoint
      from the object SpatialObject. DE-9IM: FF*FF****
    </skos:definition>
        <skos:prefLabel xml:lang="en">disjoint</skos:prefLabel>
    </owl:ObjectProperty>
    


    <!-- http://www.opengis.net/ont/geosparql#ehEquals -->


    <owl:ObjectProperty rdf:about="http://www.opengis.net/ont/geosparql#ehEquals">
        <rdfs:domain rdf:resource="http://www.opengis.net/ont/geosparql#SpatialObject"/>
        <rdfs:range rdf:resource="http://www.opengis.net/ont/geosparql#SpatialObject"/>
        <dc:contributor>Matthew Perry</dc:contributor>
        <dc:creator>OGC GeoSPARQL 1.0 Standard Working Group</dc:creator>
        <dc:date rdf:datatype="http://www.w3.org/2001/XMLSchema#date">2011-06-16</dc:date>
        <dc:description xml:lang="en">
      Exists if the subject SpatialObject spatially equals the 
      object SpatialObject. DE-9IM: TFFFTFFFT
    </dc:description>
        <rdfs:comment xml:lang="en">
      Exists if the subject SpatialObject spatially equals the 
      object SpatialObject. DE-9IM: TFFFTFFFT
    </rdfs:comment>
        <rdfs:isDefinedBy rdf:resource="http://www.opengis.net/ont/geosparql"/>
        <rdfs:isDefinedBy rdf:resource="http://www.opengis.net/spec/geosparql/1.0"/>
        <rdfs:label xml:lang="en">equals</rdfs:label>
        <skos:definition xml:lang="en">
      Exists if the subject SpatialObject spatially equals the 
      object SpatialObject. DE-9IM: TFFFTFFFT
    </skos:definition>
        <skos:prefLabel xml:lang="en">equals</skos:prefLabel>
    </owl:ObjectProperty>
    


    <!-- http://www.opengis.net/ont/geosparql#ehInside -->


    <owl:ObjectProperty rdf:about="http://www.opengis.net/ont/geosparql#ehInside">
        <rdfs:domain rdf:resource="http://www.opengis.net/ont/geosparql#SpatialObject"/>
        <rdfs:range rdf:resource="http://www.opengis.net/ont/geosparql#SpatialObject"/>
        <dc:contributor>Matthew Perry</dc:contributor>
        <dc:creator>OGC GeoSPARQL 1.0 Standard Working Group</dc:creator>
        <dc:date rdf:datatype="http://www.w3.org/2001/XMLSchema#date">2011-06-16</dc:date>
        <dc:description xml:lang="en">
      Exists if the subject SpatialObject is spatially inside 
      the object SpatialObject. DE-9IM: TFF*FFT**
    </dc:description>
        <rdfs:comment xml:lang="en">
      Exists if the subject SpatialObject is spatially inside 
      the object SpatialObject. DE-9IM: TFF*FFT**
    </rdfs:comment>
        <rdfs:isDefinedBy rdf:resource="http://www.opengis.net/ont/geosparql"/>
        <rdfs:isDefinedBy rdf:resource="http://www.opengis.net/spec/geosparql/1.0"/>
        <rdfs:label xml:lang="en">inside</rdfs:label>
        <skos:definition xml:lang="en">
      Exists if the subject SpatialObject is spatially inside 
      the object SpatialObject. DE-9IM: TFF*FFT**
    </skos:definition>
        <skos:prefLabel xml:lang="en">inside</skos:prefLabel>
    </owl:ObjectProperty>
    


    <!-- http://www.opengis.net/ont/geosparql#ehMeet -->


    <owl:ObjectProperty rdf:about="http://www.opengis.net/ont/geosparql#ehMeet">
        <rdfs:domain rdf:resource="http://www.opengis.net/ont/geosparql#SpatialObject"/>
        <rdfs:range rdf:resource="http://www.opengis.net/ont/geosparql#SpatialObject"/>
        <dc:contributor>Matthew Perry</dc:contributor>
        <dc:creator>OGC GeoSPARQL 1.0 Standard Working Group</dc:creator>
        <dc:date rdf:datatype="http://www.w3.org/2001/XMLSchema#date">2011-06-16</dc:date>
        <dc:description xml:lang="en">
      Exists if the subject SpatialObject spatially meets the 
      object SpatialObject. 
      DE-9IM: FT******* ^ F**T***** ^ F***T****
    </dc:description>
        <rdfs:comment xml:lang="en">
      Exists if the subject SpatialObject spatially meets the 
      object SpatialObject. 
      DE-9IM: FT******* ^ F**T***** ^ F***T****
    </rdfs:comment>
        <rdfs:isDefinedBy rdf:resource="http://www.opengis.net/ont/geosparql"/>
        <rdfs:isDefinedBy rdf:resource="http://www.opengis.net/spec/geosparql/1.0"/>
        <rdfs:label xml:lang="en">meet</rdfs:label>
        <skos:definition xml:lang="en">
      Exists if the subject SpatialObject spatially meets the 
      object SpatialObject. 
      DE-9IM: FT******* ^ F**T***** ^ F***T****
    </skos:definition>
        <skos:prefLabel xml:lang="en">meet</skos:prefLabel>
    </owl:ObjectProperty>
    


    <!-- http://www.opengis.net/ont/geosparql#ehOverlap -->


    <owl:ObjectProperty rdf:about="http://www.opengis.net/ont/geosparql#ehOverlap">
        <rdfs:domain rdf:resource="http://www.opengis.net/ont/geosparql#SpatialObject"/>
        <rdfs:range rdf:resource="http://www.opengis.net/ont/geosparql#SpatialObject"/>
        <dc:contributor>Matthew Perry</dc:contributor>
        <dc:creator>OGC GeoSPARQL 1.0 Standard Working Group</dc:creator>
        <dc:date rdf:datatype="http://www.w3.org/2001/XMLSchema#date">2011-06-16</dc:date>
        <dc:description xml:lang="en">
      Exists if the subject SpatialObject spatially overlaps the 
      object SpatialObject. DE-9IM: T*T***T**
    </dc:description>
        <rdfs:comment xml:lang="en">
      Exists if the subject SpatialObject spatially overlaps the 
      object SpatialObject. DE-9IM: T*T***T**
    </rdfs:comment>
        <rdfs:isDefinedBy rdf:resource="http://www.opengis.net/ont/geosparql"/>
        <rdfs:isDefinedBy rdf:resource="http://www.opengis.net/spec/geosparql/1.0"/>
        <rdfs:label xml:lang="en">overlap</rdfs:label>
        <skos:definition xml:lang="en">
      Exists if the subject SpatialObject spatially overlaps the 
      object SpatialObject. DE-9IM: T*T***T**
    </skos:definition>
        <skos:prefLabel xml:lang="en">overlap</skos:prefLabel>
    </owl:ObjectProperty>
    


    <!-- http://www.opengis.net/ont/geosparql#hasGeometry -->


    <owl:ObjectProperty rdf:about="http://www.opengis.net/ont/geosparql#hasGeometry">
        <rdfs:domain rdf:resource="http://www.opengis.net/ont/geosparql#Feature"/>
        <rdfs:range rdf:resource="http://www.opengis.net/ont/geosparql#Geometry"/>
        <dc:contributor>Matthew Perry</dc:contributor>
        <dc:creator>OGC GeoSPARQL 1.0 Standard Working Group</dc:creator>
        <dc:date rdf:datatype="http://www.w3.org/2001/XMLSchema#date">2011-06-16</dc:date>
        <dc:description xml:lang="en">
      A spatial representation for a given feature.
    </dc:description>
        <rdfs:comment xml:lang="en">
      A spatial representation for a given feature.
    </rdfs:comment>
        <rdfs:isDefinedBy rdf:resource="http://www.opengis.net/ont/geosparql"/>
        <rdfs:isDefinedBy rdf:resource="http://www.opengis.net/spec/geosparql/1.0"/>
        <rdfs:label xml:lang="en">hasGeometry</rdfs:label>
        <skos:definition xml:lang="en">
      A spatial representation for a given feature.
    </skos:definition>
        <skos:prefLabel xml:lang="en">hasGeometry</skos:prefLabel>
    </owl:ObjectProperty>
    


    <!-- http://www.opengis.net/ont/geosparql#rcc8dc -->


    <owl:ObjectProperty rdf:about="http://www.opengis.net/ont/geosparql#rcc8dc">
        <rdfs:domain rdf:resource="http://www.opengis.net/ont/geosparql#SpatialObject"/>
        <rdfs:range rdf:resource="http://www.opengis.net/ont/geosparql#SpatialObject"/>
        <dc:contributor>Matthew Perry</dc:contributor>
        <dc:creator>OGC GeoSPARQL 1.0 Standard Working Group</dc:creator>
        <dc:date rdf:datatype="http://www.w3.org/2001/XMLSchema#date">2011-06-16</dc:date>
        <dc:description xml:lang="en">
      Exists if the subject SpatialObject is spatially disjoint
      from the object SpatialObject. DE-9IM: FFTFFTTTT
    </dc:description>
        <rdfs:comment xml:lang="en">
      Exists if the subject SpatialObject is spatially disjoint
      from the object SpatialObject. DE-9IM: FFTFFTTTT
    </rdfs:comment>
        <rdfs:isDefinedBy rdf:resource="http://www.opengis.net/ont/geosparql"/>
        <rdfs:isDefinedBy rdf:resource="http://www.opengis.net/spec/geosparql/1.0"/>
        <rdfs:label xml:lang="en">disconnected</rdfs:label>
        <skos:definition xml:lang="en">
      Exists if the subject SpatialObject is spatially disjoint
      from the object SpatialObject. DE-9IM: FFTFFTTTT
    </skos:definition>
        <skos:prefLabel xml:lang="en">disconnected</skos:prefLabel>
    </owl:ObjectProperty>
    


    <!-- http://www.opengis.net/ont/geosparql#rcc8ec -->


    <owl:ObjectProperty rdf:about="http://www.opengis.net/ont/geosparql#rcc8ec">
        <rdfs:domain rdf:resource="http://www.opengis.net/ont/geosparql#SpatialObject"/>
        <rdfs:range rdf:resource="http://www.opengis.net/ont/geosparql#SpatialObject"/>
        <dc:contributor>Matthew Perry</dc:contributor>
        <dc:creator>OGC GeoSPARQL 1.0 Standard Working Group</dc:creator>
        <dc:date rdf:datatype="http://www.w3.org/2001/XMLSchema#date">2011-06-16</dc:date>
        <dc:description xml:lang="en">
      Exists if the subject SpatialObject spatially meets the 
      object SpatialObject. DE-9IM: FFTFTTTTT
    </dc:description>
        <rdfs:comment xml:lang="en">
      Exists if the subject SpatialObject spatially meets the 
      object SpatialObject. DE-9IM: FFTFTTTTT
    </rdfs:comment>
        <rdfs:isDefinedBy rdf:resource="http://www.opengis.net/ont/geosparql"/>
        <rdfs:isDefinedBy rdf:resource="http://www.opengis.net/spec/geosparql/1.0"/>
        <rdfs:label xml:lang="en">externally connected</rdfs:label>
        <skos:definition xml:lang="en">
      Exists if the subject SpatialObject spatially meets the 
      object SpatialObject. DE-9IM: FFTFTTTTT
    </skos:definition>
        <skos:prefLabel xml:lang="en">externally connected</skos:prefLabel>
    </owl:ObjectProperty>
    


    <!-- http://www.opengis.net/ont/geosparql#rcc8eq -->


    <owl:ObjectProperty rdf:about="http://www.opengis.net/ont/geosparql#rcc8eq">
        <rdfs:domain rdf:resource="http://www.opengis.net/ont/geosparql#SpatialObject"/>
        <rdfs:range rdf:resource="http://www.opengis.net/ont/geosparql#SpatialObject"/>
        <dc:contributor>Matthew Perry</dc:contributor>
        <dc:creator>OGC GeoSPARQL 1.0 Standard Working Group</dc:creator>
        <dc:date rdf:datatype="http://www.w3.org/2001/XMLSchema#date">2011-06-16</dc:date>
        <dc:description xml:lang="en">
      Exists if the subject SpatialObject spatially equals the 
      object SpatialObject. DE-9IM: TFFFTFFFT
    </dc:description>
        <rdfs:comment xml:lang="en">
      Exists if the subject SpatialObject spatially equals the 
      object SpatialObject. DE-9IM: TFFFTFFFT
    </rdfs:comment>
        <rdfs:isDefinedBy rdf:resource="http://www.opengis.net/ont/geosparql"/>
        <rdfs:isDefinedBy rdf:resource="http://www.opengis.net/spec/geosparql/1.0"/>
        <rdfs:label xml:lang="en">equals</rdfs:label>
        <skos:definition xml:lang="en">
      Exists if the subject SpatialObject spatially equals the 
      object SpatialObject. DE-9IM: TFFFTFFFT
    </skos:definition>
        <skos:prefLabel xml:lang="en">equals</skos:prefLabel>
    </owl:ObjectProperty>
    


    <!-- http://www.opengis.net/ont/geosparql#rcc8ntpp -->


    <owl:ObjectProperty rdf:about="http://www.opengis.net/ont/geosparql#rcc8ntpp">
        <rdfs:domain rdf:resource="http://www.opengis.net/ont/geosparql#SpatialObject"/>
        <rdfs:range rdf:resource="http://www.opengis.net/ont/geosparql#SpatialObject"/>
        <dc:contributor>Matthew Perry</dc:contributor>
        <dc:creator>OGC GeoSPARQL 1.0 Standard Working Group</dc:creator>
        <dc:date rdf:datatype="http://www.w3.org/2001/XMLSchema#date">2011-06-16</dc:date>
        <dc:description xml:lang="en">
      Exists if the subject SpatialObject is spatially inside 
      the object SpatialObject. DE-9IM: TFFTFFTTT
    </dc:description>
        <rdfs:comment xml:lang="en">
      Exists if the subject SpatialObject is spatially inside 
      the object SpatialObject. DE-9IM: TFFTFFTTT
    </rdfs:comment>
        <rdfs:isDefinedBy rdf:resource="http://www.opengis.net/ont/geosparql"/>
        <rdfs:isDefinedBy rdf:resource="http://www.opengis.net/spec/geosparql/1.0"/>
        <rdfs:label xml:lang="en">non-tangential proper part</rdfs:label>
        <skos:definition xml:lang="en">
      Exists if the subject SpatialObject is spatially inside 
      the object SpatialObject. DE-9IM: TFFTFFTTT
    </skos:definition>
        <skos:prefLabel xml:lang="en">non-tangential proper part</skos:prefLabel>
    </owl:ObjectProperty>
    


    <!-- http://www.opengis.net/ont/geosparql#rcc8ntppi -->


    <owl:ObjectProperty rdf:about="http://www.opengis.net/ont/geosparql#rcc8ntppi">
        <rdfs:domain rdf:resource="http://www.opengis.net/ont/geosparql#SpatialObject"/>
        <rdfs:range rdf:resource="http://www.opengis.net/ont/geosparql#SpatialObject"/>
        <dc:contributor>Matthew Perry</dc:contributor>
        <dc:creator>OGC GeoSPARQL 1.0 Standard Working Group</dc:creator>
        <dc:date rdf:datatype="http://www.w3.org/2001/XMLSchema#date">2011-06-16</dc:date>
        <dc:description xml:lang="en">
      Exists if the subject SpatialObject spatially contains the 
      object SpatialObject. DE-9IM: TTTFFTFFT
    </dc:description>
        <rdfs:comment xml:lang="en">
      Exists if the subject SpatialObject spatially contains the 
      object SpatialObject. DE-9IM: TTTFFTFFT
    </rdfs:comment>
        <rdfs:isDefinedBy rdf:resource="http://www.opengis.net/ont/geosparql"/>
        <rdfs:isDefinedBy rdf:resource="http://www.opengis.net/spec/geosparql/1.0"/>
        <rdfs:label xml:lang="en">non-tangential proper part inverse</rdfs:label>
        <skos:definition xml:lang="en">
      Exists if the subject SpatialObject spatially contains the 
      object SpatialObject. DE-9IM: TTTFFTFFT
    </skos:definition>
        <skos:prefLabel xml:lang="en">non-tangential proper part inverse</skos:prefLabel>
    </owl:ObjectProperty>
    


    <!-- http://www.opengis.net/ont/geosparql#rcc8po -->


    <owl:ObjectProperty rdf:about="http://www.opengis.net/ont/geosparql#rcc8po">
        <rdfs:domain rdf:resource="http://www.opengis.net/ont/geosparql#SpatialObject"/>
        <rdfs:range rdf:resource="http://www.opengis.net/ont/geosparql#SpatialObject"/>
        <dc:contributor>Matthew Perry</dc:contributor>
        <dc:creator>OGC GeoSPARQL 1.0 Standard Working Group</dc:creator>
        <dc:date rdf:datatype="http://www.w3.org/2001/XMLSchema#date">2011-06-16</dc:date>
        <dc:description xml:lang="en">
      Exists if the subject SpatialObject spatially overlaps the 
      object SpatialObject. DE-9IM: TTTTTTTTT
    </dc:description>
        <rdfs:comment xml:lang="en">
      Exists if the subject SpatialObject spatially overlaps the 
      object SpatialObject. DE-9IM: TTTTTTTTT
    </rdfs:comment>
        <rdfs:isDefinedBy rdf:resource="http://www.opengis.net/ont/geosparql"/>
        <rdfs:isDefinedBy rdf:resource="http://www.opengis.net/spec/geosparql/1.0"/>
        <rdfs:label xml:lang="en">partially overlapping</rdfs:label>
        <skos:definition xml:lang="en">
      Exists if the subject SpatialObject spatially overlaps the 
      object SpatialObject. DE-9IM: TTTTTTTTT
    </skos:definition>
        <skos:prefLabel xml:lang="en">partially overlapping</skos:prefLabel>
    </owl:ObjectProperty>
    


    <!-- http://www.opengis.net/ont/geosparql#rcc8tpp -->


    <owl:ObjectProperty rdf:about="http://www.opengis.net/ont/geosparql#rcc8tpp">
        <rdfs:domain rdf:resource="http://www.opengis.net/ont/geosparql#SpatialObject"/>
        <rdfs:range rdf:resource="http://www.opengis.net/ont/geosparql#SpatialObject"/>
        <dc:contributor>Matthew Perry</dc:contributor>
        <dc:creator>OGC GeoSPARQL 1.0 Standard Working Group</dc:creator>
        <dc:date rdf:datatype="http://www.w3.org/2001/XMLSchema#date">2011-06-16</dc:date>
        <dc:description xml:lang="en">
      Exists if the subject SpatialObject is spatially covered 
      by the object SpatialObject. DE-9IM: TFFTTFTTT
    </dc:description>
        <rdfs:comment xml:lang="en">
      Exists if the subject SpatialObject is spatially covered 
      by the object SpatialObject. DE-9IM: TFFTTFTTT
    </rdfs:comment>
        <rdfs:isDefinedBy rdf:resource="http://www.opengis.net/ont/geosparql"/>
        <rdfs:isDefinedBy rdf:resource="http://www.opengis.net/spec/geosparql/1.0"/>
        <rdfs:label xml:lang="en">tangential proper part</rdfs:label>
        <skos:definition xml:lang="en">
      Exists if the subject SpatialObject is spatially covered 
      by the object SpatialObject. DE-9IM: TFFTTFTTT
    </skos:definition>
        <skos:prefLabel xml:lang="en">tangential proper part</skos:prefLabel>
    </owl:ObjectProperty>
    


    <!-- http://www.opengis.net/ont/geosparql#rcc8tppi -->


    <owl:ObjectProperty rdf:about="http://www.opengis.net/ont/geosparql#rcc8tppi">
        <rdfs:domain rdf:resource="http://www.opengis.net/ont/geosparql#SpatialObject"/>
        <rdfs:range rdf:resource="http://www.opengis.net/ont/geosparql#SpatialObject"/>
        <dc:contributor>Matthew Perry</dc:contributor>
        <dc:creator>OGC GeoSPARQL 1.0 Standard Working Group</dc:creator>
        <dc:date rdf:datatype="http://www.w3.org/2001/XMLSchema#date">2011-06-16</dc:date>
        <dc:description xml:lang="en">
      Exists if the subject SpatialObject spatially covers the 
      object SpatialObject. DE-9IM: TTTFTTFFT
    </dc:description>
        <rdfs:comment xml:lang="en">
      Exists if the subject SpatialObject spatially covers the 
      object SpatialObject. DE-9IM: TTTFTTFFT
    </rdfs:comment>
        <rdfs:isDefinedBy rdf:resource="http://www.opengis.net/ont/geosparql"/>
        <rdfs:isDefinedBy rdf:resource="http://www.opengis.net/spec/geosparql/1.0"/>
        <rdfs:label xml:lang="en">tangential proper part inverse</rdfs:label>
        <skos:definition xml:lang="en">
      Exists if the subject SpatialObject spatially covers the 
      object SpatialObject. DE-9IM: TTTFTTFFT
    </skos:definition>
        <skos:prefLabel xml:lang="en">tangential proper part inverse</skos:prefLabel>
    </owl:ObjectProperty>
    


    <!-- http://www.opengis.net/ont/geosparql#sfContains -->


    <owl:ObjectProperty rdf:about="http://www.opengis.net/ont/geosparql#sfContains">
        <rdfs:domain rdf:resource="http://www.opengis.net/ont/geosparql#SpatialObject"/>
        <rdfs:range rdf:resource="http://www.opengis.net/ont/geosparql#SpatialObject"/>
        <dc:contributor>Matthew Perry</dc:contributor>
        <dc:creator>OGC GeoSPARQL 1.0 Standard Working Group</dc:creator>
        <dc:date rdf:datatype="http://www.w3.org/2001/XMLSchema#date">2011-06-16</dc:date>
        <dc:description xml:lang="en">
      Exists if the subject SpatialObject spatially contains the 
      object SpatialObject. DE-9IM: T*****FF*
    </dc:description>
        <rdfs:comment xml:lang="en">
      Exists if the subject SpatialObject spatially contains the 
      object SpatialObject. DE-9IM: T*****FF*
    </rdfs:comment>
        <rdfs:isDefinedBy rdf:resource="http://www.opengis.net/ont/geosparql"/>
        <rdfs:isDefinedBy rdf:resource="http://www.opengis.net/spec/geosparql/1.0"/>
        <rdfs:label xml:lang="en">contains</rdfs:label>
        <skos:definition xml:lang="en">
      Exists if the subject SpatialObject spatially contains the 
      object SpatialObject. DE-9IM: T*****FF*
    </skos:definition>
        <skos:prefLabel xml:lang="en">contains</skos:prefLabel>
    </owl:ObjectProperty>
    


    <!-- http://www.opengis.net/ont/geosparql#sfCrosses -->


    <owl:ObjectProperty rdf:about="http://www.opengis.net/ont/geosparql#sfCrosses">
        <rdfs:domain rdf:resource="http://www.opengis.net/ont/geosparql#SpatialObject"/>
        <rdfs:range rdf:resource="http://www.opengis.net/ont/geosparql#SpatialObject"/>
        <dc:contributor>Matthew Perry</dc:contributor>
        <dc:creator>OGC GeoSPARQL 1.0 Standard Working Group</dc:creator>
        <dc:date rdf:datatype="http://www.w3.org/2001/XMLSchema#date">2011-06-16</dc:date>
        <dc:description xml:lang="en">
      Exists if the subject SpatialObject spatially crosses the 
      object SpatialObject. DE-9IM: T*T******
    </dc:description>
        <rdfs:comment xml:lang="en">
      Exists if the subject SpatialObject spatially crosses the 
      object SpatialObject. DE-9IM: T*T******
    </rdfs:comment>
        <rdfs:isDefinedBy rdf:resource="http://www.opengis.net/ont/geosparql"/>
        <rdfs:isDefinedBy rdf:resource="http://www.opengis.net/spec/geosparql/1.0"/>
        <rdfs:label xml:lang="en">crosses</rdfs:label>
        <skos:definition xml:lang="en">
      Exists if the subject SpatialObject spatially crosses the 
      object SpatialObject. DE-9IM: T*T******
    </skos:definition>
        <skos:prefLabel xml:lang="en">crosses</skos:prefLabel>
    </owl:ObjectProperty>
    


    <!-- http://www.opengis.net/ont/geosparql#sfDisjoint -->


    <owl:ObjectProperty rdf:about="http://www.opengis.net/ont/geosparql#sfDisjoint">
        <rdfs:domain rdf:resource="http://www.opengis.net/ont/geosparql#SpatialObject"/>
        <rdfs:range rdf:resource="http://www.opengis.net/ont/geosparql#SpatialObject"/>
        <dc:contributor>Matthew Perry</dc:contributor>
        <dc:creator>OGC GeoSPARQL 1.0 Standard Working Group</dc:creator>
        <dc:date rdf:datatype="http://www.w3.org/2001/XMLSchema#date">2011-06-16</dc:date>
        <dc:description xml:lang="en">
      Exists if the subject SpatialObject is spatially disjoint 
      from the object SpatialObject. DE-9IM: FF*FF****
    </dc:description>
        <rdfs:comment xml:lang="en">
      Exists if the subject SpatialObject is spatially disjoint 
      from the object SpatialObject. DE-9IM: FF*FF****
    </rdfs:comment>
        <rdfs:isDefinedBy rdf:resource="http://www.opengis.net/ont/geosparql"/>
        <rdfs:isDefinedBy rdf:resource="http://www.opengis.net/spec/geosparql/1.0"/>
        <rdfs:label xml:lang="en">disjoint</rdfs:label>
        <skos:definition xml:lang="en">
      Exists if the subject SpatialObject is spatially disjoint 
      from the object SpatialObject. DE-9IM: FF*FF****
    </skos:definition>
        <skos:prefLabel xml:lang="en">disjoint</skos:prefLabel>
    </owl:ObjectProperty>
    


    <!-- http://www.opengis.net/ont/geosparql#sfEquals -->


    <owl:ObjectProperty rdf:about="http://www.opengis.net/ont/geosparql#sfEquals">
        <rdfs:domain rdf:resource="http://www.opengis.net/ont/geosparql#SpatialObject"/>
        <rdfs:range rdf:resource="http://www.opengis.net/ont/geosparql#SpatialObject"/>
        <dc:contributor>Matthew Perry</dc:contributor>
        <dc:creator>OGC GeoSPARQL 1.0 Standard Working Group</dc:creator>
        <dc:date rdf:datatype="http://www.w3.org/2001/XMLSchema#date">2011-06-16</dc:date>
        <dc:description xml:lang="en">
      Exists if the subject SpatialObject spatially equals the 
      object SpatialObject. DE-9IM: TFFFTFFFT
    </dc:description>
        <rdfs:comment xml:lang="en">
      Exists if the subject SpatialObject spatially equals the 
      object SpatialObject. DE-9IM: TFFFTFFFT
    </rdfs:comment>
        <rdfs:isDefinedBy rdf:resource="http://www.opengis.net/ont/geosparql"/>
        <rdfs:isDefinedBy rdf:resource="http://www.opengis.net/spec/geosparql/1.0"/>
        <rdfs:label xml:lang="en">equals</rdfs:label>
        <skos:definition xml:lang="en">
      Exists if the subject SpatialObject spatially equals the 
      object SpatialObject. DE-9IM: TFFFTFFFT
    </skos:definition>
        <skos:prefLabel xml:lang="en">equals</skos:prefLabel>
    </owl:ObjectProperty>
    


    <!-- http://www.opengis.net/ont/geosparql#sfIntersects -->


    <owl:ObjectProperty rdf:about="http://www.opengis.net/ont/geosparql#sfIntersects">
        <rdfs:domain rdf:resource="http://www.opengis.net/ont/geosparql#SpatialObject"/>
        <rdfs:range rdf:resource="http://www.opengis.net/ont/geosparql#SpatialObject"/>
        <dc:contributor>Matthew Perry</dc:contributor>
        <dc:creator>OGC GeoSPARQL 1.0 Standard Working Group</dc:creator>
        <dc:date rdf:datatype="http://www.w3.org/2001/XMLSchema#date">2011-06-16</dc:date>
        <dc:description xml:lang="en">
      Exists if the subject SpatialObject is not spatially disjoint 
      from the object SpatialObject.
      DE-9IM: T******** ^ *T******* ^ ***T***** ^ ****T**** 
    </dc:description>
        <rdfs:comment xml:lang="en">
      Exists if the subject SpatialObject is not spatially disjoint 
      from the object SpatialObject.
      DE-9IM: T******** ^ *T******* ^ ***T***** ^ ****T**** 
    </rdfs:comment>
        <rdfs:isDefinedBy rdf:resource="http://www.opengis.net/ont/geosparql"/>
        <rdfs:isDefinedBy rdf:resource="http://www.opengis.net/spec/geosparql/1.0"/>
        <rdfs:label xml:lang="en">intersects</rdfs:label>
        <skos:definition xml:lang="en">
      Exists if the subject SpatialObject is not spatially disjoint 
      from the object SpatialObject.
      DE-9IM: T******** ^ *T******* ^ ***T***** ^ ****T**** 
    </skos:definition>
        <skos:prefLabel xml:lang="en">intersects</skos:prefLabel>
    </owl:ObjectProperty>
    


    <!-- http://www.opengis.net/ont/geosparql#sfOverlaps -->


    <owl:ObjectProperty rdf:about="http://www.opengis.net/ont/geosparql#sfOverlaps">
        <rdfs:domain rdf:resource="http://www.opengis.net/ont/geosparql#SpatialObject"/>
        <rdfs:range rdf:resource="http://www.opengis.net/ont/geosparql#SpatialObject"/>
        <dc:contributor>Matthew Perry</dc:contributor>
        <dc:creator>OGC GeoSPARQL 1.0 Standard Working Group</dc:creator>
        <dc:date rdf:datatype="http://www.w3.org/2001/XMLSchema#date">2011-06-16</dc:date>
        <dc:description xml:lang="en">
      Exists if the subject SpatialObject spatially overlaps the 
      object SpatialObject. DE-9IM: T*T***T** 
    </dc:description>
        <rdfs:comment xml:lang="en">
      Exists if the subject SpatialObject spatially overlaps the 
      object SpatialObject. DE-9IM: T*T***T** 
    </rdfs:comment>
        <rdfs:isDefinedBy rdf:resource="http://www.opengis.net/ont/geosparql"/>
        <rdfs:isDefinedBy rdf:resource="http://www.opengis.net/spec/geosparql/1.0"/>
        <rdfs:label xml:lang="en">overlaps</rdfs:label>
        <skos:definition xml:lang="en">
      Exists if the subject SpatialObject spatially overlaps the 
      object SpatialObject. DE-9IM: T*T***T** 
    </skos:definition>
        <skos:prefLabel xml:lang="en">overlaps</skos:prefLabel>
    </owl:ObjectProperty>
    


    <!-- http://www.opengis.net/ont/geosparql#sfTouches -->


    <owl:ObjectProperty rdf:about="http://www.opengis.net/ont/geosparql#sfTouches">
        <rdfs:domain rdf:resource="http://www.opengis.net/ont/geosparql#SpatialObject"/>
        <rdfs:range rdf:resource="http://www.opengis.net/ont/geosparql#SpatialObject"/>
        <dc:contributor>Matthew Perry</dc:contributor>
        <dc:creator>OGC GeoSPARQL 1.0 Standard Working Group</dc:creator>
        <dc:date rdf:datatype="http://www.w3.org/2001/XMLSchema#date">2011-06-16</dc:date>
        <dc:description xml:lang="en">
      Exists if the subject SpatialObject spatially touches the 
      object SpatialObject.
      DE-9IM: FT******* ^ F**T***** ^ F***T****
    </dc:description>
        <rdfs:comment xml:lang="en">
      Exists if the subject SpatialObject spatially touches the 
      object SpatialObject.
      DE-9IM: FT******* ^ F**T***** ^ F***T****
    </rdfs:comment>
        <rdfs:isDefinedBy rdf:resource="http://www.opengis.net/ont/geosparql"/>
        <rdfs:isDefinedBy rdf:resource="http://www.opengis.net/spec/geosparql/1.0"/>
        <rdfs:label xml:lang="en">touches</rdfs:label>
        <skos:definition xml:lang="en">
      Exists if the subject SpatialObject spatially touches the 
      object SpatialObject.
      DE-9IM: FT******* ^ F**T***** ^ F***T****
    </skos:definition>
        <skos:prefLabel xml:lang="en">touches</skos:prefLabel>
    </owl:ObjectProperty>
    


    <!-- http://www.opengis.net/ont/geosparql#sfWithin -->


    <owl:ObjectProperty rdf:about="http://www.opengis.net/ont/geosparql#sfWithin">
        <rdfs:domain rdf:resource="http://www.opengis.net/ont/geosparql#SpatialObject"/>
        <rdfs:range rdf:resource="http://www.opengis.net/ont/geosparql#SpatialObject"/>
        <dc:contributor>Matthew Perry</dc:contributor>
        <dc:creator>OGC GeoSPARQL 1.0 Standard Working Group</dc:creator>
        <dc:date rdf:datatype="http://www.w3.org/2001/XMLSchema#date">2011-06-16</dc:date>
        <dc:description xml:lang="en">
      Exists if the subject SpatialObject is spatially within the 
      object SpatialObject. DE-9IM: T*F**F***
    </dc:description>
        <rdfs:comment xml:lang="en">
      Exists if the subject SpatialObject is spatially within the 
      object SpatialObject. DE-9IM: T*F**F***
    </rdfs:comment>
        <rdfs:isDefinedBy rdf:resource="http://www.opengis.net/ont/geosparql"/>
        <rdfs:isDefinedBy rdf:resource="http://www.opengis.net/spec/geosparql/1.0"/>
        <rdfs:label xml:lang="en">within</rdfs:label>
        <skos:definition xml:lang="en">
      Exists if the subject SpatialObject is spatially within the 
      object SpatialObject. DE-9IM: T*F**F***
    </skos:definition>
        <skos:prefLabel xml:lang="en">within</skos:prefLabel>
    </owl:ObjectProperty>
    


    <!-- https://w3id.org/latuli/ontology/m3#belongsToShipment -->


    <owl:ObjectProperty rdf:about="https://w3id.org/latuli/ontology/m3#belongsToShipment">
        <rdfs:subPropertyOf rdf:resource="http://www.w3.org/2002/07/owl#topObjectProperty"/>
        <rdfs:range rdf:resource="https://w3id.org/latuli/ontology/m3#Shipment"/>
        <rdfs:comment>Relates a TradeItem or a ShipmentItem to a Shipment.</rdfs:comment>
    </owl:ObjectProperty>
    


    <!-- https://w3id.org/latuli/ontology/m3#hasCarrierParty -->


    <owl:ObjectProperty rdf:about="https://w3id.org/latuli/ontology/m3#hasCarrierParty">
        <rdfs:subPropertyOf rdf:resource="http://www.w3.org/2002/07/owl#topObjectProperty"/>
        <rdfs:range rdf:resource="https://w3id.org/latuli/ontology/m3#Carrier"/>
        <rdfs:comment>Relates a Consignment or an XDocLoadingUnit (cross-dock loading unit) to a Carrier</rdfs:comment>
    </owl:ObjectProperty>
    


    <!-- https://w3id.org/latuli/ontology/m3#hasConsigneeParty -->


    <owl:ObjectProperty rdf:about="https://w3id.org/latuli/ontology/m3#hasConsigneeParty">
        <rdfs:subPropertyOf rdf:resource="http://www.w3.org/2002/07/owl#topObjectProperty"/>
        <rdfs:range rdf:resource="https://w3id.org/latuli/ontology/m3#Consignee"/>
        <rdfs:comment>Relates a Consignment or an XDocLoadingUnit (cross-dock loading unit) to a Consignee</rdfs:comment>
    </owl:ObjectProperty>
    


    <!-- https://w3id.org/latuli/ontology/m3#hasConsignorParty -->


    <owl:ObjectProperty rdf:about="https://w3id.org/latuli/ontology/m3#hasConsignorParty">
        <rdfs:subPropertyOf rdf:resource="http://www.w3.org/2002/07/owl#topObjectProperty"/>
        <rdfs:range rdf:resource="https://w3id.org/latuli/ontology/m3#Consignor"/>
        <rdfs:comment>Relates a Consignment or an XDocLoadingUnit (cross-dock loading unit) to a Consignor</rdfs:comment>
    </owl:ObjectProperty>
    


    <!-- https://w3id.org/latuli/ontology/m3#hasHubParty -->


    <owl:ObjectProperty rdf:about="https://w3id.org/latuli/ontology/m3#hasHubParty">
        <rdfs:range rdf:resource="https://w3id.org/latuli/ontology/m3#Party"/>
        <rdfs:comment>Relates a HubReconstructionLocation, an XDocLoadingUnit (cross-dock loading unit), a Wave, or a Transport to a TerminalOperator</rdfs:comment>
    </owl:ObjectProperty>
    


    <!-- https://w3id.org/latuli/ontology/m3#hasHubReconstructionLocation -->


    <owl:ObjectProperty rdf:about="https://w3id.org/latuli/ontology/m3#hasHubReconstructionLocation">
        <rdfs:range rdf:resource="https://w3id.org/latuli/ontology/m3#HubReconstructionLocation"/>
        <rdfs:comment>Relates an XDocLoadingUnit (cross-dock loading unit) to an HubReconstructionLocation</rdfs:comment>
    </owl:ObjectProperty>
    


    <!-- https://w3id.org/latuli/ontology/m3#hasHubReconstructionParty -->


    <owl:ObjectProperty rdf:about="https://w3id.org/latuli/ontology/m3#hasHubReconstructionParty">
        <rdfs:subPropertyOf rdf:resource="http://www.w3.org/2002/07/owl#topObjectProperty"/>
        <rdfs:range rdf:resource="https://w3id.org/latuli/ontology/m3#Party"/>
    </owl:ObjectProperty>
    


    <!-- https://w3id.org/latuli/ontology/m3#hasInboundConsignment -->


    <owl:ObjectProperty rdf:about="https://w3id.org/latuli/ontology/m3#hasInboundConsignment">
        <rdfs:subPropertyOf rdf:resource="http://www.w3.org/2002/07/owl#topObjectProperty"/>
        <rdfs:range rdf:resource="https://w3id.org/latuli/ontology/m3#Consignment"/>
        <rdfs:comment>Relates an XDocLoadingUnit (cross-dock loading unit) to an inbound Consignment</rdfs:comment>
    </owl:ObjectProperty>
    


    <!-- https://w3id.org/latuli/ontology/m3#hasInboundParentLoadingUnit -->


    <owl:ObjectProperty rdf:about="https://w3id.org/latuli/ontology/m3#hasInboundParentLoadingUnit">
        <rdfs:subPropertyOf rdf:resource="http://www.w3.org/2002/07/owl#topObjectProperty"/>
        <rdfs:range rdf:resource="https://w3id.org/latuli/ontology/m3#LoadingUnit"/>
        <rdfs:comment>Relates an XDocLoadingUnit (cross-dock loading unit) to an inbound parent LoadingUnit</rdfs:comment>
    </owl:ObjectProperty>
    


    <!-- https://w3id.org/latuli/ontology/m3#hasLoadingUnit -->


    <owl:ObjectProperty rdf:about="https://w3id.org/latuli/ontology/m3#hasLoadingUnit">
        <rdfs:subPropertyOf rdf:resource="http://www.w3.org/2002/07/owl#topObjectProperty"/>
        <rdfs:range rdf:resource="https://w3id.org/latuli/ontology/m3#LoadingUnit"/>
        <rdfs:comment>Relates an XDocLoadingUnit (cross-dock loading unit), a TradeItem, a ShipmentItem or a DGR (dangerous goods) to a LoadingUnit</rdfs:comment>
    </owl:ObjectProperty>
    


    <!-- https://w3id.org/latuli/ontology/m3#hasOutboundConsignment -->


    <owl:ObjectProperty rdf:about="https://w3id.org/latuli/ontology/m3#hasOutboundConsignment">
        <rdfs:subPropertyOf rdf:resource="http://www.w3.org/2002/07/owl#topObjectProperty"/>
        <rdfs:range rdf:resource="https://w3id.org/latuli/ontology/m3#Consignment"/>
        <rdfs:comment>Relates an XDocLoadingUnit (cross-dock loading unit) to an outbound Consignment</rdfs:comment>
    </owl:ObjectProperty>
    


    <!-- https://w3id.org/latuli/ontology/m3#hasOutboundParentLoadingUnit -->


    <owl:ObjectProperty rdf:about="https://w3id.org/latuli/ontology/m3#hasOutboundParentLoadingUnit">
        <rdfs:subPropertyOf rdf:resource="http://www.w3.org/2002/07/owl#topObjectProperty"/>
        <rdfs:range rdf:resource="https://w3id.org/latuli/ontology/m3#LoadingUnit"/>
        <rdfs:comment>Relates an XDocLoadingUnit (cross-dock loading unit) to an outbound parent LoadingUnit</rdfs:comment>
    </owl:ObjectProperty>
    


    <!-- https://w3id.org/latuli/ontology/m3#hasParty -->


    <owl:ObjectProperty rdf:about="https://w3id.org/latuli/ontology/m3#hasParty">
        <rdfs:subPropertyOf rdf:resource="http://www.w3.org/2002/07/owl#topObjectProperty"/>
        <rdfs:range rdf:resource="https://w3id.org/latuli/ontology/m3#Party"/>
    </owl:ObjectProperty>
    


    <!-- https://w3id.org/latuli/ontology/m3#hasReceiverParty -->


    <owl:ObjectProperty rdf:about="https://w3id.org/latuli/ontology/m3#hasReceiverParty">
        <rdfs:subPropertyOf rdf:resource="http://www.w3.org/2002/07/owl#topObjectProperty"/>
        <rdfs:range rdf:resource="https://w3id.org/latuli/ontology/m3#Receiver"/>
        <rdfs:comment>Relates an XDocLoadingUnit (cross-dock loading unit) or a Shipment to a Receiver.</rdfs:comment>
    </owl:ObjectProperty>
    


    <!-- https://w3id.org/latuli/ontology/m3#hasShipperParty -->


    <owl:ObjectProperty rdf:about="https://w3id.org/latuli/ontology/m3#hasShipperParty">
        <rdfs:subPropertyOf rdf:resource="http://www.w3.org/2002/07/owl#topObjectProperty"/>
        <rdfs:range rdf:resource="https://w3id.org/latuli/ontology/m3#Shipper"/>
        <rdfs:comment>Relates an XDocLoadingUnit (cross-dock loading unit) or a Shipment to a Shipper.</rdfs:comment>
    </owl:ObjectProperty>
    


    <!-- https://w3id.org/latuli/ontology/m3#includesTransport -->


    <owl:ObjectProperty rdf:about="https://w3id.org/latuli/ontology/m3#includesTransport">
        <rdfs:range rdf:resource="https://w3id.org/latuli/ontology/m3#Transport"/>
        <rdfs:comment>Relates a Consignment to a Transport</rdfs:comment>
    </owl:ObjectProperty>
    


    <!-- https://w3id.org/latuli/ontology/m3#processedByWave -->


    <owl:ObjectProperty rdf:about="https://w3id.org/latuli/ontology/m3#processedByWave">
        <rdfs:subPropertyOf rdf:resource="http://www.w3.org/2002/07/owl#topObjectProperty"/>
        <rdfs:range rdf:resource="https://w3id.org/latuli/ontology/m3#Wave"/>
        <rdfs:comment>Relates an XDocLoadingUnit (cross-dock loading unit) or a Consignment to a Wave.</rdfs:comment>
    </owl:ObjectProperty>
    


    <!-- https://w3id.org/latuli/ontology/m3#relatesToTradeItem -->


    <owl:ObjectProperty rdf:about="https://w3id.org/latuli/ontology/m3#relatesToTradeItem">
        <rdfs:subPropertyOf rdf:resource="http://www.w3.org/2002/07/owl#topObjectProperty"/>
        <rdfs:range rdf:resource="https://w3id.org/latuli/ontology/m3#TradeItem"/>
        <rdfs:comment>Relates a DGR (dangerous goods) to a Trade Item.</rdfs:comment>
    </owl:ObjectProperty>
    


    <!-- 
    ///////////////////////////////////////////////////////////////////////////////////////
    //
    // Data properties
    //
    ///////////////////////////////////////////////////////////////////////////////////////
     -->


    


    <!-- http://www.opengis.net/ont/geosparql#asGML -->


    <owl:DatatypeProperty rdf:about="http://www.opengis.net/ont/geosparql#asGML">
        <rdfs:subPropertyOf rdf:resource="http://www.opengis.net/ont/geosparql#hasSerialization"/>
        <rdfs:domain rdf:resource="http://www.opengis.net/ont/geosparql#Geometry"/>
        <rdfs:range rdf:resource="http://www.opengis.net/ont/geosparql#gmlLiteral"/>
        <dc:contributor>Matthew Perry</dc:contributor>
        <dc:creator>OGC GeoSPARQL 1.0 Standard Working Group</dc:creator>
        <dc:date rdf:datatype="http://www.w3.org/2001/XMLSchema#date">2011-06-16</dc:date>
        <dc:description xml:lang="en">
      The GML serialization of a geometry
    </dc:description>
        <rdfs:comment xml:lang="en">
      The GML serialization of a geometry
    </rdfs:comment>
        <rdfs:isDefinedBy rdf:resource="http://www.opengis.net/ont/geosparql"/>
        <rdfs:isDefinedBy rdf:resource="http://www.opengis.net/spec/geosparql/1.0"/>
        <rdfs:label xml:lang="en">asGML</rdfs:label>
        <skos:definition xml:lang="en">
      The GML serialization of a geometry
    </skos:definition>
        <skos:prefLabel xml:lang="en">asGML</skos:prefLabel>
    </owl:DatatypeProperty>
    


    <!-- http://www.opengis.net/ont/geosparql#asWKT -->


    <owl:DatatypeProperty rdf:about="http://www.opengis.net/ont/geosparql#asWKT">
        <rdfs:subPropertyOf rdf:resource="http://www.opengis.net/ont/geosparql#hasSerialization"/>
        <rdfs:domain rdf:resource="http://www.opengis.net/ont/geosparql#Geometry"/>
        <rdfs:range rdf:resource="http://www.opengis.net/ont/geosparql#wktLiteral"/>
        <dc:contributor>Matthew Perry</dc:contributor>
        <dc:creator>OGC GeoSPARQL 1.0 Standard Working Group</dc:creator>
        <dc:date rdf:datatype="http://www.w3.org/2001/XMLSchema#date">2011-06-16</dc:date>
        <dc:description xml:lang="en">
      The WKT serialization of a geometry
    </dc:description>
        <rdfs:comment xml:lang="en">
      The WKT serialization of a geometry
    </rdfs:comment>
        <rdfs:isDefinedBy rdf:resource="http://www.opengis.net/ont/geosparql"/>
        <rdfs:isDefinedBy rdf:resource="http://www.opengis.net/spec/geosparql/1.0"/>
        <rdfs:label xml:lang="en">asWKT</rdfs:label>
        <skos:definition xml:lang="en">
      The WKT serialization of a geometry
    </skos:definition>
        <skos:prefLabel xml:lang="en">asWKT</skos:prefLabel>
    </owl:DatatypeProperty>
    


    <!-- http://www.opengis.net/ont/geosparql#coordinateDimension -->


    <owl:DatatypeProperty rdf:about="http://www.opengis.net/ont/geosparql#coordinateDimension">
        <rdfs:domain rdf:resource="http://www.opengis.net/ont/geosparql#Geometry"/>
        <rdfs:range rdf:resource="http://www.w3.org/2001/XMLSchema#integer"/>
        <dc:contributor>Matthew Perry</dc:contributor>
        <dc:creator>OGC GeoSPARQL 1.0 Standard Working Group</dc:creator>
        <dc:date rdf:datatype="http://www.w3.org/2001/XMLSchema#date">2011-06-16</dc:date>
        <dc:description xml:lang="en">
      The number of measurements or axes needed to describe the position of this
      geometry in a coordinate system.
    </dc:description>
        <rdfs:comment xml:lang="en">
      The number of measurements or axes needed to describe the position of this
      geometry in a coordinate system.
    </rdfs:comment>
        <rdfs:isDefinedBy rdf:resource="http://www.opengis.net/ont/geosparql"/>
        <rdfs:isDefinedBy rdf:resource="http://www.opengis.net/spec/geosparql/1.0"/>
        <rdfs:label xml:lang="en">coordinateDimension</rdfs:label>
        <skos:definition xml:lang="en">
      The number of measurements or axes needed to describe the position of this
      geometry in a coordinate system.
    </skos:definition>
        <skos:prefLabel xml:lang="en">coordinateDimension</skos:prefLabel>
    </owl:DatatypeProperty>
    


    <!-- http://www.opengis.net/ont/geosparql#dimension -->


    <owl:DatatypeProperty rdf:about="http://www.opengis.net/ont/geosparql#dimension">
        <rdfs:domain rdf:resource="http://www.opengis.net/ont/geosparql#Geometry"/>
        <rdfs:range rdf:resource="http://www.w3.org/2001/XMLSchema#integer"/>
        <dc:contributor>Matthew Perry</dc:contributor>
        <dc:creator>OGC GeoSPARQL 1.0 Standard Working Group</dc:creator>
        <dc:date rdf:datatype="http://www.w3.org/2001/XMLSchema#date">2011-06-16</dc:date>
        <dc:description xml:lang="en">
      The topological dimension of this geometric object, which 
      must be less than or equal to the coordinate dimension. 
      In non-homogeneous collections, this will return the largest 
      topological dimension of the contained objects.
    </dc:description>
        <rdfs:comment xml:lang="en">
      The topological dimension of this geometric object, which 
      must be less than or equal to the coordinate dimension. 
      In non-homogeneous collections, this will return the largest 
      topological dimension of the contained objects.
    </rdfs:comment>
        <rdfs:isDefinedBy rdf:resource="http://www.opengis.net/ont/geosparql"/>
        <rdfs:isDefinedBy rdf:resource="http://www.opengis.net/spec/geosparql/1.0"/>
        <rdfs:label xml:lang="en">dimension</rdfs:label>
        <skos:definition xml:lang="en">
      The topological dimension of this geometric object, which 
      must be less than or equal to the coordinate dimension. 
      In non-homogeneous collections, this will return the largest 
      topological dimension of the contained objects.
    </skos:definition>
        <skos:prefLabel xml:lang="en">dimension</skos:prefLabel>
    </owl:DatatypeProperty>
    


    <!-- http://www.opengis.net/ont/geosparql#hasSerialization -->


    <owl:DatatypeProperty rdf:about="http://www.opengis.net/ont/geosparql#hasSerialization">
        <rdfs:domain rdf:resource="http://www.opengis.net/ont/geosparql#Geometry"/>
        <rdfs:range rdf:resource="http://www.w3.org/2000/01/rdf-schema#Literal"/>
        <dc:contributor>Matthew Perry</dc:contributor>
        <dc:creator>OGC GeoSPARQL 1.0 Standard Working Group</dc:creator>
        <dc:date rdf:datatype="http://www.w3.org/2001/XMLSchema#date">2011-06-16</dc:date>
        <dc:description xml:lang="en">
      Connects a geometry object with its text-based serialization.
    </dc:description>
        <rdfs:comment xml:lang="en">
      Connects a geometry object with its text-based serialization.
    </rdfs:comment>
        <rdfs:isDefinedBy rdf:resource="http://www.opengis.net/ont/geosparql"/>
        <rdfs:isDefinedBy rdf:resource="http://www.opengis.net/spec/geosparql/1.0"/>
        <rdfs:label xml:lang="en">has serialization</rdfs:label>
        <skos:definition xml:lang="en">
      Connects a geometry object with its text-based serialization.
    </skos:definition>
        <skos:prefLabel xml:lang="en">has serialization</skos:prefLabel>
    </owl:DatatypeProperty>
    


    <!-- http://www.opengis.net/ont/geosparql#isEmpty -->


    <owl:DatatypeProperty rdf:about="http://www.opengis.net/ont/geosparql#isEmpty">
        <rdfs:domain rdf:resource="http://www.opengis.net/ont/geosparql#Geometry"/>
        <rdfs:range rdf:resource="http://www.w3.org/2001/XMLSchema#boolean"/>
        <dc:contributor>Matthew Perry</dc:contributor>
        <dc:creator>OGC GeoSPARQL 1.0 Standard Working Group</dc:creator>
        <dc:date rdf:datatype="http://www.w3.org/2001/XMLSchema#date">2011-06-16</dc:date>
        <dc:description xml:lang="en">
      (true) if this geometric object is the empty Geometry. If 
      true, then this geometric object represents the empty point 
      set for the coordinate space.
    </dc:description>
        <rdfs:comment xml:lang="en">
      (true) if this geometric object is the empty Geometry. If 
      true, then this geometric object represents the empty point 
      set for the coordinate space.
    </rdfs:comment>
        <rdfs:isDefinedBy rdf:resource="http://www.opengis.net/ont/geosparql"/>
        <rdfs:isDefinedBy rdf:resource="http://www.opengis.net/spec/geosparql/1.0"/>
        <rdfs:label xml:lang="en">isEmpty</rdfs:label>
        <skos:definition xml:lang="en">
      (true) if this geometric object is the empty Geometry. If 
      true, then this geometric object represents the empty point 
      set for the coordinate space.
    </skos:definition>
        <skos:prefLabel xml:lang="en">isEmpty</skos:prefLabel>
    </owl:DatatypeProperty>
    


    <!-- http://www.opengis.net/ont/geosparql#isSimple -->


    <owl:DatatypeProperty rdf:about="http://www.opengis.net/ont/geosparql#isSimple">
        <rdfs:domain rdf:resource="http://www.opengis.net/ont/geosparql#Geometry"/>
        <rdfs:range rdf:resource="http://www.w3.org/2001/XMLSchema#boolean"/>
        <dc:contributor>Matthew Perry</dc:contributor>
        <dc:creator>OGC GeoSPARQL 1.0 Standard Working Group</dc:creator>
        <dc:date rdf:datatype="http://www.w3.org/2001/XMLSchema#date">2011-06-16</dc:date>
        <dc:description xml:lang="en">
      (true) if this geometric object has no anomalous geometric 
      points, such as self intersection or self tangency.
    </dc:description>
        <rdfs:comment xml:lang="en">
      (true) if this geometric object has no anomalous geometric 
      points, such as self intersection or self tangency.
    </rdfs:comment>
        <rdfs:isDefinedBy rdf:resource="http://www.opengis.net/ont/geosparql"/>
        <rdfs:isDefinedBy rdf:resource="http://www.opengis.net/spec/geosparql/1.0"/>
        <rdfs:label xml:lang="en">isSimple</rdfs:label>
        <skos:definition xml:lang="en">
      (true) if this geometric object has no anomalous geometric 
      points, such as self intersection or self tangency.
    </skos:definition>
        <skos:prefLabel xml:lang="en">isSimple</skos:prefLabel>
    </owl:DatatypeProperty>
    


    <!-- http://www.opengis.net/ont/geosparql#spatialDimension -->


    <owl:DatatypeProperty rdf:about="http://www.opengis.net/ont/geosparql#spatialDimension">
        <rdfs:domain rdf:resource="http://www.opengis.net/ont/geosparql#Geometry"/>
        <rdfs:range rdf:resource="http://www.w3.org/2001/XMLSchema#integer"/>
        <dc:contributor>Matthew Perry</dc:contributor>
        <dc:creator>OGC GeoSPARQL 1.0 Standard Working Group</dc:creator>
        <dc:date rdf:datatype="http://www.w3.org/2001/XMLSchema#date">2011-06-16</dc:date>
        <dc:description xml:lang="en">
      The number of measurements or axes needed to describe the spatial position of 
      this geometry in a coordinate system.
    </dc:description>
        <rdfs:comment xml:lang="en">
      The number of measurements or axes needed to describe the spatial position of 
      this geometry in a coordinate system.
    </rdfs:comment>
        <rdfs:isDefinedBy rdf:resource="http://www.opengis.net/ont/geosparql"/>
        <rdfs:isDefinedBy rdf:resource="http://www.opengis.net/spec/geosparql/1.0"/>
        <rdfs:label xml:lang="en">spatialDimension</rdfs:label>
        <skos:definition xml:lang="en">
      The number of measurements or axes needed to describe the spatial position of 
      this geometry in a coordinate system.
    </skos:definition>
        <skos:prefLabel xml:lang="en">spatialDimension</skos:prefLabel>
    </owl:DatatypeProperty>
    


    <!-- https://w3id.org/latuli/ontology/m3#additionalPartyIdentification -->


    <owl:DatatypeProperty rdf:about="https://w3id.org/latuli/ontology/m3#additionalPartyIdentification">
        <rdfs:range rdf:resource="http://www.w3.org/2001/XMLSchema#string"/>
        <rdfs:comment>Identifies a party using a custom identification scheme.</rdfs:comment>
    </owl:DatatypeProperty>
    


    <!-- https://w3id.org/latuli/ontology/m3#asWKT -->


    <owl:DatatypeProperty rdf:about="https://w3id.org/latuli/ontology/m3#asWKT">
        <rdfs:subPropertyOf rdf:resource="http://www.w3.org/2002/07/owl#topDataProperty"/>
        <rdfs:domain rdf:resource="https://w3id.org/latuli/ontology/m3#Party"/>
        <rdfs:range rdf:resource="http://www.opengis.net/ont/geosparql#wktLiteral"/>
    </owl:DatatypeProperty>
    


    <!-- https://w3id.org/latuli/ontology/m3#carrierHashCode -->


    <owl:DatatypeProperty rdf:about="https://w3id.org/latuli/ontology/m3#carrierHashCode">
        <rdfs:range rdf:resource="http://www.w3.org/2001/XMLSchema#string"/>
        <rdfs:comment>A hashcode which represents a carrier party using a numeric value</rdfs:comment>
    </owl:DatatypeProperty>
    


    <!-- https://w3id.org/latuli/ontology/m3#closedOn -->


    <owl:DatatypeProperty rdf:about="https://w3id.org/latuli/ontology/m3#closedOn">
        <rdfs:subPropertyOf rdf:resource="http://www.w3.org/2002/07/owl#topDataProperty"/>
        <rdfs:range rdf:resource="http://www.w3.org/2001/XMLSchema#dateTime"/>
        <rdfs:comment>Timestamp for when a wave is closed.</rdfs:comment>
    </owl:DatatypeProperty>
    


    <!-- https://w3id.org/latuli/ontology/m3#code2 -->


    <owl:DatatypeProperty rdf:about="https://w3id.org/latuli/ontology/m3#code2">
        <rdfs:subPropertyOf rdf:resource="http://www.w3.org/2002/07/owl#topDataProperty"/>
        <rdfs:domain rdf:resource="https://w3id.org/latuli/ontology/m3#Party"/>
        <rdfs:range rdf:resource="http://www.w3.org/2001/XMLSchema#string"/>
        <rdfs:comment>Two-digit identifier for describing a country.</rdfs:comment>
    </owl:DatatypeProperty>
    


    <!-- https://w3id.org/latuli/ontology/m3#consigneeHashCode -->


    <owl:DatatypeProperty rdf:about="https://w3id.org/latuli/ontology/m3#consigneeHashCode">
        <rdfs:range rdf:resource="http://www.w3.org/2001/XMLSchema#string"/>
        <rdfs:comment>A hashcode which represents a consignee party using a numeric value</rdfs:comment>
    </owl:DatatypeProperty>
    


    <!-- https://w3id.org/latuli/ontology/m3#consignmentId -->


    <owl:DatatypeProperty rdf:about="https://w3id.org/latuli/ontology/m3#consignmentId">
        <rdfs:subPropertyOf rdf:resource="http://www.w3.org/2002/07/owl#topDataProperty"/>
        <rdfs:range rdf:resource="http://www.w3.org/2001/XMLSchema#string"/>
        <rdfs:comment>An unique identifier for a consignment.</rdfs:comment>
    </owl:DatatypeProperty>
    


    <!-- https://w3id.org/latuli/ontology/m3#consignmentType -->


    <owl:DatatypeProperty rdf:about="https://w3id.org/latuli/ontology/m3#consignmentType">
        <rdfs:subPropertyOf rdf:resource="http://www.w3.org/2002/07/owl#topDataProperty"/>
        <rdfs:range rdf:resource="http://www.w3.org/2001/XMLSchema#string"/>
        <rdfs:comment>Describes whether a consignment is inbound or outbound</rdfs:comment>
    </owl:DatatypeProperty>
    


    <!-- https://w3id.org/latuli/ontology/m3#consignorHashCode -->


    <owl:DatatypeProperty rdf:about="https://w3id.org/latuli/ontology/m3#consignorHashCode">
        <rdfs:range rdf:resource="http://www.w3.org/2001/XMLSchema#string"/>
        <rdfs:comment>A hashcode which represents a consignor  party using a numeric value</rdfs:comment>
    </owl:DatatypeProperty>
    


    <!-- https://w3id.org/latuli/ontology/m3#createdOn -->


    <owl:DatatypeProperty rdf:about="https://w3id.org/latuli/ontology/m3#createdOn">
        <rdfs:range rdf:resource="http://www.w3.org/2001/XMLSchema#dateTime"/>
        <rdfs:comment>A hashcode which represents a consignor  party using a numeric value</rdfs:comment>
    </owl:DatatypeProperty>
    


    <!-- https://w3id.org/latuli/ontology/m3#customerProductDescription -->


    <owl:DatatypeProperty rdf:about="https://w3id.org/latuli/ontology/m3#customerProductDescription">
        <rdfs:subPropertyOf rdf:resource="http://www.w3.org/2002/07/owl#topDataProperty"/>
        <rdfs:range rdf:resource="http://www.w3.org/2001/XMLSchema#string"/>
        <rdfs:comment>A description of a trade item by the customer.</rdfs:comment>
    </owl:DatatypeProperty>
    


    <!-- https://w3id.org/latuli/ontology/m3#customerProductId -->


    <owl:DatatypeProperty rdf:about="https://w3id.org/latuli/ontology/m3#customerProductId">
        <rdfs:subPropertyOf rdf:resource="http://www.w3.org/2002/07/owl#topDataProperty"/>
        <rdfs:range rdf:resource="http://www.w3.org/2001/XMLSchema#string"/>
        <rdfs:comment>The identifier of a trade item used by the customer</rdfs:comment>
    </owl:DatatypeProperty>
    


    <!-- https://w3id.org/latuli/ontology/m3#customerQuantity -->


    <owl:DatatypeProperty rdf:about="https://w3id.org/latuli/ontology/m3#customerQuantity">
        <rdfs:subPropertyOf rdf:resource="http://www.w3.org/2002/07/owl#topDataProperty"/>
        <rdfs:range rdf:resource="http://www.w3.org/2001/XMLSchema#decimal"/>
        <rdfs:comment>The quantity of trade items expected by the customer.</rdfs:comment>
    </owl:DatatypeProperty>
    


    <!-- https://w3id.org/latuli/ontology/m3#description -->


    <owl:DatatypeProperty rdf:about="https://w3id.org/latuli/ontology/m3#description">
        <rdfs:subPropertyOf rdf:resource="http://www.w3.org/2002/07/owl#topDataProperty"/>
        <rdfs:range rdf:resource="http://www.w3.org/2001/XMLSchema#string"/>
        <rdfs:comment>A description of a trade item.</rdfs:comment>
    </owl:DatatypeProperty>
    


    <!-- https://w3id.org/latuli/ontology/m3#effectiveArrival -->


    <owl:DatatypeProperty rdf:about="https://w3id.org/latuli/ontology/m3#effectiveArrival">
        <rdfs:range rdf:resource="http://www.w3.org/2001/XMLSchema#dateTime"/>
        <rdfs:comment>Timestamp for when a transport means actually arrived at an hub.</rdfs:comment>
    </owl:DatatypeProperty>
    


    <!-- https://w3id.org/latuli/ontology/m3#expectedArrival -->


    <owl:DatatypeProperty rdf:about="https://w3id.org/latuli/ontology/m3#expectedArrival">
        <rdfs:range rdf:resource="http://www.w3.org/2001/XMLSchema#dateTime"/>
        <rdfs:comment>Timestamp for when a transport means is expected to arrive at an hub.</rdfs:comment>
    </owl:DatatypeProperty>
    


    <!-- https://w3id.org/latuli/ontology/m3#expectedDeliveryOn -->


    <owl:DatatypeProperty rdf:about="https://w3id.org/latuli/ontology/m3#expectedDeliveryOn">
        <rdfs:subPropertyOf rdf:resource="http://www.w3.org/2002/07/owl#topDataProperty"/>
        <rdfs:domain rdf:resource="https://w3id.org/latuli/ontology/m3#Shipment"/>
        <rdfs:range rdf:resource="http://www.w3.org/2001/XMLSchema#dateTime"/>
        <rdfs:comment>Timestamp for when a shipment is expected to be delivered to a receiver.</rdfs:comment>
        <skos:prefLabel xml:lang="nb">expectedDeliveryOn</skos:prefLabel>
    </owl:DatatypeProperty>
    


    <!-- https://w3id.org/latuli/ontology/m3#finishedScanOn -->


    <owl:DatatypeProperty rdf:about="https://w3id.org/latuli/ontology/m3#finishedScanOn">
        <rdfs:range rdf:resource="http://www.w3.org/2001/XMLSchema#dateTime"/>
        <rdfs:comment>Timestamp for when a xDocLoadingUnit (cross dock loading unit) has been scanned.</rdfs:comment>
    </owl:DatatypeProperty>
    


    <!-- https://w3id.org/latuli/ontology/m3#fullPalletConsignment -->


    <owl:DatatypeProperty rdf:about="https://w3id.org/latuli/ontology/m3#fullPalletConsignment">
        <rdfs:subPropertyOf rdf:resource="http://www.w3.org/2002/07/owl#topDataProperty"/>
        <rdfs:range rdf:resource="http://www.w3.org/2001/XMLSchema#string"/>
        <rdfs:comment>Describes whether a consignment consist of full pallets (1) or not (0)</rdfs:comment>
    </owl:DatatypeProperty>
    


    <!-- https://w3id.org/latuli/ontology/m3#gln -->


    <owl:DatatypeProperty rdf:about="https://w3id.org/latuli/ontology/m3#gln">
        <rdfs:subPropertyOf rdf:resource="http://www.w3.org/2002/07/owl#topDataProperty"/>
        <rdfs:range rdf:resource="http://www.w3.org/2001/XMLSchema#string"/>
        <rdfs:comment>GLN is the GS1 Identification Key used to identify physical locations or parties. The key comprises a GS1 Company Prefix, Location Reference, and Check Digit</rdfs:comment>
    </owl:DatatypeProperty>
    


    <!-- https://w3id.org/latuli/ontology/m3#gtin -->


    <owl:DatatypeProperty rdf:about="https://w3id.org/latuli/ontology/m3#gtin">
        <rdfs:range rdf:resource="http://www.w3.org/2001/XMLSchema#string"/>
        <rdfs:comment>GTIN is the GS1 Identification Key used to identify trade items. The key comprises a GS1 Company Prefix, an Item Reference and Check Digit.</rdfs:comment>
    </owl:DatatypeProperty>
    


    <!-- https://w3id.org/latuli/ontology/m3#handlingInstruction -->


    <owl:DatatypeProperty rdf:about="https://w3id.org/latuli/ontology/m3#handlingInstruction">
        <rdfs:subPropertyOf rdf:resource="http://www.w3.org/2002/07/owl#topDataProperty"/>
        <rdfs:range rdf:resource="http://www.w3.org/2001/XMLSchema#string"/>
        <rdfs:comment>Instructions that describe how goods should be expedited during transport and other goods handling.</rdfs:comment>
    </owl:DatatypeProperty>
    


    <!-- https://w3id.org/latuli/ontology/m3#hashCode -->


    <owl:DatatypeProperty rdf:about="https://w3id.org/latuli/ontology/m3#hashCode">
        <rdfs:subPropertyOf rdf:resource="http://www.w3.org/2002/07/owl#topDataProperty"/>
        <rdfs:range rdf:resource="http://www.w3.org/2001/XMLSchema#string"/>
        <rdfs:comment>A hashcode which represents a hub party using a numeric value</rdfs:comment>
    </owl:DatatypeProperty>
    


    <!-- https://w3id.org/latuli/ontology/m3#hubAdditionalPartyIdentification -->


    <owl:DatatypeProperty rdf:about="https://w3id.org/latuli/ontology/m3#hubAdditionalPartyIdentification">
        <rdfs:subPropertyOf rdf:resource="http://www.w3.org/2002/07/owl#topDataProperty"/>
        <rdfs:range rdf:resource="http://www.w3.org/2001/XMLSchema#string"/>
        <rdfs:comment>Identifies a hub party using a custom identification scheme.</rdfs:comment>
    </owl:DatatypeProperty>
    


    <!-- https://w3id.org/latuli/ontology/m3#hubHashCode -->


    <owl:DatatypeProperty rdf:about="https://w3id.org/latuli/ontology/m3#hubHashCode">
        <rdfs:range rdf:resource="http://www.w3.org/2001/XMLSchema#string"/>
        <rdfs:comment>A hashcode which represents a hub party using a numeric value</rdfs:comment>
    </owl:DatatypeProperty>
    


    <!-- https://w3id.org/latuli/ontology/m3#hubReconstructionHashCode -->


    <owl:DatatypeProperty rdf:about="https://w3id.org/latuli/ontology/m3#hubReconstructionHashCode">
        <rdfs:range rdf:resource="http://www.w3.org/2001/XMLSchema#string"/>
        <rdfs:comment>A hashcode which represents a hub reconstruction location using a numeric value</rdfs:comment>
    </owl:DatatypeProperty>
    


    <!-- https://w3id.org/latuli/ontology/m3#hubReconstructionLocationId -->


    <owl:DatatypeProperty rdf:about="https://w3id.org/latuli/ontology/m3#hubReconstructionLocationId">
        <rdfs:range rdf:resource="http://www.w3.org/2001/XMLSchema#string"/>
        <rdfs:comment>A unique identifier for a hub reconstruction location</rdfs:comment>
    </owl:DatatypeProperty>
    


    <!-- https://w3id.org/latuli/ontology/m3#internalId -->


    <owl:DatatypeProperty rdf:about="https://w3id.org/latuli/ontology/m3#internalId">
        <rdfs:range rdf:resource="http://www.w3.org/2001/XMLSchema#string"/>
        <rdfs:comment>A unique identifier for an xDocLoadingUnit (cross-dock loading unit)</rdfs:comment>
    </owl:DatatypeProperty>
    


    <!-- https://w3id.org/latuli/ontology/m3#isCarrier -->


    <owl:DatatypeProperty rdf:about="https://w3id.org/latuli/ontology/m3#isCarrier">
        <rdfs:range rdf:resource="http://www.w3.org/2001/XMLSchema#boolean"/>
        <rdfs:comment>A flag that defines whether a party is a carrier (1) or not (0)</rdfs:comment>
    </owl:DatatypeProperty>
    


    <!-- https://w3id.org/latuli/ontology/m3#isConsignor -->


    <owl:DatatypeProperty rdf:about="https://w3id.org/latuli/ontology/m3#isConsignor">
        <rdfs:range rdf:resource="http://www.w3.org/2001/XMLSchema#boolean"/>
        <rdfs:comment>A flag that defines whether a party is a consignor (1) or not (0)</rdfs:comment>
    </owl:DatatypeProperty>
    


    <!-- https://w3id.org/latuli/ontology/m3#isHub -->


    <owl:DatatypeProperty rdf:about="https://w3id.org/latuli/ontology/m3#isHub">
        <rdfs:range rdf:resource="http://www.w3.org/2001/XMLSchema#boolean"/>
        <rdfs:comment>A flag that defines whether a party is a hub (1) or not (0)</rdfs:comment>
    </owl:DatatypeProperty>
    


    <!-- https://w3id.org/latuli/ontology/m3#isShipper -->


    <owl:DatatypeProperty rdf:about="https://w3id.org/latuli/ontology/m3#isShipper">
        <rdfs:range rdf:resource="http://www.w3.org/2001/XMLSchema#boolean"/>
        <rdfs:comment>A flag that defines whether a party is a shipper (1) or not (0)</rdfs:comment>
    </owl:DatatypeProperty>
    


    <!-- https://w3id.org/latuli/ontology/m3#location -->


    <owl:DatatypeProperty rdf:about="https://w3id.org/latuli/ontology/m3#location">
        <rdfs:subPropertyOf rdf:resource="http://www.w3.org/2002/07/owl#topDataProperty"/>
        <rdfs:domain rdf:resource="https://w3id.org/latuli/ontology/m3#Party"/>
        <rdfs:range rdf:resource="http://www.w3.org/2001/XMLSchema#string"/>
        <rdfs:comment>The name of the city associated with a party</rdfs:comment>
    </owl:DatatypeProperty>
    


    <!-- https://w3id.org/latuli/ontology/m3#lotNumber -->


    <owl:DatatypeProperty rdf:about="https://w3id.org/latuli/ontology/m3#lotNumber">
        <rdfs:subPropertyOf rdf:resource="http://www.w3.org/2002/07/owl#topDataProperty"/>
        <rdfs:range rdf:resource="http://www.w3.org/2001/XMLSchema#string"/>
        <rdfs:comment>A lot number is an identification number assigned to a particular quantity or lot of material from a single manufacturer</rdfs:comment>
    </owl:DatatypeProperty>
    


    <!-- https://w3id.org/latuli/ontology/m3#material -->


    <owl:DatatypeProperty rdf:about="https://w3id.org/latuli/ontology/m3#material">
        <rdfs:subPropertyOf rdf:resource="http://www.w3.org/2002/07/owl#topDataProperty"/>
        <rdfs:range rdf:resource="http://www.w3.org/2001/XMLSchema#string"/>
        <rdfs:comment>Describes the material used in a trade item</rdfs:comment>
    </owl:DatatypeProperty>
    


    <!-- https://w3id.org/latuli/ontology/m3#modifiedOn -->


    <owl:DatatypeProperty rdf:about="https://w3id.org/latuli/ontology/m3#modifiedOn">
        <rdfs:subPropertyOf rdf:resource="http://www.w3.org/2002/07/owl#topDataProperty"/>
        <rdfs:range rdf:resource="http://www.w3.org/2001/XMLSchema#dateTime"/>
        <rdfs:comment>Timestamp for when an entry in the database is modified.</rdfs:comment>
    </owl:DatatypeProperty>
    


    <!-- https://w3id.org/latuli/ontology/m3#orderNumber -->


    <owl:DatatypeProperty rdf:about="https://w3id.org/latuli/ontology/m3#orderNumber">
        <rdfs:range rdf:resource="http://www.w3.org/2001/XMLSchema#string"/>
        <rdfs:comment>A reference to the order number when describing a loading unit.</rdfs:comment>
    </owl:DatatypeProperty>
    


    <!-- https://w3id.org/latuli/ontology/m3#packageTypeId -->


    <owl:DatatypeProperty rdf:about="https://w3id.org/latuli/ontology/m3#packageTypeId">
        <rdfs:subPropertyOf rdf:resource="http://www.w3.org/2002/07/owl#topDataProperty"/>
        <rdfs:domain rdf:resource="https://w3id.org/latuli/ontology/m3#LoadingUnit"/>
        <rdfs:range rdf:resource="http://www.w3.org/2001/XMLSchema#string"/>
        <rdfs:comment>Describes what type of packaging type the loading unit consists of. Examples are BX (box) and PX (pallet).</rdfs:comment>
    </owl:DatatypeProperty>
    


    <!-- https://w3id.org/latuli/ontology/m3#plannedDeliveryDate -->


    <owl:DatatypeProperty rdf:about="https://w3id.org/latuli/ontology/m3#plannedDeliveryDate">
        <rdfs:subPropertyOf rdf:resource="http://www.w3.org/2002/07/owl#topDataProperty"/>
        <rdfs:domain rdf:resource="https://w3id.org/latuli/ontology/m3#Shipment"/>
        <rdfs:range rdf:resource="http://www.w3.org/2001/XMLSchema#dateTime"/>
        <rdfs:comment>Timestamp for when a shipment is planned to be delivered to the receiver.</rdfs:comment>
    </owl:DatatypeProperty>
    


    <!-- https://w3id.org/latuli/ontology/m3#plannedOn -->


    <owl:DatatypeProperty rdf:about="https://w3id.org/latuli/ontology/m3#plannedOn">
        <rdfs:range rdf:resource="http://www.w3.org/2001/XMLSchema#dateTime"/>
        <rdfs:comment>Timestamp for when a wave has been planned.</rdfs:comment>
    </owl:DatatypeProperty>
    


    <!-- https://w3id.org/latuli/ontology/m3#postalCode -->


    <owl:DatatypeProperty rdf:about="https://w3id.org/latuli/ontology/m3#postalCode">
        <rdfs:subPropertyOf rdf:resource="http://www.w3.org/2002/07/owl#topDataProperty"/>
        <rdfs:domain rdf:resource="https://w3id.org/latuli/ontology/m3#Party"/>
        <rdfs:range rdf:resource="http://www.w3.org/2001/XMLSchema#string"/>
        <rdfs:comment>Describes the postal code associated with a party.</rdfs:comment>
    </owl:DatatypeProperty>
    


    <!-- https://w3id.org/latuli/ontology/m3#preSortScanOn -->


    <owl:DatatypeProperty rdf:about="https://w3id.org/latuli/ontology/m3#preSortScanOn">
        <rdfs:subPropertyOf rdf:resource="http://www.w3.org/2002/07/owl#topDataProperty"/>
        <rdfs:domain rdf:resource="https://w3id.org/latuli/ontology/m3#XDocLoadingUnit"/>
        <rdfs:range rdf:resource="http://www.w3.org/2001/XMLSchema#dateTime"/>
        <rdfs:comment>Timestamp for when an XDocLoadingUnit (cross-dock loading unit) has been presorted.</rdfs:comment>
    </owl:DatatypeProperty>
    


    <!-- https://w3id.org/latuli/ontology/m3#purchaseOrder -->


    <owl:DatatypeProperty rdf:about="https://w3id.org/latuli/ontology/m3#purchaseOrder">
        <rdfs:subPropertyOf rdf:resource="http://www.w3.org/2002/07/owl#topDataProperty"/>
        <rdfs:range rdf:resource="http://www.w3.org/2001/XMLSchema#string"/>
        <rdfs:comment>A reference to a purchase order associated with a trade item</rdfs:comment>
    </owl:DatatypeProperty>
    


    <!-- https://w3id.org/latuli/ontology/m3#qttBoxes -->


    <owl:DatatypeProperty rdf:about="https://w3id.org/latuli/ontology/m3#qttBoxes">
        <rdfs:subPropertyOf rdf:resource="http://www.w3.org/2002/07/owl#topDataProperty"/>
        <rdfs:domain rdf:resource="https://w3id.org/latuli/ontology/m3#Consignment"/>
        <rdfs:range rdf:resource="http://www.w3.org/2001/XMLSchema#int"/>
        <rdfs:comment>The quantity of boxes in a consignment, a shipment or in a wave</rdfs:comment>
    </owl:DatatypeProperty>
    


    <!-- https://w3id.org/latuli/ontology/m3#qttBoxesProcessed -->


    <owl:DatatypeProperty rdf:about="https://w3id.org/latuli/ontology/m3#qttBoxesProcessed">
        <rdfs:subPropertyOf rdf:resource="http://www.w3.org/2002/07/owl#topDataProperty"/>
        <rdfs:range rdf:resource="http://www.w3.org/2001/XMLSchema#int"/>
        <rdfs:comment>The quantity of boxes processed in a wave</rdfs:comment>
    </owl:DatatypeProperty>
    


    <!-- https://w3id.org/latuli/ontology/m3#qttPallets -->


    <owl:DatatypeProperty rdf:about="https://w3id.org/latuli/ontology/m3#qttPallets">
        <rdfs:subPropertyOf rdf:resource="http://www.w3.org/2002/07/owl#topDataProperty"/>
        <rdfs:range rdf:resource="http://www.w3.org/2001/XMLSchema#int"/>
        <rdfs:comment>The quantity of pallets in a consignment, a shipment or in wave</rdfs:comment>
    </owl:DatatypeProperty>
    


    <!-- https://w3id.org/latuli/ontology/m3#qttPalletsBuilt -->


    <owl:DatatypeProperty rdf:about="https://w3id.org/latuli/ontology/m3#qttPalletsBuilt">
        <rdfs:subPropertyOf rdf:resource="http://www.w3.org/2002/07/owl#topDataProperty"/>
        <rdfs:range rdf:resource="http://www.w3.org/2001/XMLSchema#int"/>
        <rdfs:comment>The quantity of pallets built in a wave</rdfs:comment>
    </owl:DatatypeProperty>
    


    <!-- https://w3id.org/latuli/ontology/m3#qttReconstructedPallets -->


    <owl:DatatypeProperty rdf:about="https://w3id.org/latuli/ontology/m3#qttReconstructedPallets">
        <rdfs:subPropertyOf rdf:resource="http://www.w3.org/2002/07/owl#topDataProperty"/>
        <rdfs:domain rdf:resource="https://w3id.org/latuli/ontology/m3#Consignment"/>
        <rdfs:range rdf:resource="http://www.w3.org/2001/XMLSchema#int"/>
        <rdfs:comment>The quantity of reconstructed pallets in a consignment</rdfs:comment>
    </owl:DatatypeProperty>
    


    <!-- https://w3id.org/latuli/ontology/m3#qttReconstructedParcels -->


    <owl:DatatypeProperty rdf:about="https://w3id.org/latuli/ontology/m3#qttReconstructedParcels">
        <rdfs:subPropertyOf rdf:resource="http://www.w3.org/2002/07/owl#topDataProperty"/>
        <rdfs:domain rdf:resource="https://w3id.org/latuli/ontology/m3#Consignment"/>
        <rdfs:range rdf:resource="http://www.w3.org/2001/XMLSchema#int"/>
        <rdfs:comment>The quantity of reconstructed parcels in a consignment</rdfs:comment>
    </owl:DatatypeProperty>
    


    <!-- https://w3id.org/latuli/ontology/m3#qttShipments -->


    <owl:DatatypeProperty rdf:about="https://w3id.org/latuli/ontology/m3#qttShipments">
        <rdfs:subPropertyOf rdf:resource="http://www.w3.org/2002/07/owl#topDataProperty"/>
        <rdfs:domain rdf:resource="https://w3id.org/latuli/ontology/m3#Wave"/>
        <rdfs:range rdf:resource="http://www.w3.org/2001/XMLSchema#int"/>
        <rdfs:comment>The quantity of shipments processed in a wave</rdfs:comment>
    </owl:DatatypeProperty>
    


    <!-- https://w3id.org/latuli/ontology/m3#qttTasks -->


    <owl:DatatypeProperty rdf:about="https://w3id.org/latuli/ontology/m3#qttTasks">
        <rdfs:subPropertyOf rdf:resource="http://www.w3.org/2002/07/owl#topDataProperty"/>
        <rdfs:domain rdf:resource="https://w3id.org/latuli/ontology/m3#Wave"/>
        <rdfs:range rdf:resource="http://www.w3.org/2001/XMLSchema#int"/>
        <rdfs:comment>The quantity of tasks processed in a wave</rdfs:comment>
    </owl:DatatypeProperty>
    


    <!-- https://w3id.org/latuli/ontology/m3#qttTrailers -->


    <owl:DatatypeProperty rdf:about="https://w3id.org/latuli/ontology/m3#qttTrailers">
        <rdfs:subPropertyOf rdf:resource="http://www.w3.org/2002/07/owl#topDataProperty"/>
        <rdfs:domain rdf:resource="https://w3id.org/latuli/ontology/m3#Wave"/>
        <rdfs:range rdf:resource="http://www.w3.org/2001/XMLSchema#int"/>
        <rdfs:comment>The quantity of trailers processed in a wave</rdfs:comment>
    </owl:DatatypeProperty>
    


    <!-- https://w3id.org/latuli/ontology/m3#quantity -->


    <owl:DatatypeProperty rdf:about="https://w3id.org/latuli/ontology/m3#quantity">
        <rdfs:subPropertyOf rdf:resource="http://www.w3.org/2002/07/owl#topDataProperty"/>
        <rdfs:domain rdf:resource="https://w3id.org/latuli/ontology/m3#ShipmentItem"/>
        <rdfs:range rdf:resource="http://www.w3.org/2001/XMLSchema#int"/>
        <rdfs:comment>The quantity of individual items in a trade item</rdfs:comment>
    </owl:DatatypeProperty>
    


    <!-- https://w3id.org/latuli/ontology/m3#receiverHashCode -->


    <owl:DatatypeProperty rdf:about="https://w3id.org/latuli/ontology/m3#receiverHashCode">
        <rdfs:range rdf:resource="http://www.w3.org/2001/XMLSchema#string"/>
        <rdfs:comment>A hashcode which represents a receiver party using a numeric value</rdfs:comment>
    </owl:DatatypeProperty>
    


    <!-- https://w3id.org/latuli/ontology/m3#reconstructedScanOn -->


    <owl:DatatypeProperty rdf:about="https://w3id.org/latuli/ontology/m3#reconstructedScanOn">
        <rdfs:subPropertyOf rdf:resource="http://www.w3.org/2002/07/owl#topDataProperty"/>
        <rdfs:domain rdf:resource="https://w3id.org/latuli/ontology/m3#XDocLoadingUnit"/>
        <rdfs:range rdf:resource="http://www.w3.org/2001/XMLSchema#dateTime"/>
        <rdfs:comment>Timestamp for when an XDocLoadingUnit (cross-dock loading unit) is being reconstructed.</rdfs:comment>
    </owl:DatatypeProperty>
    


    <!-- https://w3id.org/latuli/ontology/m3#reconstructionLane -->


    <owl:DatatypeProperty rdf:about="https://w3id.org/latuli/ontology/m3#reconstructionLane">
        <rdfs:subPropertyOf rdf:resource="http://www.w3.org/2002/07/owl#topDataProperty"/>
        <rdfs:range rdf:resource="http://www.w3.org/2001/XMLSchema#string"/>
        <rdfs:comment>A lane or section in a terminal or hub used for the reconstruction of goods</rdfs:comment>
    </owl:DatatypeProperty>
    


    <!-- https://w3id.org/latuli/ontology/m3#reconstructionLocation -->


    <owl:DatatypeProperty rdf:about="https://w3id.org/latuli/ontology/m3#reconstructionLocation">
        <rdfs:range rdf:resource="http://www.w3.org/2001/XMLSchema#string"/>
        <rdfs:comment>A location in which a reconstruction takes place.</rdfs:comment>
    </owl:DatatypeProperty>
    


    <!-- https://w3id.org/latuli/ontology/m3#reconstructionTypeId -->


    <owl:DatatypeProperty rdf:about="https://w3id.org/latuli/ontology/m3#reconstructionTypeId">
        <rdfs:range rdf:resource="http://www.w3.org/2001/XMLSchema#string"/>
        <rdfs:comment>The type of reconstruction performed. Values are either loose cartons (LooseCarton), recon pallet (ReconPallet), or recon parcel (ReconParcel).</rdfs:comment>
    </owl:DatatypeProperty>
    


    <!-- https://w3id.org/latuli/ontology/m3#releasedOn -->


    <owl:DatatypeProperty rdf:about="https://w3id.org/latuli/ontology/m3#releasedOn">
        <rdfs:subPropertyOf rdf:resource="http://www.w3.org/2002/07/owl#topDataProperty"/>
        <rdfs:range rdf:resource="http://www.w3.org/2001/XMLSchema#dateTime"/>
        <rdfs:comment>Timestamp for when a wave is released.</rdfs:comment>
    </owl:DatatypeProperty>
    


    <!-- https://w3id.org/latuli/ontology/m3#salesOrder -->


    <owl:DatatypeProperty rdf:about="https://w3id.org/latuli/ontology/m3#salesOrder">
        <rdfs:subPropertyOf rdf:resource="http://www.w3.org/2002/07/owl#topDataProperty"/>
        <rdfs:range rdf:resource="http://www.w3.org/2001/XMLSchema#string"/>
        <rdfs:comment>A reference to a sales order associated with a trade item</rdfs:comment>
    </owl:DatatypeProperty>
    


    <!-- https://w3id.org/latuli/ontology/m3#shipmentId -->


    <owl:DatatypeProperty rdf:about="https://w3id.org/latuli/ontology/m3#shipmentId">
        <rdfs:range rdf:resource="http://www.w3.org/2001/XMLSchema#string"/>
        <rdfs:comment>A unique identifier for a shipment.</rdfs:comment>
    </owl:DatatypeProperty>
    


    <!-- https://w3id.org/latuli/ontology/m3#shippedOn -->


    <owl:DatatypeProperty rdf:about="https://w3id.org/latuli/ontology/m3#shippedOn">
        <rdfs:subPropertyOf rdf:resource="http://www.w3.org/2002/07/owl#topDataProperty"/>
        <rdfs:domain rdf:resource="https://w3id.org/latuli/ontology/m3#Shipment"/>
        <rdfs:range rdf:resource="http://www.w3.org/2001/XMLSchema#dateTime"/>
        <rdfs:comment>Timestamp for when a shipment is sent from a shipper.</rdfs:comment>
        <skos:prefLabel xml:lang="nb">shippedOn</skos:prefLabel>
    </owl:DatatypeProperty>
    


    <!-- https://w3id.org/latuli/ontology/m3#shipperHashCode -->


    <owl:DatatypeProperty rdf:about="https://w3id.org/latuli/ontology/m3#shipperHashCode">
        <rdfs:range rdf:resource="http://www.w3.org/2001/XMLSchema#string"/>
        <rdfs:comment>A hashcode which represents a shipper party using a numeric value</rdfs:comment>
    </owl:DatatypeProperty>
    


    <!-- https://w3id.org/latuli/ontology/m3#splitShipment -->


    <owl:DatatypeProperty rdf:about="https://w3id.org/latuli/ontology/m3#splitShipment">
        <rdfs:subPropertyOf rdf:resource="http://www.w3.org/2002/07/owl#topDataProperty"/>
        <rdfs:range rdf:resource="http://www.w3.org/2001/XMLSchema#int"/>
        <rdfs:comment>A flag that defines whether a shipment has been split or not.</rdfs:comment>
    </owl:DatatypeProperty>
    


    <!-- https://w3id.org/latuli/ontology/m3#status -->


    <owl:DatatypeProperty rdf:about="https://w3id.org/latuli/ontology/m3#status">
        <rdfs:subPropertyOf rdf:resource="http://www.w3.org/2002/07/owl#topDataProperty"/>
        <rdfs:range rdf:resource="http://www.w3.org/2001/XMLSchema#string"/>
        <rdfs:comment>The status of a wave.</rdfs:comment>
    </owl:DatatypeProperty>
    


    <!-- https://w3id.org/latuli/ontology/m3#supplierProductDescription -->


    <owl:DatatypeProperty rdf:about="https://w3id.org/latuli/ontology/m3#supplierProductDescription">
        <rdfs:subPropertyOf rdf:resource="http://www.w3.org/2002/07/owl#topDataProperty"/>
        <rdfs:range rdf:resource="http://www.w3.org/2001/XMLSchema#string"/>
        <rdfs:comment>A description of a trade item by the supplier.</rdfs:comment>
    </owl:DatatypeProperty>
    


    <!-- https://w3id.org/latuli/ontology/m3#supplierProductId -->


    <owl:DatatypeProperty rdf:about="https://w3id.org/latuli/ontology/m3#supplierProductId">
        <rdfs:subPropertyOf rdf:resource="http://www.w3.org/2002/07/owl#topDataProperty"/>
        <rdfs:range rdf:resource="http://www.w3.org/2001/XMLSchema#string"/>
        <rdfs:comment>The identifier of a trade item used by the supplier.</rdfs:comment>
    </owl:DatatypeProperty>
    


    <!-- https://w3id.org/latuli/ontology/m3#supplierQuantity -->


    <owl:DatatypeProperty rdf:about="https://w3id.org/latuli/ontology/m3#supplierQuantity">
        <rdfs:subPropertyOf rdf:resource="http://www.w3.org/2002/07/owl#topDataProperty"/>
        <rdfs:range rdf:resource="http://www.w3.org/2001/XMLSchema#decimal"/>
        <rdfs:comment>The quantity of trade items as provided by the supplier.</rdfs:comment>
    </owl:DatatypeProperty>
    


    <!-- https://w3id.org/latuli/ontology/m3#taskClosedOn -->


    <owl:DatatypeProperty rdf:about="https://w3id.org/latuli/ontology/m3#taskClosedOn">
        <rdfs:subPropertyOf rdf:resource="http://www.w3.org/2002/07/owl#topDataProperty"/>
        <rdfs:domain rdf:resource="https://w3id.org/latuli/ontology/m3#Consignment"/>
        <rdfs:range rdf:resource="http://www.w3.org/2001/XMLSchema#dateTime"/>
        <rdfs:comment>Timestamp for when a consignment task is closed.</rdfs:comment>
    </owl:DatatypeProperty>
    


    <!-- https://w3id.org/latuli/ontology/m3#taskDescription -->


    <owl:DatatypeProperty rdf:about="https://w3id.org/latuli/ontology/m3#taskDescription">
        <rdfs:subPropertyOf rdf:resource="http://www.w3.org/2002/07/owl#topDataProperty"/>
        <rdfs:range rdf:resource="http://www.w3.org/2001/XMLSchema#string"/>
        <rdfs:comment>A description of a reconstruction task related to a consignment. Examples are Reconstruct by Address, Reconstruct by Product or Reconstruct by Order.</rdfs:comment>
    </owl:DatatypeProperty>
    


    <!-- https://w3id.org/latuli/ontology/m3#taskId -->


    <owl:DatatypeProperty rdf:about="https://w3id.org/latuli/ontology/m3#taskId">
        <rdfs:subPropertyOf rdf:resource="http://www.w3.org/2002/07/owl#topDataProperty"/>
        <rdfs:range rdf:resource="http://www.w3.org/2001/XMLSchema#string"/>
        <rdfs:comment>An identifier that describes the reconstruction task related to a consignment.</rdfs:comment>
    </owl:DatatypeProperty>
    


    <!-- https://w3id.org/latuli/ontology/m3#totalConsignmentVolume -->


    <owl:DatatypeProperty rdf:about="https://w3id.org/latuli/ontology/m3#totalConsignmentVolume">
        <rdfs:subPropertyOf rdf:resource="http://www.w3.org/2002/07/owl#topDataProperty"/>
        <rdfs:domain rdf:resource="https://w3id.org/latuli/ontology/m3#Consignment"/>
        <rdfs:range rdf:resource="http://www.w3.org/2001/XMLSchema#decimal"/>
        <rdfs:comment>The total volume of a consignment.</rdfs:comment>
    </owl:DatatypeProperty>
    


    <!-- https://w3id.org/latuli/ontology/m3#totalConsignmentWeight -->


    <owl:DatatypeProperty rdf:about="https://w3id.org/latuli/ontology/m3#totalConsignmentWeight">
        <rdfs:subPropertyOf rdf:resource="http://www.w3.org/2002/07/owl#topDataProperty"/>
        <rdfs:domain rdf:resource="https://w3id.org/latuli/ontology/m3#Consignment"/>
        <rdfs:range rdf:resource="http://www.w3.org/2001/XMLSchema#decimal"/>
        <rdfs:comment>The total weight of a consignment.</rdfs:comment>
    </owl:DatatypeProperty>
    


    <!-- https://w3id.org/latuli/ontology/m3#transportId -->


    <owl:DatatypeProperty rdf:about="https://w3id.org/latuli/ontology/m3#transportId">
        <rdfs:subPropertyOf rdf:resource="http://www.w3.org/2002/07/owl#topDataProperty"/>
        <rdfs:range rdf:resource="http://www.w3.org/2001/XMLSchema#string"/>
        <rdfs:comment>A unique identifier for a transport.</rdfs:comment>
    </owl:DatatypeProperty>
    


    <!-- https://w3id.org/latuli/ontology/m3#transportName -->


    <owl:DatatypeProperty rdf:about="https://w3id.org/latuli/ontology/m3#transportName">
        <rdfs:range rdf:resource="http://www.w3.org/2001/XMLSchema#string"/>
        <rdfs:comment>The name of a transport. Examples are TJUE042ZU2 and 528776.</rdfs:comment>
    </owl:DatatypeProperty>
    


    <!-- https://w3id.org/latuli/ontology/m3#transportType -->


    <owl:DatatypeProperty rdf:about="https://w3id.org/latuli/ontology/m3#transportType">
        <rdfs:subPropertyOf rdf:resource="http://www.w3.org/2002/07/owl#topDataProperty"/>
        <rdfs:domain rdf:resource="https://w3id.org/latuli/ontology/m3#Transport"/>
        <rdfs:range rdf:resource="http://www.w3.org/2001/XMLSchema#string"/>
        <rdfs:comment>A flag that defines whether a transport is inbound (IN) or outbound (OUT)</rdfs:comment>
    </owl:DatatypeProperty>
    


    <!-- https://w3id.org/latuli/ontology/m3#volume -->


    <owl:DatatypeProperty rdf:about="https://w3id.org/latuli/ontology/m3#volume">
        <rdfs:subPropertyOf rdf:resource="http://www.w3.org/2002/07/owl#topDataProperty"/>
        <rdfs:range rdf:resource="http://www.w3.org/2001/XMLSchema#decimal"/>
        <rdfs:comment>The volume of an xDocLoadingUnit (cross-dock loading unit).</rdfs:comment>
    </owl:DatatypeProperty>
    


    <!-- https://w3id.org/latuli/ontology/m3#waveClosedOn -->


    <owl:DatatypeProperty rdf:about="https://w3id.org/latuli/ontology/m3#waveClosedOn">
        <rdfs:range rdf:resource="http://www.w3.org/2001/XMLSchema#dateTime"/>
        <rdfs:comment>Timestamp for when a wave is closed.</rdfs:comment>
    </owl:DatatypeProperty>
    


    <!-- https://w3id.org/latuli/ontology/m3#waveEndProcessingOn -->


    <owl:DatatypeProperty rdf:about="https://w3id.org/latuli/ontology/m3#waveEndProcessingOn">
        <rdfs:subPropertyOf rdf:resource="http://www.w3.org/2002/07/owl#topDataProperty"/>
        <rdfs:domain rdf:resource="https://w3id.org/latuli/ontology/m3#Wave"/>
        <rdfs:range rdf:resource="http://www.w3.org/2001/XMLSchema#dateTime"/>
        <rdfs:comment>Timestamp for when a wave process is ended.</rdfs:comment>
    </owl:DatatypeProperty>
    


    <!-- https://w3id.org/latuli/ontology/m3#waveId -->


    <owl:DatatypeProperty rdf:about="https://w3id.org/latuli/ontology/m3#waveId">
        <rdfs:range rdf:resource="http://www.w3.org/2001/XMLSchema#string"/>
        <rdfs:comment>A unique identifier for a wave.</rdfs:comment>
    </owl:DatatypeProperty>
    


    <!-- https://w3id.org/latuli/ontology/m3#wavePlannedOn -->


    <owl:DatatypeProperty rdf:about="https://w3id.org/latuli/ontology/m3#wavePlannedOn">
        <rdfs:range rdf:resource="http://www.w3.org/2001/XMLSchema#dateTime"/>
        <rdfs:comment>Timestamp for when a wave has been planned.</rdfs:comment>
    </owl:DatatypeProperty>
    


    <!-- https://w3id.org/latuli/ontology/m3#waveReleasedOn -->


    <owl:DatatypeProperty rdf:about="https://w3id.org/latuli/ontology/m3#waveReleasedOn">
        <rdfs:range rdf:resource="http://www.w3.org/2001/XMLSchema#dateTime"/>
        <rdfs:comment>Timestamp for when a wave has been released to the floor.</rdfs:comment>
    </owl:DatatypeProperty>
    


    <!-- https://w3id.org/latuli/ontology/m3#waveStartProcessingOn -->


    <owl:DatatypeProperty rdf:about="https://w3id.org/latuli/ontology/m3#waveStartProcessingOn">
        <rdfs:subPropertyOf rdf:resource="http://www.w3.org/2002/07/owl#topDataProperty"/>
        <rdfs:domain rdf:resource="https://w3id.org/latuli/ontology/m3#Wave"/>
        <rdfs:range rdf:resource="http://www.w3.org/2001/XMLSchema#dateTime"/>
        <rdfs:comment>Timestamp for when a wave process is started.</rdfs:comment>
    </owl:DatatypeProperty>
    


    <!-- https://w3id.org/latuli/ontology/m3#weight -->


    <owl:DatatypeProperty rdf:about="https://w3id.org/latuli/ontology/m3#weight">
        <rdfs:subPropertyOf rdf:resource="http://www.w3.org/2002/07/owl#topDataProperty"/>
        <rdfs:range rdf:resource="http://www.w3.org/2001/XMLSchema#decimal"/>
        <rdfs:comment>The weight of an xDocLoadingUnit (cross-dock loading unit).</rdfs:comment>
    </owl:DatatypeProperty>
    


    <!-- 
    ///////////////////////////////////////////////////////////////////////////////////////
    //
    // Classes
    //
    ///////////////////////////////////////////////////////////////////////////////////////
     -->


    


    <!-- http://www.opengis.net/ont/geosparql#Feature -->


    <owl:Class rdf:about="http://www.opengis.net/ont/geosparql#Feature">
        <rdfs:subClassOf rdf:resource="http://www.opengis.net/ont/geosparql#SpatialObject"/>
        <owl:disjointWith rdf:resource="http://www.opengis.net/ont/geosparql#Geometry"/>
        <dc:contributor>Matthew Perry</dc:contributor>
        <dc:creator>OGC GeoSPARQL 1.0 Standard Working Group</dc:creator>
        <dc:date rdf:datatype="http://www.w3.org/2001/XMLSchema#date">2011-06-16</dc:date>
        <dc:description xml:lang="en">
      This class represents the top-level feature type. This class is 
      equivalent to GFI_Feature defined in ISO 19156:2011, and it is 
      superclass of all feature types.
    </dc:description>
        <rdfs:comment xml:lang="en">
      This class represents the top-level feature type. This class is 
      equivalent to GFI_Feature defined in ISO 19156:2011, and it is 
      superclass of all feature types.
    </rdfs:comment>
        <rdfs:isDefinedBy rdf:resource="http://www.opengis.net/ont/geosparql"/>
        <rdfs:isDefinedBy rdf:resource="http://www.opengis.net/spec/geosparql/1.0"/>
        <rdfs:label xml:lang="en">Feature</rdfs:label>
        <skos:definition xml:lang="en">
      This class represents the top-level feature type. This class is 
      equivalent to GFI_Feature defined in ISO 19156:2011, and it is 
      superclass of all feature types.
    </skos:definition>
        <skos:prefLabel xml:lang="en">Feature</skos:prefLabel>
    </owl:Class>
    


    <!-- http://www.opengis.net/ont/geosparql#Geometry -->


    <owl:Class rdf:about="http://www.opengis.net/ont/geosparql#Geometry">
        <rdfs:subClassOf rdf:resource="http://www.opengis.net/ont/geosparql#SpatialObject"/>
        <dc:contributor>Matthew Perry</dc:contributor>
        <dc:creator>OGC GeoSPARQL 1.0 Standard Working Group</dc:creator>
        <dc:date rdf:datatype="http://www.w3.org/2001/XMLSchema#date">2011-06-16</dc:date>
        <dc:description xml:lang="en">
      The class represents the top-level geometry type. This class is 
      equivalent to the UML class GM_Object defined in ISO 19107, and 
      it is superclass of all geometry types.
    </dc:description>
        <rdfs:comment xml:lang="en">
      The class represents the top-level geometry type. This class is 
      equivalent to the UML class GM_Object defined in ISO 19107, and 
      it is superclass of all geometry types.
    </rdfs:comment>
        <rdfs:isDefinedBy rdf:resource="http://www.opengis.net/ont/geosparql"/>
        <rdfs:isDefinedBy rdf:resource="http://www.opengis.net/spec/geosparql/1.0"/>
        <rdfs:label xml:lang="en">Geometry</rdfs:label>
        <skos:definition xml:lang="en">
      The class represents the top-level geometry type. This class is 
      equivalent to the UML class GM_Object defined in ISO 19107, and 
      it is superclass of all geometry types.
    </skos:definition>
        <skos:prefLabel xml:lang="en">Geometry</skos:prefLabel>
    </owl:Class>
    


    <!-- http://www.opengis.net/ont/geosparql#SpatialObject -->


    <owl:Class rdf:about="http://www.opengis.net/ont/geosparql#SpatialObject">
        <dc:contributor>Matthew Perry</dc:contributor>
        <dc:creator>OGC GeoSPARQL 1.0 Standard Working Group</dc:creator>
        <dc:date rdf:datatype="http://www.w3.org/2001/XMLSchema#date">2011-06-16</dc:date>
        <dc:description xml:lang="en">
      The class spatial-object represents everything that can have 
      a spatial representation. It is superclass of feature and geometry.
    </dc:description>
        <rdfs:comment xml:lang="en">
      The class spatial-object represents everything that can have 
      a spatial representation. It is superclass of feature and geometry.
    </rdfs:comment>
        <rdfs:isDefinedBy rdf:resource="http://www.opengis.net/ont/geosparql"/>
        <rdfs:isDefinedBy rdf:resource="http://www.opengis.net/spec/geosparql/1.0"/>
        <rdfs:label xml:lang="en">SpatialObject</rdfs:label>
        <skos:definition xml:lang="en">
      The class spatial-object represents everything that can have 
      a spatial representation. It is superclass of feature and geometry.
    </skos:definition>
        <skos:prefLabel xml:lang="en">SpatialObject</skos:prefLabel>
    </owl:Class>
    


    <!-- https://w3id.org/latuli/ontology/m3#Carrier -->


    <owl:Class rdf:about="https://w3id.org/latuli/ontology/m3#Carrier">
        <rdfs:subClassOf rdf:resource="https://w3id.org/latuli/ontology/m3#Party"/>
        <rdfs:comment>A company, which physically transports goods from one place to another.</rdfs:comment>
    </owl:Class>
    


    <!-- https://w3id.org/latuli/ontology/m3#Consignee -->


    <owl:Class rdf:about="https://w3id.org/latuli/ontology/m3#Consignee">
        <rdfs:subClassOf rdf:resource="https://w3id.org/latuli/ontology/m3#Party"/>
        <rdfs:comment>In a consignment view / scenario, the entity who will receive the physical shipment.</rdfs:comment>
    </owl:Class>
    


    <!-- https://w3id.org/latuli/ontology/m3#Consignment -->


    <owl:Class rdf:about="https://w3id.org/latuli/ontology/m3#Consignment">
        <rdfs:subClassOf>
            <owl:Restriction>
                <owl:onProperty rdf:resource="https://w3id.org/latuli/ontology/m3#hasCarrierParty"/>
                <owl:someValuesFrom rdf:resource="https://w3id.org/latuli/ontology/m3#Carrier"/>
            </owl:Restriction>
        </rdfs:subClassOf>
        <rdfs:subClassOf>
            <owl:Restriction>
                <owl:onProperty rdf:resource="https://w3id.org/latuli/ontology/m3#hasConsigneeParty"/>
                <owl:someValuesFrom rdf:resource="https://w3id.org/latuli/ontology/m3#Consignee"/>
            </owl:Restriction>
        </rdfs:subClassOf>
        <rdfs:subClassOf>
            <owl:Restriction>
                <owl:onProperty rdf:resource="https://w3id.org/latuli/ontology/m3#hasConsignorParty"/>
                <owl:someValuesFrom rdf:resource="https://w3id.org/latuli/ontology/m3#Consignor"/>
            </owl:Restriction>
        </rdfs:subClassOf>
        <rdfs:subClassOf>
            <owl:Restriction>
                <owl:onProperty rdf:resource="https://w3id.org/latuli/ontology/m3#hasHubParty"/>
                <owl:someValuesFrom rdf:resource="https://w3id.org/latuli/ontology/m3#Party"/>
            </owl:Restriction>
        </rdfs:subClassOf>
        <rdfs:subClassOf>
            <owl:Restriction>
                <owl:onProperty rdf:resource="https://w3id.org/latuli/ontology/m3#includesTransport"/>
                <owl:someValuesFrom rdf:resource="https://w3id.org/latuli/ontology/m3#Transport"/>
            </owl:Restriction>
        </rdfs:subClassOf>
        <rdfs:subClassOf>
            <owl:Restriction>
                <owl:onProperty rdf:resource="https://w3id.org/latuli/ontology/m3#processedByWave"/>
                <owl:someValuesFrom rdf:resource="https://w3id.org/latuli/ontology/m3#Wave"/>
            </owl:Restriction>
        </rdfs:subClassOf>
        <rdfs:comment>A consignment is a logical grouping of goods (one or more physical entities) that is intended to be transported as a whole from a consignor to a consignee by a carrier or freight forwarder via one or more modes of transport, subject to one single transport contract.</rdfs:comment>
    </owl:Class>
    


    <!-- https://w3id.org/latuli/ontology/m3#Consignor -->


    <owl:Class rdf:about="https://w3id.org/latuli/ontology/m3#Consignor">
        <rdfs:subClassOf rdf:resource="https://w3id.org/latuli/ontology/m3#Party"/>
        <rdfs:comment>In a consignment view / scenario, the entity who will ship the physical shipment.</rdfs:comment>
    </owl:Class>
    


    <!-- https://w3id.org/latuli/ontology/m3#DangerousGoods -->


    <owl:Class rdf:about="https://w3id.org/latuli/ontology/m3#DangerousGoods">
        <rdfs:subClassOf>
            <owl:Restriction>
                <owl:onProperty rdf:resource="https://w3id.org/latuli/ontology/m3#belongsToShipment"/>
                <owl:someValuesFrom rdf:resource="https://w3id.org/latuli/ontology/m3#Shipment"/>
            </owl:Restriction>
        </rdfs:subClassOf>
        <rdfs:subClassOf>
            <owl:Restriction>
                <owl:onProperty rdf:resource="https://w3id.org/latuli/ontology/m3#hasLoadingUnit"/>
                <owl:someValuesFrom rdf:resource="https://w3id.org/latuli/ontology/m3#LoadingUnit"/>
            </owl:Restriction>
        </rdfs:subClassOf>
        <rdfs:subClassOf>
            <owl:Restriction>
                <owl:onProperty rdf:resource="https://w3id.org/latuli/ontology/m3#relatesToTradeItem"/>
                <owl:someValuesFrom rdf:resource="https://w3id.org/latuli/ontology/m3#TradeItem"/>
            </owl:Restriction>
        </rdfs:subClassOf>
    </owl:Class>
    


    <!-- https://w3id.org/latuli/ontology/m3#HubReconstructionLocation -->


    <owl:Class rdf:about="https://w3id.org/latuli/ontology/m3#HubReconstructionLocation">
        <owl:equivalentClass rdf:resource="https://w3id.org/latuli/ontology/m3#Terminal"/>
        <rdfs:subClassOf>
            <owl:Restriction>
                <owl:onProperty rdf:resource="https://w3id.org/latuli/ontology/m3#hasParty"/>
                <owl:someValuesFrom rdf:resource="https://w3id.org/latuli/ontology/m3#Party"/>
            </owl:Restriction>
        </rdfs:subClassOf>
        <rdfs:comment>The location where a reconstruction of goods takes place.</rdfs:comment>
    </owl:Class>
    


    <!-- https://w3id.org/latuli/ontology/m3#LoadingUnit -->


    <owl:Class rdf:about="https://w3id.org/latuli/ontology/m3#LoadingUnit">
        <rdfs:comment>A logistic unit is a unit of any composition made up for transport and or storage which has to be managed throughout the supply chain.</rdfs:comment>
    </owl:Class>
    


    <!-- https://w3id.org/latuli/ontology/m3#Party -->


    <owl:Class rdf:about="https://w3id.org/latuli/ontology/m3#Party">
        <rdfs:comment>A person or group of people constituting a particular side in a contract or legal action.</rdfs:comment>
    </owl:Class>
    


    <!-- https://w3id.org/latuli/ontology/m3#Receiver -->


    <owl:Class rdf:about="https://w3id.org/latuli/ontology/m3#Receiver">
        <rdfs:subClassOf rdf:resource="https://w3id.org/latuli/ontology/m3#Party"/>
        <rdfs:comment>In a shipment scenario, a party who engages in receiving goods.</rdfs:comment>
    </owl:Class>
    


    <!-- https://w3id.org/latuli/ontology/m3#Shipment -->


    <owl:Class rdf:about="https://w3id.org/latuli/ontology/m3#Shipment">
        <rdfs:subClassOf>
            <owl:Restriction>
                <owl:onProperty rdf:resource="https://w3id.org/latuli/ontology/m3#hasReceiverParty"/>
                <owl:someValuesFrom rdf:resource="https://w3id.org/latuli/ontology/m3#Receiver"/>
            </owl:Restriction>
        </rdfs:subClassOf>
        <rdfs:subClassOf>
            <owl:Restriction>
                <owl:onProperty rdf:resource="https://w3id.org/latuli/ontology/m3#hasShipperParty"/>
                <owl:someValuesFrom rdf:resource="https://w3id.org/latuli/ontology/m3#Shipper"/>
            </owl:Restriction>
        </rdfs:subClassOf>
        <rdfs:comment>A shipment is an identifiable collection of one or more Trade Items available to be transported together from the shipper (Original Consignor/Shipper), to the receiver (Final/Ultimate Consignee). Typically the shipment is the entity communicated between trading partners in the Despatch and Receiving Advice.</rdfs:comment>
    </owl:Class>
    


    <!-- https://w3id.org/latuli/ontology/m3#ShipmentItem -->


    <owl:Class rdf:about="https://w3id.org/latuli/ontology/m3#ShipmentItem">
        <rdfs:subClassOf>
            <owl:Restriction>
                <owl:onProperty rdf:resource="https://w3id.org/latuli/ontology/m3#belongsToShipment"/>
                <owl:someValuesFrom rdf:resource="https://w3id.org/latuli/ontology/m3#Shipment"/>
            </owl:Restriction>
        </rdfs:subClassOf>
        <rdfs:subClassOf>
            <owl:Restriction>
                <owl:onProperty rdf:resource="https://w3id.org/latuli/ontology/m3#hasLoadingUnit"/>
                <owl:someValuesFrom rdf:resource="https://w3id.org/latuli/ontology/m3#LoadingUnit"/>
            </owl:Restriction>
        </rdfs:subClassOf>
        <rdfs:comment>A shipment is an identifiable collection of one or more Trade Items available to be transported together from the shipper (Original Consignor/Shipper), to the receiver (Final/Ultimate Consignee). Typically the shipment is the entity communicated between trading partners in the Despatch and Receiving Advice.</rdfs:comment>
    </owl:Class>
    


    <!-- https://w3id.org/latuli/ontology/m3#Shipper -->


    <owl:Class rdf:about="https://w3id.org/latuli/ontology/m3#Shipper">
        <rdfs:subClassOf rdf:resource="https://w3id.org/latuli/ontology/m3#Party"/>
        <rdfs:comment>In a shipment scenario, a party who engages in shipping goods.</rdfs:comment>
    </owl:Class>
    


    <!-- https://w3id.org/latuli/ontology/m3#Terminal -->


    <owl:Class rdf:about="https://w3id.org/latuli/ontology/m3#Terminal"/>
    


    <!-- https://w3id.org/latuli/ontology/m3#TerminalOperator -->


    <owl:Class rdf:about="https://w3id.org/latuli/ontology/m3#TerminalOperator">
        <rdfs:subClassOf rdf:resource="https://w3id.org/latuli/ontology/m3#Party"/>
        <rdfs:comment>Terminal operator means a person who by ownership or contractual agreement is charged with the responsibility for, or physical control over, and operation of a logistics terminal.</rdfs:comment>
    </owl:Class>
    


    <!-- https://w3id.org/latuli/ontology/m3#TradeItem -->


    <owl:Class rdf:about="https://w3id.org/latuli/ontology/m3#TradeItem">
        <rdfs:subClassOf>
            <owl:Restriction>
                <owl:onProperty rdf:resource="https://w3id.org/latuli/ontology/m3#belongsToShipment"/>
                <owl:someValuesFrom rdf:resource="https://w3id.org/latuli/ontology/m3#Shipment"/>
            </owl:Restriction>
        </rdfs:subClassOf>
        <rdfs:subClassOf>
            <owl:Restriction>
                <owl:onProperty rdf:resource="https://w3id.org/latuli/ontology/m3#hasLoadingUnit"/>
                <owl:someValuesFrom rdf:resource="https://w3id.org/latuli/ontology/m3#LoadingUnit"/>
            </owl:Restriction>
        </rdfs:subClassOf>
        <rdfs:comment>A trade item is any item (product or service) upon which there is a need to retrieve pre-defined information and that may be priced, or ordered, or invoiced at any point in any supply chain.</rdfs:comment>
    </owl:Class>
    


    <!-- https://w3id.org/latuli/ontology/m3#Transport -->


    <owl:Class rdf:about="https://w3id.org/latuli/ontology/m3#Transport">
        <rdfs:comment>Transport is the act of moving goods and materials from one location to another</rdfs:comment>
    </owl:Class>
    


    <!-- https://w3id.org/latuli/ontology/m3#Wave -->


    <owl:Class rdf:about="https://w3id.org/latuli/ontology/m3#Wave">
        <rdfs:subClassOf>
            <owl:Restriction>
                <owl:onProperty rdf:resource="https://w3id.org/latuli/ontology/m3#hasHubParty"/>
                <owl:someValuesFrom rdf:resource="https://w3id.org/latuli/ontology/m3#Party"/>
            </owl:Restriction>
        </rdfs:subClassOf>
        <rdfs:comment>A wave is a planning event that involves allocating a specific inventory or storage zone, and employees to pick items from those sections.</rdfs:comment>
    </owl:Class>
    


    <!-- https://w3id.org/latuli/ontology/m3#XDocLoadingUnit -->


    <owl:Class rdf:about="https://w3id.org/latuli/ontology/m3#XDocLoadingUnit">
        <rdfs:subClassOf>
            <owl:Restriction>
                <owl:onProperty rdf:resource="https://w3id.org/latuli/ontology/m3#hasCarrierParty"/>
                <owl:someValuesFrom rdf:resource="https://w3id.org/latuli/ontology/m3#Carrier"/>
            </owl:Restriction>
        </rdfs:subClassOf>
        <rdfs:subClassOf>
            <owl:Restriction>
                <owl:onProperty rdf:resource="https://w3id.org/latuli/ontology/m3#hasConsigneeParty"/>
                <owl:someValuesFrom rdf:resource="https://w3id.org/latuli/ontology/m3#Consignee"/>
            </owl:Restriction>
        </rdfs:subClassOf>
        <rdfs:subClassOf>
            <owl:Restriction>
                <owl:onProperty rdf:resource="https://w3id.org/latuli/ontology/m3#hasConsignorParty"/>
                <owl:someValuesFrom rdf:resource="https://w3id.org/latuli/ontology/m3#Consignor"/>
            </owl:Restriction>
        </rdfs:subClassOf>
        <rdfs:subClassOf>
            <owl:Restriction>
                <owl:onProperty rdf:resource="https://w3id.org/latuli/ontology/m3#hasHubReconstructionParty"/>
                <owl:someValuesFrom rdf:resource="https://w3id.org/latuli/ontology/m3#Party"/>
            </owl:Restriction>
        </rdfs:subClassOf>
        <rdfs:subClassOf>
            <owl:Restriction>
                <owl:onProperty rdf:resource="https://w3id.org/latuli/ontology/m3#hasInboundConsignment"/>
                <owl:someValuesFrom rdf:resource="https://w3id.org/latuli/ontology/m3#Consignment"/>
            </owl:Restriction>
        </rdfs:subClassOf>
        <rdfs:subClassOf>
            <owl:Restriction>
                <owl:onProperty rdf:resource="https://w3id.org/latuli/ontology/m3#hasInboundParentLoadingUnit"/>
                <owl:someValuesFrom rdf:resource="https://w3id.org/latuli/ontology/m3#LoadingUnit"/>
            </owl:Restriction>
        </rdfs:subClassOf>
        <rdfs:subClassOf>
            <owl:Restriction>
                <owl:onProperty rdf:resource="https://w3id.org/latuli/ontology/m3#hasLoadingUnit"/>
                <owl:someValuesFrom rdf:resource="https://w3id.org/latuli/ontology/m3#LoadingUnit"/>
            </owl:Restriction>
        </rdfs:subClassOf>
        <rdfs:subClassOf>
            <owl:Restriction>
                <owl:onProperty rdf:resource="https://w3id.org/latuli/ontology/m3#hasOutboundConsignment"/>
                <owl:someValuesFrom rdf:resource="https://w3id.org/latuli/ontology/m3#Consignment"/>
            </owl:Restriction>
        </rdfs:subClassOf>
        <rdfs:subClassOf>
            <owl:Restriction>
                <owl:onProperty rdf:resource="https://w3id.org/latuli/ontology/m3#hasOutboundParentLoadingUnit"/>
                <owl:someValuesFrom rdf:resource="https://w3id.org/latuli/ontology/m3#LoadingUnit"/>
            </owl:Restriction>
        </rdfs:subClassOf>
        <rdfs:subClassOf>
            <owl:Restriction>
                <owl:onProperty rdf:resource="https://w3id.org/latuli/ontology/m3#hasParty"/>
                <owl:someValuesFrom rdf:resource="https://w3id.org/latuli/ontology/m3#Party"/>
            </owl:Restriction>
        </rdfs:subClassOf>
        <rdfs:subClassOf>
            <owl:Restriction>
                <owl:onProperty rdf:resource="https://w3id.org/latuli/ontology/m3#hasReceiverParty"/>
                <owl:someValuesFrom rdf:resource="https://w3id.org/latuli/ontology/m3#Receiver"/>
            </owl:Restriction>
        </rdfs:subClassOf>
        <rdfs:subClassOf>
            <owl:Restriction>
                <owl:onProperty rdf:resource="https://w3id.org/latuli/ontology/m3#hasShipperParty"/>
                <owl:someValuesFrom rdf:resource="https://w3id.org/latuli/ontology/m3#Shipper"/>
            </owl:Restriction>
        </rdfs:subClassOf>
        <rdfs:subClassOf>
            <owl:Restriction>
                <owl:onProperty rdf:resource="https://w3id.org/latuli/ontology/m3#processedByWave"/>
                <owl:someValuesFrom rdf:resource="https://w3id.org/latuli/ontology/m3#Wave"/>
            </owl:Restriction>
        </rdfs:subClassOf>
        <rdfs:comment>A loading unit which is received through an inbound dock and then transferred across the dock to an outbound transportation dock.</rdfs:comment>
    </owl:Class>
</rdf:RDF>



<!-- Generated by the OWL API (version 5.1.14) https://github.com/owlcs/owlapi/ -->


