@prefix : <https://w3id.org/latuli/ontology/m3#> .
@prefix owl: <http://www.w3.org/2002/07/owl#> .
@prefix rdf: <http://www.w3.org/1999/02/22-rdf-syntax-ns#> .
@prefix xml: <http://www.w3.org/XML/1998/namespace> .
@prefix xsd: <http://www.w3.org/2001/XMLSchema#> .
@prefix rdfs: <http://www.w3.org/2000/01/rdf-schema#> .
@base <https://w3id.org/latuli/ontology/m3#> .

<https://w3id.org/latuli/ontology/m3#> rdf:type owl:Ontology ;
                                        owl:imports <http://www.opengis.net/ont/geosparql> .

#################################################################
#    Annotation properties
#################################################################

###  http://www.w3.org/2004/02/skos/core#prefLabel
<http://www.w3.org/2004/02/skos/core#prefLabel> rdf:type owl:AnnotationProperty .


#################################################################
#    Datatypes
#################################################################

###  http://www.opengis.net/ont/geosparql#gmlLiteral
<http://www.opengis.net/ont/geosparql#gmlLiteral> rdf:type rdfs:Datatype ;
                                                  <http://purl.org/dc/elements/1.1/contributor> "Matthew Perry" ;
                                                  <http://purl.org/dc/elements/1.1/creator> "OGC GeoSPARQL 1.0 Standard Working Group" ;
                                                  <http://purl.org/dc/elements/1.1/date> "2011-06-16"^^xsd:date ;
                                                  <http://purl.org/dc/elements/1.1/description> """
      A GML serialization of a geometry object.
    """@en ;
                                                  rdfs:comment """
      A GML serialization of a geometry object.
    """@en ;
                                                  rdfs:isDefinedBy <http://www.opengis.net/ont/geosparql> ,
                                                                   <http://www.opengis.net/spec/geosparql/1.0> ;
                                                  rdfs:label "GML Literal"@en ;
                                                  <http://www.w3.org/2004/02/skos/core#definition> """
      A GML serialization of a geometry object.
    """@en ;
                                                  <http://www.w3.org/2004/02/skos/core#prefLabel> "GML Literal"@en .


###  http://www.opengis.net/ont/geosparql#wktLiteral
<http://www.opengis.net/ont/geosparql#wktLiteral> rdf:type rdfs:Datatype ;
                                                  <http://purl.org/dc/elements/1.1/contributor> "Matthew Perry" ;
                                                  <http://purl.org/dc/elements/1.1/creator> "OGC GeoSPARQL 1.0 Standard Working Group" ;
                                                  <http://purl.org/dc/elements/1.1/date> "2011-06-16"^^xsd:date ;
                                                  <http://purl.org/dc/elements/1.1/description> """
      A Well-known Text serialization of a geometry object.
    """@en ;
                                                  rdfs:comment """
      A Well-known Text serialization of a geometry object.
    """@en ;
                                                  rdfs:isDefinedBy <http://www.opengis.net/ont/geosparql> ,
                                                                   <http://www.opengis.net/spec/geosparql/1.0> ;
                                                  rdfs:label "Well-known Text Literal"@en ;
                                                  <http://www.w3.org/2004/02/skos/core#definition> """
      A Well-known Text serialization of a geometry object.
    """@en ;
                                                  <http://www.w3.org/2004/02/skos/core#prefLabel> "Well-known Text Literal"@en .


#################################################################
#    Object Properties
#################################################################

###  http://www.opengis.net/ont/geosparql#defaultGeometry
<http://www.opengis.net/ont/geosparql#defaultGeometry> rdf:type owl:ObjectProperty ;
                                                       rdfs:subPropertyOf <http://www.opengis.net/ont/geosparql#hasGeometry> ;
                                                       rdfs:domain <http://www.opengis.net/ont/geosparql#Feature> ;
                                                       rdfs:range <http://www.opengis.net/ont/geosparql#Geometry> ;
                                                       <http://purl.org/dc/elements/1.1/contributor> "Matthew Perry" ;
                                                       <http://purl.org/dc/elements/1.1/creator> "OGC GeoSPARQL 1.0 Standard Working Group" ;
                                                       <http://purl.org/dc/elements/1.1/date> "2011-06-16"^^xsd:date ;
                                                       <http://purl.org/dc/elements/1.1/description> """
      The default geometry to be used in spatial calculations.
      It is Usually the most detailed geometry.
    """@en ;
                                                       rdfs:comment """
      The default geometry to be used in spatial calculations.
      It is Usually the most detailed geometry.
    """@en ;
                                                       rdfs:isDefinedBy <http://www.opengis.net/ont/geosparql> ,
                                                                        <http://www.opengis.net/spec/geosparql/1.0> ;
                                                       rdfs:label "defaultGeometry"@en ;
                                                       <http://www.w3.org/2004/02/skos/core#definition> """
      The default geometry to be used in spatial calculations.
      It is Usually the most detailed geometry.
    """@en ;
                                                       <http://www.w3.org/2004/02/skos/core#prefLabel> "defaultGeometry"@en .


###  http://www.opengis.net/ont/geosparql#ehContains
<http://www.opengis.net/ont/geosparql#ehContains> rdf:type owl:ObjectProperty ;
                                                  rdfs:domain <http://www.opengis.net/ont/geosparql#SpatialObject> ;
                                                  rdfs:range <http://www.opengis.net/ont/geosparql#SpatialObject> ;
                                                  <http://purl.org/dc/elements/1.1/contributor> "Matthew Perry" ;
                                                  <http://purl.org/dc/elements/1.1/creator> "OGC GeoSPARQL 1.0 Standard Working Group" ;
                                                  <http://purl.org/dc/elements/1.1/date> "2011-06-16"^^xsd:date ;
                                                  <http://purl.org/dc/elements/1.1/description> """
      Exists if the subject SpatialObject spatially contains the 
      object SpatialObject. DE-9IM: T*TFF*FF*
    """@en ;
                                                  rdfs:comment """
      Exists if the subject SpatialObject spatially contains the 
      object SpatialObject. DE-9IM: T*TFF*FF*
    """@en ;
                                                  rdfs:isDefinedBy <http://www.opengis.net/ont/geosparql> ,
                                                                   <http://www.opengis.net/spec/geosparql/1.0> ;
                                                  rdfs:label "contains"@en ;
                                                  <http://www.w3.org/2004/02/skos/core#definition> """
      Exists if the subject SpatialObject spatially contains the 
      object SpatialObject. DE-9IM: T*TFF*FF*
    """@en ;
                                                  <http://www.w3.org/2004/02/skos/core#prefLabel> "contains"@en .


###  http://www.opengis.net/ont/geosparql#ehCoveredBy
<http://www.opengis.net/ont/geosparql#ehCoveredBy> rdf:type owl:ObjectProperty ;
                                                   rdfs:domain <http://www.opengis.net/ont/geosparql#SpatialObject> ;
                                                   rdfs:range <http://www.opengis.net/ont/geosparql#SpatialObject> ;
                                                   <http://purl.org/dc/elements/1.1/contributor> "Matthew Perry" ;
                                                   <http://purl.org/dc/elements/1.1/creator> "OGC GeoSPARQL 1.0 Standard Working Group" ;
                                                   <http://purl.org/dc/elements/1.1/date> "2011-06-16"^^xsd:date ;
                                                   <http://purl.org/dc/elements/1.1/description> """
      Exists if the subject SpatialObject is spatially covered 
      by the object SpatialObject. DE-9IM: TFF*TFT**
    """@en ;
                                                   rdfs:comment """
      Exists if the subject SpatialObject is spatially covered 
      by the object SpatialObject. DE-9IM: TFF*TFT**
    """@en ;
                                                   rdfs:isDefinedBy <http://www.opengis.net/ont/geosparql> ,
                                                                    <http://www.opengis.net/spec/geosparql/1.0> ;
                                                   rdfs:label "coveredBy"@en ;
                                                   <http://www.w3.org/2004/02/skos/core#definition> """
      Exists if the subject SpatialObject is spatially covered 
      by the object SpatialObject. DE-9IM: TFF*TFT**
    """@en ;
                                                   <http://www.w3.org/2004/02/skos/core#prefLabel> "coveredBy"@en .


###  http://www.opengis.net/ont/geosparql#ehCovers
<http://www.opengis.net/ont/geosparql#ehCovers> rdf:type owl:ObjectProperty ;
                                                rdfs:domain <http://www.opengis.net/ont/geosparql#SpatialObject> ;
                                                rdfs:range <http://www.opengis.net/ont/geosparql#SpatialObject> ;
                                                <http://purl.org/dc/elements/1.1/contributor> "Matthew Perry" ;
                                                <http://purl.org/dc/elements/1.1/creator> "OGC GeoSPARQL 1.0 Standard Working Group" ;
                                                <http://purl.org/dc/elements/1.1/date> "2011-06-16"^^xsd:date ;
                                                <http://purl.org/dc/elements/1.1/description> """
      Exists if the subject SpatialObject spatially covers the 
      object SpatialObject. DE-9IM: T*TFT*FF*
    """@en ;
                                                rdfs:comment """
      Exists if the subject SpatialObject spatially covers the 
      object SpatialObject. DE-9IM: T*TFT*FF*
    """@en ;
                                                rdfs:isDefinedBy <http://www.opengis.net/ont/geosparql> ,
                                                                 <http://www.opengis.net/spec/geosparql/1.0> ;
                                                rdfs:label "covers"@en ;
                                                <http://www.w3.org/2004/02/skos/core#definition> """
      Exists if the subject SpatialObject spatially covers the 
      object SpatialObject. DE-9IM: T*TFT*FF*
    """@en ;
                                                <http://www.w3.org/2004/02/skos/core#prefLabel> "covers"@en .


###  http://www.opengis.net/ont/geosparql#ehDisjoint
<http://www.opengis.net/ont/geosparql#ehDisjoint> rdf:type owl:ObjectProperty ;
                                                  rdfs:domain <http://www.opengis.net/ont/geosparql#SpatialObject> ;
                                                  rdfs:range <http://www.opengis.net/ont/geosparql#SpatialObject> ;
                                                  <http://purl.org/dc/elements/1.1/contributor> "Matthew Perry" ;
                                                  <http://purl.org/dc/elements/1.1/creator> "OGC GeoSPARQL 1.0 Standard Working Group" ;
                                                  <http://purl.org/dc/elements/1.1/date> "2011-06-16"^^xsd:date ;
                                                  <http://purl.org/dc/elements/1.1/description> """
      Exists if the subject SpatialObject is spatially disjoint
      from the object SpatialObject. DE-9IM: FF*FF****
    """@en ;
                                                  rdfs:comment """
      Exists if the subject SpatialObject is spatially disjoint
      from the object SpatialObject. DE-9IM: FF*FF****
    """@en ;
                                                  rdfs:isDefinedBy <http://www.opengis.net/ont/geosparql> ,
                                                                   <http://www.opengis.net/spec/geosparql/1.0> ;
                                                  rdfs:label "disjoint"@en ;
                                                  <http://www.w3.org/2004/02/skos/core#definition> """
      Exists if the subject SpatialObject is spatially disjoint
      from the object SpatialObject. DE-9IM: FF*FF****
    """@en ;
                                                  <http://www.w3.org/2004/02/skos/core#prefLabel> "disjoint"@en .


###  http://www.opengis.net/ont/geosparql#ehEquals
<http://www.opengis.net/ont/geosparql#ehEquals> rdf:type owl:ObjectProperty ;
                                                rdfs:domain <http://www.opengis.net/ont/geosparql#SpatialObject> ;
                                                rdfs:range <http://www.opengis.net/ont/geosparql#SpatialObject> ;
                                                <http://purl.org/dc/elements/1.1/contributor> "Matthew Perry" ;
                                                <http://purl.org/dc/elements/1.1/creator> "OGC GeoSPARQL 1.0 Standard Working Group" ;
                                                <http://purl.org/dc/elements/1.1/date> "2011-06-16"^^xsd:date ;
                                                <http://purl.org/dc/elements/1.1/description> """
      Exists if the subject SpatialObject spatially equals the 
      object SpatialObject. DE-9IM: TFFFTFFFT
    """@en ;
                                                rdfs:comment """
      Exists if the subject SpatialObject spatially equals the 
      object SpatialObject. DE-9IM: TFFFTFFFT
    """@en ;
                                                rdfs:isDefinedBy <http://www.opengis.net/ont/geosparql> ,
                                                                 <http://www.opengis.net/spec/geosparql/1.0> ;
                                                rdfs:label "equals"@en ;
                                                <http://www.w3.org/2004/02/skos/core#definition> """
      Exists if the subject SpatialObject spatially equals the 
      object SpatialObject. DE-9IM: TFFFTFFFT
    """@en ;
                                                <http://www.w3.org/2004/02/skos/core#prefLabel> "equals"@en .


###  http://www.opengis.net/ont/geosparql#ehInside
<http://www.opengis.net/ont/geosparql#ehInside> rdf:type owl:ObjectProperty ;
                                                rdfs:domain <http://www.opengis.net/ont/geosparql#SpatialObject> ;
                                                rdfs:range <http://www.opengis.net/ont/geosparql#SpatialObject> ;
                                                <http://purl.org/dc/elements/1.1/contributor> "Matthew Perry" ;
                                                <http://purl.org/dc/elements/1.1/creator> "OGC GeoSPARQL 1.0 Standard Working Group" ;
                                                <http://purl.org/dc/elements/1.1/date> "2011-06-16"^^xsd:date ;
                                                <http://purl.org/dc/elements/1.1/description> """
      Exists if the subject SpatialObject is spatially inside 
      the object SpatialObject. DE-9IM: TFF*FFT**
    """@en ;
                                                rdfs:comment """
      Exists if the subject SpatialObject is spatially inside 
      the object SpatialObject. DE-9IM: TFF*FFT**
    """@en ;
                                                rdfs:isDefinedBy <http://www.opengis.net/ont/geosparql> ,
                                                                 <http://www.opengis.net/spec/geosparql/1.0> ;
                                                rdfs:label "inside"@en ;
                                                <http://www.w3.org/2004/02/skos/core#definition> """
      Exists if the subject SpatialObject is spatially inside 
      the object SpatialObject. DE-9IM: TFF*FFT**
    """@en ;
                                                <http://www.w3.org/2004/02/skos/core#prefLabel> "inside"@en .


###  http://www.opengis.net/ont/geosparql#ehMeet
<http://www.opengis.net/ont/geosparql#ehMeet> rdf:type owl:ObjectProperty ;
                                              rdfs:domain <http://www.opengis.net/ont/geosparql#SpatialObject> ;
                                              rdfs:range <http://www.opengis.net/ont/geosparql#SpatialObject> ;
                                              <http://purl.org/dc/elements/1.1/contributor> "Matthew Perry" ;
                                              <http://purl.org/dc/elements/1.1/creator> "OGC GeoSPARQL 1.0 Standard Working Group" ;
                                              <http://purl.org/dc/elements/1.1/date> "2011-06-16"^^xsd:date ;
                                              <http://purl.org/dc/elements/1.1/description> """
      Exists if the subject SpatialObject spatially meets the 
      object SpatialObject. 
      DE-9IM: FT******* ^ F**T***** ^ F***T****
    """@en ;
                                              rdfs:comment """
      Exists if the subject SpatialObject spatially meets the 
      object SpatialObject. 
      DE-9IM: FT******* ^ F**T***** ^ F***T****
    """@en ;
                                              rdfs:isDefinedBy <http://www.opengis.net/ont/geosparql> ,
                                                               <http://www.opengis.net/spec/geosparql/1.0> ;
                                              rdfs:label "meet"@en ;
                                              <http://www.w3.org/2004/02/skos/core#definition> """
      Exists if the subject SpatialObject spatially meets the 
      object SpatialObject. 
      DE-9IM: FT******* ^ F**T***** ^ F***T****
    """@en ;
                                              <http://www.w3.org/2004/02/skos/core#prefLabel> "meet"@en .


###  http://www.opengis.net/ont/geosparql#ehOverlap
<http://www.opengis.net/ont/geosparql#ehOverlap> rdf:type owl:ObjectProperty ;
                                                 rdfs:domain <http://www.opengis.net/ont/geosparql#SpatialObject> ;
                                                 rdfs:range <http://www.opengis.net/ont/geosparql#SpatialObject> ;
                                                 <http://purl.org/dc/elements/1.1/contributor> "Matthew Perry" ;
                                                 <http://purl.org/dc/elements/1.1/creator> "OGC GeoSPARQL 1.0 Standard Working Group" ;
                                                 <http://purl.org/dc/elements/1.1/date> "2011-06-16"^^xsd:date ;
                                                 <http://purl.org/dc/elements/1.1/description> """
      Exists if the subject SpatialObject spatially overlaps the 
      object SpatialObject. DE-9IM: T*T***T**
    """@en ;
                                                 rdfs:comment """
      Exists if the subject SpatialObject spatially overlaps the 
      object SpatialObject. DE-9IM: T*T***T**
    """@en ;
                                                 rdfs:isDefinedBy <http://www.opengis.net/ont/geosparql> ,
                                                                  <http://www.opengis.net/spec/geosparql/1.0> ;
                                                 rdfs:label "overlap"@en ;
                                                 <http://www.w3.org/2004/02/skos/core#definition> """
      Exists if the subject SpatialObject spatially overlaps the 
      object SpatialObject. DE-9IM: T*T***T**
    """@en ;
                                                 <http://www.w3.org/2004/02/skos/core#prefLabel> "overlap"@en .


###  http://www.opengis.net/ont/geosparql#hasGeometry
<http://www.opengis.net/ont/geosparql#hasGeometry> rdf:type owl:ObjectProperty ;
                                                   rdfs:domain <http://www.opengis.net/ont/geosparql#Feature> ;
                                                   rdfs:range <http://www.opengis.net/ont/geosparql#Geometry> ;
                                                   <http://purl.org/dc/elements/1.1/contributor> "Matthew Perry" ;
                                                   <http://purl.org/dc/elements/1.1/creator> "OGC GeoSPARQL 1.0 Standard Working Group" ;
                                                   <http://purl.org/dc/elements/1.1/date> "2011-06-16"^^xsd:date ;
                                                   <http://purl.org/dc/elements/1.1/description> """
      A spatial representation for a given feature.
    """@en ;
                                                   rdfs:comment """
      A spatial representation for a given feature.
    """@en ;
                                                   rdfs:isDefinedBy <http://www.opengis.net/ont/geosparql> ,
                                                                    <http://www.opengis.net/spec/geosparql/1.0> ;
                                                   rdfs:label "hasGeometry"@en ;
                                                   <http://www.w3.org/2004/02/skos/core#definition> """
      A spatial representation for a given feature.
    """@en ;
                                                   <http://www.w3.org/2004/02/skos/core#prefLabel> "hasGeometry"@en .


###  http://www.opengis.net/ont/geosparql#rcc8dc
<http://www.opengis.net/ont/geosparql#rcc8dc> rdf:type owl:ObjectProperty ;
                                              rdfs:domain <http://www.opengis.net/ont/geosparql#SpatialObject> ;
                                              rdfs:range <http://www.opengis.net/ont/geosparql#SpatialObject> ;
                                              <http://purl.org/dc/elements/1.1/contributor> "Matthew Perry" ;
                                              <http://purl.org/dc/elements/1.1/creator> "OGC GeoSPARQL 1.0 Standard Working Group" ;
                                              <http://purl.org/dc/elements/1.1/date> "2011-06-16"^^xsd:date ;
                                              <http://purl.org/dc/elements/1.1/description> """
      Exists if the subject SpatialObject is spatially disjoint
      from the object SpatialObject. DE-9IM: FFTFFTTTT
    """@en ;
                                              rdfs:comment """
      Exists if the subject SpatialObject is spatially disjoint
      from the object SpatialObject. DE-9IM: FFTFFTTTT
    """@en ;
                                              rdfs:isDefinedBy <http://www.opengis.net/ont/geosparql> ,
                                                               <http://www.opengis.net/spec/geosparql/1.0> ;
                                              rdfs:label "disconnected"@en ;
                                              <http://www.w3.org/2004/02/skos/core#definition> """
      Exists if the subject SpatialObject is spatially disjoint
      from the object SpatialObject. DE-9IM: FFTFFTTTT
    """@en ;
                                              <http://www.w3.org/2004/02/skos/core#prefLabel> "disconnected"@en .


###  http://www.opengis.net/ont/geosparql#rcc8ec
<http://www.opengis.net/ont/geosparql#rcc8ec> rdf:type owl:ObjectProperty ;
                                              rdfs:domain <http://www.opengis.net/ont/geosparql#SpatialObject> ;
                                              rdfs:range <http://www.opengis.net/ont/geosparql#SpatialObject> ;
                                              <http://purl.org/dc/elements/1.1/contributor> "Matthew Perry" ;
                                              <http://purl.org/dc/elements/1.1/creator> "OGC GeoSPARQL 1.0 Standard Working Group" ;
                                              <http://purl.org/dc/elements/1.1/date> "2011-06-16"^^xsd:date ;
                                              <http://purl.org/dc/elements/1.1/description> """
      Exists if the subject SpatialObject spatially meets the 
      object SpatialObject. DE-9IM: FFTFTTTTT
    """@en ;
                                              rdfs:comment """
      Exists if the subject SpatialObject spatially meets the 
      object SpatialObject. DE-9IM: FFTFTTTTT
    """@en ;
                                              rdfs:isDefinedBy <http://www.opengis.net/ont/geosparql> ,
                                                               <http://www.opengis.net/spec/geosparql/1.0> ;
                                              rdfs:label "externally connected"@en ;
                                              <http://www.w3.org/2004/02/skos/core#definition> """
      Exists if the subject SpatialObject spatially meets the 
      object SpatialObject. DE-9IM: FFTFTTTTT
    """@en ;
                                              <http://www.w3.org/2004/02/skos/core#prefLabel> "externally connected"@en .


###  http://www.opengis.net/ont/geosparql#rcc8eq
<http://www.opengis.net/ont/geosparql#rcc8eq> rdf:type owl:ObjectProperty ;
                                              rdfs:domain <http://www.opengis.net/ont/geosparql#SpatialObject> ;
                                              rdfs:range <http://www.opengis.net/ont/geosparql#SpatialObject> ;
                                              <http://purl.org/dc/elements/1.1/contributor> "Matthew Perry" ;
                                              <http://purl.org/dc/elements/1.1/creator> "OGC GeoSPARQL 1.0 Standard Working Group" ;
                                              <http://purl.org/dc/elements/1.1/date> "2011-06-16"^^xsd:date ;
                                              <http://purl.org/dc/elements/1.1/description> """
      Exists if the subject SpatialObject spatially equals the 
      object SpatialObject. DE-9IM: TFFFTFFFT
    """@en ;
                                              rdfs:comment """
      Exists if the subject SpatialObject spatially equals the 
      object SpatialObject. DE-9IM: TFFFTFFFT
    """@en ;
                                              rdfs:isDefinedBy <http://www.opengis.net/ont/geosparql> ,
                                                               <http://www.opengis.net/spec/geosparql/1.0> ;
                                              rdfs:label "equals"@en ;
                                              <http://www.w3.org/2004/02/skos/core#definition> """
      Exists if the subject SpatialObject spatially equals the 
      object SpatialObject. DE-9IM: TFFFTFFFT
    """@en ;
                                              <http://www.w3.org/2004/02/skos/core#prefLabel> "equals"@en .


###  http://www.opengis.net/ont/geosparql#rcc8ntpp
<http://www.opengis.net/ont/geosparql#rcc8ntpp> rdf:type owl:ObjectProperty ;
                                                rdfs:domain <http://www.opengis.net/ont/geosparql#SpatialObject> ;
                                                rdfs:range <http://www.opengis.net/ont/geosparql#SpatialObject> ;
                                                <http://purl.org/dc/elements/1.1/contributor> "Matthew Perry" ;
                                                <http://purl.org/dc/elements/1.1/creator> "OGC GeoSPARQL 1.0 Standard Working Group" ;
                                                <http://purl.org/dc/elements/1.1/date> "2011-06-16"^^xsd:date ;
                                                <http://purl.org/dc/elements/1.1/description> """
      Exists if the subject SpatialObject is spatially inside 
      the object SpatialObject. DE-9IM: TFFTFFTTT
    """@en ;
                                                rdfs:comment """
      Exists if the subject SpatialObject is spatially inside 
      the object SpatialObject. DE-9IM: TFFTFFTTT
    """@en ;
                                                rdfs:isDefinedBy <http://www.opengis.net/ont/geosparql> ,
                                                                 <http://www.opengis.net/spec/geosparql/1.0> ;
                                                rdfs:label "non-tangential proper part"@en ;
                                                <http://www.w3.org/2004/02/skos/core#definition> """
      Exists if the subject SpatialObject is spatially inside 
      the object SpatialObject. DE-9IM: TFFTFFTTT
    """@en ;
                                                <http://www.w3.org/2004/02/skos/core#prefLabel> "non-tangential proper part"@en .


###  http://www.opengis.net/ont/geosparql#rcc8ntppi
<http://www.opengis.net/ont/geosparql#rcc8ntppi> rdf:type owl:ObjectProperty ;
                                                 rdfs:domain <http://www.opengis.net/ont/geosparql#SpatialObject> ;
                                                 rdfs:range <http://www.opengis.net/ont/geosparql#SpatialObject> ;
                                                 <http://purl.org/dc/elements/1.1/contributor> "Matthew Perry" ;
                                                 <http://purl.org/dc/elements/1.1/creator> "OGC GeoSPARQL 1.0 Standard Working Group" ;
                                                 <http://purl.org/dc/elements/1.1/date> "2011-06-16"^^xsd:date ;
                                                 <http://purl.org/dc/elements/1.1/description> """
      Exists if the subject SpatialObject spatially contains the 
      object SpatialObject. DE-9IM: TTTFFTFFT
    """@en ;
                                                 rdfs:comment """
      Exists if the subject SpatialObject spatially contains the 
      object SpatialObject. DE-9IM: TTTFFTFFT
    """@en ;
                                                 rdfs:isDefinedBy <http://www.opengis.net/ont/geosparql> ,
                                                                  <http://www.opengis.net/spec/geosparql/1.0> ;
                                                 rdfs:label "non-tangential proper part inverse"@en ;
                                                 <http://www.w3.org/2004/02/skos/core#definition> """
      Exists if the subject SpatialObject spatially contains the 
      object SpatialObject. DE-9IM: TTTFFTFFT
    """@en ;
                                                 <http://www.w3.org/2004/02/skos/core#prefLabel> "non-tangential proper part inverse"@en .


###  http://www.opengis.net/ont/geosparql#rcc8po
<http://www.opengis.net/ont/geosparql#rcc8po> rdf:type owl:ObjectProperty ;
                                              rdfs:domain <http://www.opengis.net/ont/geosparql#SpatialObject> ;
                                              rdfs:range <http://www.opengis.net/ont/geosparql#SpatialObject> ;
                                              <http://purl.org/dc/elements/1.1/contributor> "Matthew Perry" ;
                                              <http://purl.org/dc/elements/1.1/creator> "OGC GeoSPARQL 1.0 Standard Working Group" ;
                                              <http://purl.org/dc/elements/1.1/date> "2011-06-16"^^xsd:date ;
                                              <http://purl.org/dc/elements/1.1/description> """
      Exists if the subject SpatialObject spatially overlaps the 
      object SpatialObject. DE-9IM: TTTTTTTTT
    """@en ;
                                              rdfs:comment """
      Exists if the subject SpatialObject spatially overlaps the 
      object SpatialObject. DE-9IM: TTTTTTTTT
    """@en ;
                                              rdfs:isDefinedBy <http://www.opengis.net/ont/geosparql> ,
                                                               <http://www.opengis.net/spec/geosparql/1.0> ;
                                              rdfs:label "partially overlapping"@en ;
                                              <http://www.w3.org/2004/02/skos/core#definition> """
      Exists if the subject SpatialObject spatially overlaps the 
      object SpatialObject. DE-9IM: TTTTTTTTT
    """@en ;
                                              <http://www.w3.org/2004/02/skos/core#prefLabel> "partially overlapping"@en .


###  http://www.opengis.net/ont/geosparql#rcc8tpp
<http://www.opengis.net/ont/geosparql#rcc8tpp> rdf:type owl:ObjectProperty ;
                                               rdfs:domain <http://www.opengis.net/ont/geosparql#SpatialObject> ;
                                               rdfs:range <http://www.opengis.net/ont/geosparql#SpatialObject> ;
                                               <http://purl.org/dc/elements/1.1/contributor> "Matthew Perry" ;
                                               <http://purl.org/dc/elements/1.1/creator> "OGC GeoSPARQL 1.0 Standard Working Group" ;
                                               <http://purl.org/dc/elements/1.1/date> "2011-06-16"^^xsd:date ;
                                               <http://purl.org/dc/elements/1.1/description> """
      Exists if the subject SpatialObject is spatially covered 
      by the object SpatialObject. DE-9IM: TFFTTFTTT
    """@en ;
                                               rdfs:comment """
      Exists if the subject SpatialObject is spatially covered 
      by the object SpatialObject. DE-9IM: TFFTTFTTT
    """@en ;
                                               rdfs:isDefinedBy <http://www.opengis.net/ont/geosparql> ,
                                                                <http://www.opengis.net/spec/geosparql/1.0> ;
                                               rdfs:label "tangential proper part"@en ;
                                               <http://www.w3.org/2004/02/skos/core#definition> """
      Exists if the subject SpatialObject is spatially covered 
      by the object SpatialObject. DE-9IM: TFFTTFTTT
    """@en ;
                                               <http://www.w3.org/2004/02/skos/core#prefLabel> "tangential proper part"@en .


###  http://www.opengis.net/ont/geosparql#rcc8tppi
<http://www.opengis.net/ont/geosparql#rcc8tppi> rdf:type owl:ObjectProperty ;
                                                rdfs:domain <http://www.opengis.net/ont/geosparql#SpatialObject> ;
                                                rdfs:range <http://www.opengis.net/ont/geosparql#SpatialObject> ;
                                                <http://purl.org/dc/elements/1.1/contributor> "Matthew Perry" ;
                                                <http://purl.org/dc/elements/1.1/creator> "OGC GeoSPARQL 1.0 Standard Working Group" ;
                                                <http://purl.org/dc/elements/1.1/date> "2011-06-16"^^xsd:date ;
                                                <http://purl.org/dc/elements/1.1/description> """
      Exists if the subject SpatialObject spatially covers the 
      object SpatialObject. DE-9IM: TTTFTTFFT
    """@en ;
                                                rdfs:comment """
      Exists if the subject SpatialObject spatially covers the 
      object SpatialObject. DE-9IM: TTTFTTFFT
    """@en ;
                                                rdfs:isDefinedBy <http://www.opengis.net/ont/geosparql> ,
                                                                 <http://www.opengis.net/spec/geosparql/1.0> ;
                                                rdfs:label "tangential proper part inverse"@en ;
                                                <http://www.w3.org/2004/02/skos/core#definition> """
      Exists if the subject SpatialObject spatially covers the 
      object SpatialObject. DE-9IM: TTTFTTFFT
    """@en ;
                                                <http://www.w3.org/2004/02/skos/core#prefLabel> "tangential proper part inverse"@en .


###  http://www.opengis.net/ont/geosparql#sfContains
<http://www.opengis.net/ont/geosparql#sfContains> rdf:type owl:ObjectProperty ;
                                                  rdfs:domain <http://www.opengis.net/ont/geosparql#SpatialObject> ;
                                                  rdfs:range <http://www.opengis.net/ont/geosparql#SpatialObject> ;
                                                  <http://purl.org/dc/elements/1.1/contributor> "Matthew Perry" ;
                                                  <http://purl.org/dc/elements/1.1/creator> "OGC GeoSPARQL 1.0 Standard Working Group" ;
                                                  <http://purl.org/dc/elements/1.1/date> "2011-06-16"^^xsd:date ;
                                                  <http://purl.org/dc/elements/1.1/description> """
      Exists if the subject SpatialObject spatially contains the 
      object SpatialObject. DE-9IM: T*****FF*
    """@en ;
                                                  rdfs:comment """
      Exists if the subject SpatialObject spatially contains the 
      object SpatialObject. DE-9IM: T*****FF*
    """@en ;
                                                  rdfs:isDefinedBy <http://www.opengis.net/ont/geosparql> ,
                                                                   <http://www.opengis.net/spec/geosparql/1.0> ;
                                                  rdfs:label "contains"@en ;
                                                  <http://www.w3.org/2004/02/skos/core#definition> """
      Exists if the subject SpatialObject spatially contains the 
      object SpatialObject. DE-9IM: T*****FF*
    """@en ;
                                                  <http://www.w3.org/2004/02/skos/core#prefLabel> "contains"@en .


###  http://www.opengis.net/ont/geosparql#sfCrosses
<http://www.opengis.net/ont/geosparql#sfCrosses> rdf:type owl:ObjectProperty ;
                                                 rdfs:domain <http://www.opengis.net/ont/geosparql#SpatialObject> ;
                                                 rdfs:range <http://www.opengis.net/ont/geosparql#SpatialObject> ;
                                                 <http://purl.org/dc/elements/1.1/contributor> "Matthew Perry" ;
                                                 <http://purl.org/dc/elements/1.1/creator> "OGC GeoSPARQL 1.0 Standard Working Group" ;
                                                 <http://purl.org/dc/elements/1.1/date> "2011-06-16"^^xsd:date ;
                                                 <http://purl.org/dc/elements/1.1/description> """
      Exists if the subject SpatialObject spatially crosses the 
      object SpatialObject. DE-9IM: T*T******
    """@en ;
                                                 rdfs:comment """
      Exists if the subject SpatialObject spatially crosses the 
      object SpatialObject. DE-9IM: T*T******
    """@en ;
                                                 rdfs:isDefinedBy <http://www.opengis.net/ont/geosparql> ,
                                                                  <http://www.opengis.net/spec/geosparql/1.0> ;
                                                 rdfs:label "crosses"@en ;
                                                 <http://www.w3.org/2004/02/skos/core#definition> """
      Exists if the subject SpatialObject spatially crosses the 
      object SpatialObject. DE-9IM: T*T******
    """@en ;
                                                 <http://www.w3.org/2004/02/skos/core#prefLabel> "crosses"@en .


###  http://www.opengis.net/ont/geosparql#sfDisjoint
<http://www.opengis.net/ont/geosparql#sfDisjoint> rdf:type owl:ObjectProperty ;
                                                  rdfs:domain <http://www.opengis.net/ont/geosparql#SpatialObject> ;
                                                  rdfs:range <http://www.opengis.net/ont/geosparql#SpatialObject> ;
                                                  <http://purl.org/dc/elements/1.1/contributor> "Matthew Perry" ;
                                                  <http://purl.org/dc/elements/1.1/creator> "OGC GeoSPARQL 1.0 Standard Working Group" ;
                                                  <http://purl.org/dc/elements/1.1/date> "2011-06-16"^^xsd:date ;
                                                  <http://purl.org/dc/elements/1.1/description> """
      Exists if the subject SpatialObject is spatially disjoint 
      from the object SpatialObject. DE-9IM: FF*FF****
    """@en ;
                                                  rdfs:comment """
      Exists if the subject SpatialObject is spatially disjoint 
      from the object SpatialObject. DE-9IM: FF*FF****
    """@en ;
                                                  rdfs:isDefinedBy <http://www.opengis.net/ont/geosparql> ,
                                                                   <http://www.opengis.net/spec/geosparql/1.0> ;
                                                  rdfs:label "disjoint"@en ;
                                                  <http://www.w3.org/2004/02/skos/core#definition> """
      Exists if the subject SpatialObject is spatially disjoint 
      from the object SpatialObject. DE-9IM: FF*FF****
    """@en ;
                                                  <http://www.w3.org/2004/02/skos/core#prefLabel> "disjoint"@en .


###  http://www.opengis.net/ont/geosparql#sfEquals
<http://www.opengis.net/ont/geosparql#sfEquals> rdf:type owl:ObjectProperty ;
                                                rdfs:domain <http://www.opengis.net/ont/geosparql#SpatialObject> ;
                                                rdfs:range <http://www.opengis.net/ont/geosparql#SpatialObject> ;
                                                <http://purl.org/dc/elements/1.1/contributor> "Matthew Perry" ;
                                                <http://purl.org/dc/elements/1.1/creator> "OGC GeoSPARQL 1.0 Standard Working Group" ;
                                                <http://purl.org/dc/elements/1.1/date> "2011-06-16"^^xsd:date ;
                                                <http://purl.org/dc/elements/1.1/description> """
      Exists if the subject SpatialObject spatially equals the 
      object SpatialObject. DE-9IM: TFFFTFFFT
    """@en ;
                                                rdfs:comment """
      Exists if the subject SpatialObject spatially equals the 
      object SpatialObject. DE-9IM: TFFFTFFFT
    """@en ;
                                                rdfs:isDefinedBy <http://www.opengis.net/ont/geosparql> ,
                                                                 <http://www.opengis.net/spec/geosparql/1.0> ;
                                                rdfs:label "equals"@en ;
                                                <http://www.w3.org/2004/02/skos/core#definition> """
      Exists if the subject SpatialObject spatially equals the 
      object SpatialObject. DE-9IM: TFFFTFFFT
    """@en ;
                                                <http://www.w3.org/2004/02/skos/core#prefLabel> "equals"@en .


###  http://www.opengis.net/ont/geosparql#sfIntersects
<http://www.opengis.net/ont/geosparql#sfIntersects> rdf:type owl:ObjectProperty ;
                                                    rdfs:domain <http://www.opengis.net/ont/geosparql#SpatialObject> ;
                                                    rdfs:range <http://www.opengis.net/ont/geosparql#SpatialObject> ;
                                                    <http://purl.org/dc/elements/1.1/contributor> "Matthew Perry" ;
                                                    <http://purl.org/dc/elements/1.1/creator> "OGC GeoSPARQL 1.0 Standard Working Group" ;
                                                    <http://purl.org/dc/elements/1.1/date> "2011-06-16"^^xsd:date ;
                                                    <http://purl.org/dc/elements/1.1/description> """
      Exists if the subject SpatialObject is not spatially disjoint 
      from the object SpatialObject.
      DE-9IM: T******** ^ *T******* ^ ***T***** ^ ****T**** 
    """@en ;
                                                    rdfs:comment """
      Exists if the subject SpatialObject is not spatially disjoint 
      from the object SpatialObject.
      DE-9IM: T******** ^ *T******* ^ ***T***** ^ ****T**** 
    """@en ;
                                                    rdfs:isDefinedBy <http://www.opengis.net/ont/geosparql> ,
                                                                     <http://www.opengis.net/spec/geosparql/1.0> ;
                                                    rdfs:label "intersects"@en ;
                                                    <http://www.w3.org/2004/02/skos/core#definition> """
      Exists if the subject SpatialObject is not spatially disjoint 
      from the object SpatialObject.
      DE-9IM: T******** ^ *T******* ^ ***T***** ^ ****T**** 
    """@en ;
                                                    <http://www.w3.org/2004/02/skos/core#prefLabel> "intersects"@en .


###  http://www.opengis.net/ont/geosparql#sfOverlaps
<http://www.opengis.net/ont/geosparql#sfOverlaps> rdf:type owl:ObjectProperty ;
                                                  rdfs:domain <http://www.opengis.net/ont/geosparql#SpatialObject> ;
                                                  rdfs:range <http://www.opengis.net/ont/geosparql#SpatialObject> ;
                                                  <http://purl.org/dc/elements/1.1/contributor> "Matthew Perry" ;
                                                  <http://purl.org/dc/elements/1.1/creator> "OGC GeoSPARQL 1.0 Standard Working Group" ;
                                                  <http://purl.org/dc/elements/1.1/date> "2011-06-16"^^xsd:date ;
                                                  <http://purl.org/dc/elements/1.1/description> """
      Exists if the subject SpatialObject spatially overlaps the 
      object SpatialObject. DE-9IM: T*T***T** 
    """@en ;
                                                  rdfs:comment """
      Exists if the subject SpatialObject spatially overlaps the 
      object SpatialObject. DE-9IM: T*T***T** 
    """@en ;
                                                  rdfs:isDefinedBy <http://www.opengis.net/ont/geosparql> ,
                                                                   <http://www.opengis.net/spec/geosparql/1.0> ;
                                                  rdfs:label "overlaps"@en ;
                                                  <http://www.w3.org/2004/02/skos/core#definition> """
      Exists if the subject SpatialObject spatially overlaps the 
      object SpatialObject. DE-9IM: T*T***T** 
    """@en ;
                                                  <http://www.w3.org/2004/02/skos/core#prefLabel> "overlaps"@en .


###  http://www.opengis.net/ont/geosparql#sfTouches
<http://www.opengis.net/ont/geosparql#sfTouches> rdf:type owl:ObjectProperty ;
                                                 rdfs:domain <http://www.opengis.net/ont/geosparql#SpatialObject> ;
                                                 rdfs:range <http://www.opengis.net/ont/geosparql#SpatialObject> ;
                                                 <http://purl.org/dc/elements/1.1/contributor> "Matthew Perry" ;
                                                 <http://purl.org/dc/elements/1.1/creator> "OGC GeoSPARQL 1.0 Standard Working Group" ;
                                                 <http://purl.org/dc/elements/1.1/date> "2011-06-16"^^xsd:date ;
                                                 <http://purl.org/dc/elements/1.1/description> """
      Exists if the subject SpatialObject spatially touches the 
      object SpatialObject.
      DE-9IM: FT******* ^ F**T***** ^ F***T****
    """@en ;
                                                 rdfs:comment """
      Exists if the subject SpatialObject spatially touches the 
      object SpatialObject.
      DE-9IM: FT******* ^ F**T***** ^ F***T****
    """@en ;
                                                 rdfs:isDefinedBy <http://www.opengis.net/ont/geosparql> ,
                                                                  <http://www.opengis.net/spec/geosparql/1.0> ;
                                                 rdfs:label "touches"@en ;
                                                 <http://www.w3.org/2004/02/skos/core#definition> """
      Exists if the subject SpatialObject spatially touches the 
      object SpatialObject.
      DE-9IM: FT******* ^ F**T***** ^ F***T****
    """@en ;
                                                 <http://www.w3.org/2004/02/skos/core#prefLabel> "touches"@en .


###  http://www.opengis.net/ont/geosparql#sfWithin
<http://www.opengis.net/ont/geosparql#sfWithin> rdf:type owl:ObjectProperty ;
                                                rdfs:domain <http://www.opengis.net/ont/geosparql#SpatialObject> ;
                                                rdfs:range <http://www.opengis.net/ont/geosparql#SpatialObject> ;
                                                <http://purl.org/dc/elements/1.1/contributor> "Matthew Perry" ;
                                                <http://purl.org/dc/elements/1.1/creator> "OGC GeoSPARQL 1.0 Standard Working Group" ;
                                                <http://purl.org/dc/elements/1.1/date> "2011-06-16"^^xsd:date ;
                                                <http://purl.org/dc/elements/1.1/description> """
      Exists if the subject SpatialObject is spatially within the 
      object SpatialObject. DE-9IM: T*F**F***
    """@en ;
                                                rdfs:comment """
      Exists if the subject SpatialObject is spatially within the 
      object SpatialObject. DE-9IM: T*F**F***
    """@en ;
                                                rdfs:isDefinedBy <http://www.opengis.net/ont/geosparql> ,
                                                                 <http://www.opengis.net/spec/geosparql/1.0> ;
                                                rdfs:label "within"@en ;
                                                <http://www.w3.org/2004/02/skos/core#definition> """
      Exists if the subject SpatialObject is spatially within the 
      object SpatialObject. DE-9IM: T*F**F***
    """@en ;
                                                <http://www.w3.org/2004/02/skos/core#prefLabel> "within"@en .


###  https://w3id.org/latuli/ontology/m3#belongsToShipment
:belongsToShipment rdf:type owl:ObjectProperty ;
                   rdfs:subPropertyOf owl:topObjectProperty ;
                   rdfs:range :Shipment ;
                   rdfs:comment "Relates a TradeItem or a ShipmentItem to a Shipment." .


###  https://w3id.org/latuli/ontology/m3#hasCarrierParty
:hasCarrierParty rdf:type owl:ObjectProperty ;
                 rdfs:subPropertyOf owl:topObjectProperty ;
                 rdfs:range :Carrier ;
                 rdfs:comment "Relates a Consignment or an XDocLoadingUnit (cross-dock loading unit) to a Carrier" .


###  https://w3id.org/latuli/ontology/m3#hasConsigneeParty
:hasConsigneeParty rdf:type owl:ObjectProperty ;
                   rdfs:subPropertyOf owl:topObjectProperty ;
                   rdfs:range :Consignee ;
                   rdfs:comment "Relates a Consignment or an XDocLoadingUnit (cross-dock loading unit) to a Consignee" .


###  https://w3id.org/latuli/ontology/m3#hasConsignorParty
:hasConsignorParty rdf:type owl:ObjectProperty ;
                   rdfs:subPropertyOf owl:topObjectProperty ;
                   rdfs:range :Consignor ;
                   rdfs:comment "Relates a Consignment or an XDocLoadingUnit (cross-dock loading unit) to a Consignor" .


###  https://w3id.org/latuli/ontology/m3#hasHubParty
:hasHubParty rdf:type owl:ObjectProperty ;
             rdfs:range :Party ;
             rdfs:comment "Relates a HubReconstructionLocation, an XDocLoadingUnit (cross-dock loading unit), a Wave, or a Transport to a TerminalOperator" .


###  https://w3id.org/latuli/ontology/m3#hasHubReconstructionLocation
:hasHubReconstructionLocation rdf:type owl:ObjectProperty ;
                              rdfs:range :HubReconstructionLocation ;
                              rdfs:comment "Relates an XDocLoadingUnit (cross-dock loading unit) to an HubReconstructionLocation" .


###  https://w3id.org/latuli/ontology/m3#hasHubReconstructionParty
:hasHubReconstructionParty rdf:type owl:ObjectProperty ;
                           rdfs:subPropertyOf owl:topObjectProperty ;
                           rdfs:range :Party .


###  https://w3id.org/latuli/ontology/m3#hasInboundConsignment
:hasInboundConsignment rdf:type owl:ObjectProperty ;
                       rdfs:subPropertyOf owl:topObjectProperty ;
                       rdfs:range :Consignment ;
                       rdfs:comment "Relates an XDocLoadingUnit (cross-dock loading unit) to an inbound Consignment" .


###  https://w3id.org/latuli/ontology/m3#hasInboundParentLoadingUnit
:hasInboundParentLoadingUnit rdf:type owl:ObjectProperty ;
                             rdfs:subPropertyOf owl:topObjectProperty ;
                             rdfs:range :LoadingUnit ;
                             rdfs:comment "Relates an XDocLoadingUnit (cross-dock loading unit) to an inbound parent LoadingUnit" .


###  https://w3id.org/latuli/ontology/m3#hasLoadingUnit
:hasLoadingUnit rdf:type owl:ObjectProperty ;
                rdfs:subPropertyOf owl:topObjectProperty ;
                rdfs:range :LoadingUnit ;
                rdfs:comment "Relates an XDocLoadingUnit (cross-dock loading unit), a TradeItem, a ShipmentItem or a DGR (dangerous goods) to a LoadingUnit" .


###  https://w3id.org/latuli/ontology/m3#hasOutboundConsignment
:hasOutboundConsignment rdf:type owl:ObjectProperty ;
                        rdfs:subPropertyOf owl:topObjectProperty ;
                        rdfs:range :Consignment ;
                        rdfs:comment "Relates an XDocLoadingUnit (cross-dock loading unit) to an outbound Consignment" .


###  https://w3id.org/latuli/ontology/m3#hasOutboundParentLoadingUnit
:hasOutboundParentLoadingUnit rdf:type owl:ObjectProperty ;
                              rdfs:subPropertyOf owl:topObjectProperty ;
                              rdfs:range :LoadingUnit ;
                              rdfs:comment "Relates an XDocLoadingUnit (cross-dock loading unit) to an outbound parent LoadingUnit" .


###  https://w3id.org/latuli/ontology/m3#hasParty
:hasParty rdf:type owl:ObjectProperty ;
          rdfs:subPropertyOf owl:topObjectProperty ;
          rdfs:range :Party .


###  https://w3id.org/latuli/ontology/m3#hasReceiverParty
:hasReceiverParty rdf:type owl:ObjectProperty ;
                  rdfs:subPropertyOf owl:topObjectProperty ;
                  rdfs:range :Receiver ;
                  rdfs:comment "Relates an XDocLoadingUnit (cross-dock loading unit) or a Shipment to a Receiver." .


###  https://w3id.org/latuli/ontology/m3#hasShipperParty
:hasShipperParty rdf:type owl:ObjectProperty ;
                 rdfs:subPropertyOf owl:topObjectProperty ;
                 rdfs:range :Shipper ;
                 rdfs:comment "Relates an XDocLoadingUnit (cross-dock loading unit) or a Shipment to a Shipper." .


###  https://w3id.org/latuli/ontology/m3#includesTransport
:includesTransport rdf:type owl:ObjectProperty ;
                   rdfs:range :Transport ;
                   rdfs:comment "Relates a Consignment to a Transport" .


###  https://w3id.org/latuli/ontology/m3#processedByWave
:processedByWave rdf:type owl:ObjectProperty ;
                 rdfs:subPropertyOf owl:topObjectProperty ;
                 rdfs:range :Wave ;
                 rdfs:comment "Relates an XDocLoadingUnit (cross-dock loading unit) or a Consignment to a Wave." .


###  https://w3id.org/latuli/ontology/m3#relatesToTradeItem
:relatesToTradeItem rdf:type owl:ObjectProperty ;
                    rdfs:subPropertyOf owl:topObjectProperty ;
                    rdfs:range :TradeItem ;
                    rdfs:comment "Relates a DGR (dangerous goods) to a Trade Item." .


#################################################################
#    Data properties
#################################################################

###  http://www.opengis.net/ont/geosparql#asGML
<http://www.opengis.net/ont/geosparql#asGML> rdf:type owl:DatatypeProperty ;
                                             rdfs:subPropertyOf <http://www.opengis.net/ont/geosparql#hasSerialization> ;
                                             rdfs:domain <http://www.opengis.net/ont/geosparql#Geometry> ;
                                             rdfs:range <http://www.opengis.net/ont/geosparql#gmlLiteral> ;
                                             <http://purl.org/dc/elements/1.1/contributor> "Matthew Perry" ;
                                             <http://purl.org/dc/elements/1.1/creator> "OGC GeoSPARQL 1.0 Standard Working Group" ;
                                             <http://purl.org/dc/elements/1.1/date> "2011-06-16"^^xsd:date ;
                                             <http://purl.org/dc/elements/1.1/description> """
      The GML serialization of a geometry
    """@en ;
                                             rdfs:comment """
      The GML serialization of a geometry
    """@en ;
                                             rdfs:isDefinedBy <http://www.opengis.net/ont/geosparql> ,
                                                              <http://www.opengis.net/spec/geosparql/1.0> ;
                                             rdfs:label "asGML"@en ;
                                             <http://www.w3.org/2004/02/skos/core#definition> """
      The GML serialization of a geometry
    """@en ;
                                             <http://www.w3.org/2004/02/skos/core#prefLabel> "asGML"@en .


###  http://www.opengis.net/ont/geosparql#asWKT
<http://www.opengis.net/ont/geosparql#asWKT> rdf:type owl:DatatypeProperty ;
                                             rdfs:subPropertyOf <http://www.opengis.net/ont/geosparql#hasSerialization> ;
                                             rdfs:domain <http://www.opengis.net/ont/geosparql#Geometry> ;
                                             rdfs:range <http://www.opengis.net/ont/geosparql#wktLiteral> ;
                                             <http://purl.org/dc/elements/1.1/contributor> "Matthew Perry" ;
                                             <http://purl.org/dc/elements/1.1/creator> "OGC GeoSPARQL 1.0 Standard Working Group" ;
                                             <http://purl.org/dc/elements/1.1/date> "2011-06-16"^^xsd:date ;
                                             <http://purl.org/dc/elements/1.1/description> """
      The WKT serialization of a geometry
    """@en ;
                                             rdfs:comment """
      The WKT serialization of a geometry
    """@en ;
                                             rdfs:isDefinedBy <http://www.opengis.net/ont/geosparql> ,
                                                              <http://www.opengis.net/spec/geosparql/1.0> ;
                                             rdfs:label "asWKT"@en ;
                                             <http://www.w3.org/2004/02/skos/core#definition> """
      The WKT serialization of a geometry
    """@en ;
                                             <http://www.w3.org/2004/02/skos/core#prefLabel> "asWKT"@en .


###  http://www.opengis.net/ont/geosparql#coordinateDimension
<http://www.opengis.net/ont/geosparql#coordinateDimension> rdf:type owl:DatatypeProperty ;
                                                           rdfs:domain <http://www.opengis.net/ont/geosparql#Geometry> ;
                                                           rdfs:range xsd:integer ;
                                                           <http://purl.org/dc/elements/1.1/contributor> "Matthew Perry" ;
                                                           <http://purl.org/dc/elements/1.1/creator> "OGC GeoSPARQL 1.0 Standard Working Group" ;
                                                           <http://purl.org/dc/elements/1.1/date> "2011-06-16"^^xsd:date ;
                                                           <http://purl.org/dc/elements/1.1/description> """
      The number of measurements or axes needed to describe the position of this
      geometry in a coordinate system.
    """@en ;
                                                           rdfs:comment """
      The number of measurements or axes needed to describe the position of this
      geometry in a coordinate system.
    """@en ;
                                                           rdfs:isDefinedBy <http://www.opengis.net/ont/geosparql> ,
                                                                            <http://www.opengis.net/spec/geosparql/1.0> ;
                                                           rdfs:label "coordinateDimension"@en ;
                                                           <http://www.w3.org/2004/02/skos/core#definition> """
      The number of measurements or axes needed to describe the position of this
      geometry in a coordinate system.
    """@en ;
                                                           <http://www.w3.org/2004/02/skos/core#prefLabel> "coordinateDimension"@en .


###  http://www.opengis.net/ont/geosparql#dimension
<http://www.opengis.net/ont/geosparql#dimension> rdf:type owl:DatatypeProperty ;
                                                 rdfs:domain <http://www.opengis.net/ont/geosparql#Geometry> ;
                                                 rdfs:range xsd:integer ;
                                                 <http://purl.org/dc/elements/1.1/contributor> "Matthew Perry" ;
                                                 <http://purl.org/dc/elements/1.1/creator> "OGC GeoSPARQL 1.0 Standard Working Group" ;
                                                 <http://purl.org/dc/elements/1.1/date> "2011-06-16"^^xsd:date ;
                                                 <http://purl.org/dc/elements/1.1/description> """
      The topological dimension of this geometric object, which 
      must be less than or equal to the coordinate dimension. 
      In non-homogeneous collections, this will return the largest 
      topological dimension of the contained objects.
    """@en ;
                                                 rdfs:comment """
      The topological dimension of this geometric object, which 
      must be less than or equal to the coordinate dimension. 
      In non-homogeneous collections, this will return the largest 
      topological dimension of the contained objects.
    """@en ;
                                                 rdfs:isDefinedBy <http://www.opengis.net/ont/geosparql> ,
                                                                  <http://www.opengis.net/spec/geosparql/1.0> ;
                                                 rdfs:label "dimension"@en ;
                                                 <http://www.w3.org/2004/02/skos/core#definition> """
      The topological dimension of this geometric object, which 
      must be less than or equal to the coordinate dimension. 
      In non-homogeneous collections, this will return the largest 
      topological dimension of the contained objects.
    """@en ;
                                                 <http://www.w3.org/2004/02/skos/core#prefLabel> "dimension"@en .


###  http://www.opengis.net/ont/geosparql#hasSerialization
<http://www.opengis.net/ont/geosparql#hasSerialization> rdf:type owl:DatatypeProperty ;
                                                        rdfs:domain <http://www.opengis.net/ont/geosparql#Geometry> ;
                                                        rdfs:range rdfs:Literal ;
                                                        <http://purl.org/dc/elements/1.1/contributor> "Matthew Perry" ;
                                                        <http://purl.org/dc/elements/1.1/creator> "OGC GeoSPARQL 1.0 Standard Working Group" ;
                                                        <http://purl.org/dc/elements/1.1/date> "2011-06-16"^^xsd:date ;
                                                        <http://purl.org/dc/elements/1.1/description> """
      Connects a geometry object with its text-based serialization.
    """@en ;
                                                        rdfs:comment """
      Connects a geometry object with its text-based serialization.
    """@en ;
                                                        rdfs:isDefinedBy <http://www.opengis.net/ont/geosparql> ,
                                                                         <http://www.opengis.net/spec/geosparql/1.0> ;
                                                        rdfs:label "has serialization"@en ;
                                                        <http://www.w3.org/2004/02/skos/core#definition> """
      Connects a geometry object with its text-based serialization.
    """@en ;
                                                        <http://www.w3.org/2004/02/skos/core#prefLabel> "has serialization"@en .


###  http://www.opengis.net/ont/geosparql#isEmpty
<http://www.opengis.net/ont/geosparql#isEmpty> rdf:type owl:DatatypeProperty ;
                                               rdfs:domain <http://www.opengis.net/ont/geosparql#Geometry> ;
                                               rdfs:range xsd:boolean ;
                                               <http://purl.org/dc/elements/1.1/contributor> "Matthew Perry" ;
                                               <http://purl.org/dc/elements/1.1/creator> "OGC GeoSPARQL 1.0 Standard Working Group" ;
                                               <http://purl.org/dc/elements/1.1/date> "2011-06-16"^^xsd:date ;
                                               <http://purl.org/dc/elements/1.1/description> """
      (true) if this geometric object is the empty Geometry. If 
      true, then this geometric object represents the empty point 
      set for the coordinate space.
    """@en ;
                                               rdfs:comment """
      (true) if this geometric object is the empty Geometry. If 
      true, then this geometric object represents the empty point 
      set for the coordinate space.
    """@en ;
                                               rdfs:isDefinedBy <http://www.opengis.net/ont/geosparql> ,
                                                                <http://www.opengis.net/spec/geosparql/1.0> ;
                                               rdfs:label "isEmpty"@en ;
                                               <http://www.w3.org/2004/02/skos/core#definition> """
      (true) if this geometric object is the empty Geometry. If 
      true, then this geometric object represents the empty point 
      set for the coordinate space.
    """@en ;
                                               <http://www.w3.org/2004/02/skos/core#prefLabel> "isEmpty"@en .


###  http://www.opengis.net/ont/geosparql#isSimple
<http://www.opengis.net/ont/geosparql#isSimple> rdf:type owl:DatatypeProperty ;
                                                rdfs:domain <http://www.opengis.net/ont/geosparql#Geometry> ;
                                                rdfs:range xsd:boolean ;
                                                <http://purl.org/dc/elements/1.1/contributor> "Matthew Perry" ;
                                                <http://purl.org/dc/elements/1.1/creator> "OGC GeoSPARQL 1.0 Standard Working Group" ;
                                                <http://purl.org/dc/elements/1.1/date> "2011-06-16"^^xsd:date ;
                                                <http://purl.org/dc/elements/1.1/description> """
      (true) if this geometric object has no anomalous geometric 
      points, such as self intersection or self tangency.
    """@en ;
                                                rdfs:comment """
      (true) if this geometric object has no anomalous geometric 
      points, such as self intersection or self tangency.
    """@en ;
                                                rdfs:isDefinedBy <http://www.opengis.net/ont/geosparql> ,
                                                                 <http://www.opengis.net/spec/geosparql/1.0> ;
                                                rdfs:label "isSimple"@en ;
                                                <http://www.w3.org/2004/02/skos/core#definition> """
      (true) if this geometric object has no anomalous geometric 
      points, such as self intersection or self tangency.
    """@en ;
                                                <http://www.w3.org/2004/02/skos/core#prefLabel> "isSimple"@en .


###  http://www.opengis.net/ont/geosparql#spatialDimension
<http://www.opengis.net/ont/geosparql#spatialDimension> rdf:type owl:DatatypeProperty ;
                                                        rdfs:domain <http://www.opengis.net/ont/geosparql#Geometry> ;
                                                        rdfs:range xsd:integer ;
                                                        <http://purl.org/dc/elements/1.1/contributor> "Matthew Perry" ;
                                                        <http://purl.org/dc/elements/1.1/creator> "OGC GeoSPARQL 1.0 Standard Working Group" ;
                                                        <http://purl.org/dc/elements/1.1/date> "2011-06-16"^^xsd:date ;
                                                        <http://purl.org/dc/elements/1.1/description> """
      The number of measurements or axes needed to describe the spatial position of 
      this geometry in a coordinate system.
    """@en ;
                                                        rdfs:comment """
      The number of measurements or axes needed to describe the spatial position of 
      this geometry in a coordinate system.
    """@en ;
                                                        rdfs:isDefinedBy <http://www.opengis.net/ont/geosparql> ,
                                                                         <http://www.opengis.net/spec/geosparql/1.0> ;
                                                        rdfs:label "spatialDimension"@en ;
                                                        <http://www.w3.org/2004/02/skos/core#definition> """
      The number of measurements or axes needed to describe the spatial position of 
      this geometry in a coordinate system.
    """@en ;
                                                        <http://www.w3.org/2004/02/skos/core#prefLabel> "spatialDimension"@en .


###  https://w3id.org/latuli/ontology/m3#additionalPartyIdentification
:additionalPartyIdentification rdf:type owl:DatatypeProperty ;
                               rdfs:range xsd:string ;
                               rdfs:comment "Identifies a party using a custom identification scheme." .


###  https://w3id.org/latuli/ontology/m3#asWKT
:asWKT rdf:type owl:DatatypeProperty ;
       rdfs:subPropertyOf owl:topDataProperty ;
       rdfs:domain :Party ;
       rdfs:range <http://www.opengis.net/ont/geosparql#wktLiteral> .


###  https://w3id.org/latuli/ontology/m3#carrierHashCode
:carrierHashCode rdf:type owl:DatatypeProperty ;
                 rdfs:range xsd:string ;
                 rdfs:comment "A hashcode which represents a carrier party using a numeric value" .


###  https://w3id.org/latuli/ontology/m3#closedOn
:closedOn rdf:type owl:DatatypeProperty ;
          rdfs:subPropertyOf owl:topDataProperty ;
          rdfs:range xsd:dateTime ;
          rdfs:comment "Timestamp for when a wave is closed." .


###  https://w3id.org/latuli/ontology/m3#code2
:code2 rdf:type owl:DatatypeProperty ;
       rdfs:subPropertyOf owl:topDataProperty ;
       rdfs:domain :Party ;
       rdfs:range xsd:string ;
       rdfs:comment "Two-digit identifier for describing a country." .


###  https://w3id.org/latuli/ontology/m3#consigneeHashCode
:consigneeHashCode rdf:type owl:DatatypeProperty ;
                   rdfs:range xsd:string ;
                   rdfs:comment "A hashcode which represents a consignee party using a numeric value" .


###  https://w3id.org/latuli/ontology/m3#consignmentId
:consignmentId rdf:type owl:DatatypeProperty ;
               rdfs:subPropertyOf owl:topDataProperty ;
               rdfs:range xsd:string ;
               rdfs:comment "An unique identifier for a consignment." .


###  https://w3id.org/latuli/ontology/m3#consignmentType
:consignmentType rdf:type owl:DatatypeProperty ;
                 rdfs:subPropertyOf owl:topDataProperty ;
                 rdfs:range xsd:string ;
                 rdfs:comment "Describes whether a consignment is inbound or outbound" .


###  https://w3id.org/latuli/ontology/m3#consignorHashCode
:consignorHashCode rdf:type owl:DatatypeProperty ;
                   rdfs:range xsd:string ;
                   rdfs:comment "A hashcode which represents a consignor  party using a numeric value" .


###  https://w3id.org/latuli/ontology/m3#createdOn
:createdOn rdf:type owl:DatatypeProperty ;
           rdfs:range xsd:dateTime ;
           rdfs:comment "A hashcode which represents a consignor  party using a numeric value" .


###  https://w3id.org/latuli/ontology/m3#customerProductDescription
:customerProductDescription rdf:type owl:DatatypeProperty ;
                            rdfs:subPropertyOf owl:topDataProperty ;
                            rdfs:range xsd:string ;
                            rdfs:comment "A description of a trade item by the customer." .


###  https://w3id.org/latuli/ontology/m3#customerProductId
:customerProductId rdf:type owl:DatatypeProperty ;
                   rdfs:subPropertyOf owl:topDataProperty ;
                   rdfs:range xsd:string ;
                   rdfs:comment "The identifier of a trade item used by the customer" .


###  https://w3id.org/latuli/ontology/m3#customerQuantity
:customerQuantity rdf:type owl:DatatypeProperty ;
                  rdfs:subPropertyOf owl:topDataProperty ;
                  rdfs:range xsd:decimal ;
                  rdfs:comment "The quantity of trade items expected by the customer." .


###  https://w3id.org/latuli/ontology/m3#description
:description rdf:type owl:DatatypeProperty ;
             rdfs:subPropertyOf owl:topDataProperty ;
             rdfs:range xsd:string ;
             rdfs:comment "A description of a trade item." .


###  https://w3id.org/latuli/ontology/m3#effectiveArrival
:effectiveArrival rdf:type owl:DatatypeProperty ;
                  rdfs:range xsd:dateTime ;
                  rdfs:comment "Timestamp for when a transport means actually arrived at an hub." .


###  https://w3id.org/latuli/ontology/m3#expectedArrival
:expectedArrival rdf:type owl:DatatypeProperty ;
                 rdfs:range xsd:dateTime ;
                 rdfs:comment "Timestamp for when a transport means is expected to arrive at an hub." .


###  https://w3id.org/latuli/ontology/m3#expectedDeliveryOn
:expectedDeliveryOn rdf:type owl:DatatypeProperty ;
                    rdfs:subPropertyOf owl:topDataProperty ;
                    rdfs:domain :Shipment ;
                    rdfs:range xsd:dateTime ;
                    rdfs:comment "Timestamp for when a shipment is expected to be delivered to a receiver." ;
                    <http://www.w3.org/2004/02/skos/core#prefLabel> "expectedDeliveryOn"@nb .


###  https://w3id.org/latuli/ontology/m3#finishedScanOn
:finishedScanOn rdf:type owl:DatatypeProperty ;
                rdfs:range xsd:dateTime ;
                rdfs:comment "Timestamp for when a xDocLoadingUnit (cross dock loading unit) has been scanned." .


###  https://w3id.org/latuli/ontology/m3#fullPalletConsignment
:fullPalletConsignment rdf:type owl:DatatypeProperty ;
                       rdfs:subPropertyOf owl:topDataProperty ;
                       rdfs:range xsd:string ;
                       rdfs:comment "Describes whether a consignment consist of full pallets (1) or not (0)" .


###  https://w3id.org/latuli/ontology/m3#gln
:gln rdf:type owl:DatatypeProperty ;
     rdfs:subPropertyOf owl:topDataProperty ;
     rdfs:range xsd:string ;
     rdfs:comment "GLN is the GS1 Identification Key used to identify physical locations or parties. The key comprises a GS1 Company Prefix, Location Reference, and Check Digit" .


###  https://w3id.org/latuli/ontology/m3#gtin
:gtin rdf:type owl:DatatypeProperty ;
      rdfs:range xsd:string ;
      rdfs:comment "GTIN is the GS1 Identification Key used to identify trade items. The key comprises a GS1 Company Prefix, an Item Reference and Check Digit." .


###  https://w3id.org/latuli/ontology/m3#handlingInstruction
:handlingInstruction rdf:type owl:DatatypeProperty ;
                     rdfs:subPropertyOf owl:topDataProperty ;
                     rdfs:range xsd:string ;
                     rdfs:comment "Instructions that describe how goods should be expedited during transport and other goods handling." .


###  https://w3id.org/latuli/ontology/m3#hashCode
:hashCode rdf:type owl:DatatypeProperty ;
          rdfs:subPropertyOf owl:topDataProperty ;
          rdfs:range xsd:string ;
          rdfs:comment "A hashcode which represents a hub party using a numeric value" .


###  https://w3id.org/latuli/ontology/m3#hubAdditionalPartyIdentification
:hubAdditionalPartyIdentification rdf:type owl:DatatypeProperty ;
                                  rdfs:subPropertyOf owl:topDataProperty ;
                                  rdfs:range xsd:string ;
                                  rdfs:comment "Identifies a hub party using a custom identification scheme." .


###  https://w3id.org/latuli/ontology/m3#hubHashCode
:hubHashCode rdf:type owl:DatatypeProperty ;
             rdfs:range xsd:string ;
             rdfs:comment "A hashcode which represents a hub party using a numeric value" .


###  https://w3id.org/latuli/ontology/m3#hubReconstructionHashCode
:hubReconstructionHashCode rdf:type owl:DatatypeProperty ;
                           rdfs:range xsd:string ;
                           rdfs:comment "A hashcode which represents a hub reconstruction location using a numeric value" .


###  https://w3id.org/latuli/ontology/m3#hubReconstructionLocationId
:hubReconstructionLocationId rdf:type owl:DatatypeProperty ;
                             rdfs:range xsd:string ;
                             rdfs:comment "A unique identifier for a hub reconstruction location" .


###  https://w3id.org/latuli/ontology/m3#internalId
:internalId rdf:type owl:DatatypeProperty ;
            rdfs:range xsd:string ;
            rdfs:comment "A unique identifier for an xDocLoadingUnit (cross-dock loading unit)" .


###  https://w3id.org/latuli/ontology/m3#isCarrier
:isCarrier rdf:type owl:DatatypeProperty ;
           rdfs:range xsd:boolean ;
           rdfs:comment "A flag that defines whether a party is a carrier (1) or not (0)" .


###  https://w3id.org/latuli/ontology/m3#isConsignor
:isConsignor rdf:type owl:DatatypeProperty ;
             rdfs:range xsd:boolean ;
             rdfs:comment "A flag that defines whether a party is a consignor (1) or not (0)" .


###  https://w3id.org/latuli/ontology/m3#isHub
:isHub rdf:type owl:DatatypeProperty ;
       rdfs:range xsd:boolean ;
       rdfs:comment "A flag that defines whether a party is a hub (1) or not (0)" .


###  https://w3id.org/latuli/ontology/m3#isShipper
:isShipper rdf:type owl:DatatypeProperty ;
           rdfs:range xsd:boolean ;
           rdfs:comment "A flag that defines whether a party is a shipper (1) or not (0)" .


###  https://w3id.org/latuli/ontology/m3#location
:location rdf:type owl:DatatypeProperty ;
          rdfs:subPropertyOf owl:topDataProperty ;
          rdfs:domain :Party ;
          rdfs:range xsd:string ;
          rdfs:comment "The name of the city associated with a party" .


###  https://w3id.org/latuli/ontology/m3#lotNumber
:lotNumber rdf:type owl:DatatypeProperty ;
           rdfs:subPropertyOf owl:topDataProperty ;
           rdfs:range xsd:string ;
           rdfs:comment "A lot number is an identification number assigned to a particular quantity or lot of material from a single manufacturer" .


###  https://w3id.org/latuli/ontology/m3#material
:material rdf:type owl:DatatypeProperty ;
          rdfs:subPropertyOf owl:topDataProperty ;
          rdfs:range xsd:string ;
          rdfs:comment "Describes the material used in a trade item" .


###  https://w3id.org/latuli/ontology/m3#modifiedOn
:modifiedOn rdf:type owl:DatatypeProperty ;
            rdfs:subPropertyOf owl:topDataProperty ;
            rdfs:range xsd:dateTime ;
            rdfs:comment "Timestamp for when an entry in the database is modified." .


###  https://w3id.org/latuli/ontology/m3#orderNumber
:orderNumber rdf:type owl:DatatypeProperty ;
             rdfs:range xsd:string ;
             rdfs:comment "A reference to the order number when describing a loading unit." .


###  https://w3id.org/latuli/ontology/m3#packageTypeId
:packageTypeId rdf:type owl:DatatypeProperty ;
               rdfs:subPropertyOf owl:topDataProperty ;
               rdfs:domain :LoadingUnit ;
               rdfs:range xsd:string ;
               rdfs:comment "Describes what type of packaging type the loading unit consists of. Examples are BX (box) and PX (pallet)." .


###  https://w3id.org/latuli/ontology/m3#plannedDeliveryDate
:plannedDeliveryDate rdf:type owl:DatatypeProperty ;
                     rdfs:subPropertyOf owl:topDataProperty ;
                     rdfs:domain :Shipment ;
                     rdfs:range xsd:dateTime ;
                     rdfs:comment "Timestamp for when a shipment is planned to be delivered to the receiver." .


###  https://w3id.org/latuli/ontology/m3#plannedOn
:plannedOn rdf:type owl:DatatypeProperty ;
           rdfs:range xsd:dateTime ;
           rdfs:comment "Timestamp for when a wave has been planned." .


###  https://w3id.org/latuli/ontology/m3#postalCode
:postalCode rdf:type owl:DatatypeProperty ;
            rdfs:subPropertyOf owl:topDataProperty ;
            rdfs:domain :Party ;
            rdfs:range xsd:string ;
            rdfs:comment "Describes the postal code associated with a party." .


###  https://w3id.org/latuli/ontology/m3#preSortScanOn
:preSortScanOn rdf:type owl:DatatypeProperty ;
               rdfs:subPropertyOf owl:topDataProperty ;
               rdfs:domain :XDocLoadingUnit ;
               rdfs:range xsd:dateTime ;
               rdfs:comment "Timestamp for when an XDocLoadingUnit (cross-dock loading unit) has been presorted." .


###  https://w3id.org/latuli/ontology/m3#purchaseOrder
:purchaseOrder rdf:type owl:DatatypeProperty ;
               rdfs:subPropertyOf owl:topDataProperty ;
               rdfs:range xsd:string ;
               rdfs:comment "A reference to a purchase order associated with a trade item" .


###  https://w3id.org/latuli/ontology/m3#qttBoxes
:qttBoxes rdf:type owl:DatatypeProperty ;
          rdfs:subPropertyOf owl:topDataProperty ;
          rdfs:domain :Consignment ;
          rdfs:range xsd:int ;
          rdfs:comment "The quantity of boxes in a consignment, a shipment or in a wave" .


###  https://w3id.org/latuli/ontology/m3#qttBoxesProcessed
:qttBoxesProcessed rdf:type owl:DatatypeProperty ;
                   rdfs:subPropertyOf owl:topDataProperty ;
                   rdfs:range xsd:int ;
                   rdfs:comment "The quantity of boxes processed in a wave" .


###  https://w3id.org/latuli/ontology/m3#qttPallets
:qttPallets rdf:type owl:DatatypeProperty ;
            rdfs:subPropertyOf owl:topDataProperty ;
            rdfs:range xsd:int ;
            rdfs:comment "The quantity of pallets in a consignment, a shipment or in wave" .


###  https://w3id.org/latuli/ontology/m3#qttPalletsBuilt
:qttPalletsBuilt rdf:type owl:DatatypeProperty ;
                 rdfs:subPropertyOf owl:topDataProperty ;
                 rdfs:range xsd:int ;
                 rdfs:comment "The quantity of pallets built in a wave" .


###  https://w3id.org/latuli/ontology/m3#qttReconstructedPallets
:qttReconstructedPallets rdf:type owl:DatatypeProperty ;
                         rdfs:subPropertyOf owl:topDataProperty ;
                         rdfs:domain :Consignment ;
                         rdfs:range xsd:int ;
                         rdfs:comment "The quantity of reconstructed pallets in a consignment" .


###  https://w3id.org/latuli/ontology/m3#qttReconstructedParcels
:qttReconstructedParcels rdf:type owl:DatatypeProperty ;
                         rdfs:subPropertyOf owl:topDataProperty ;
                         rdfs:domain :Consignment ;
                         rdfs:range xsd:int ;
                         rdfs:comment "The quantity of reconstructed parcels in a consignment" .


###  https://w3id.org/latuli/ontology/m3#qttShipments
:qttShipments rdf:type owl:DatatypeProperty ;
              rdfs:subPropertyOf owl:topDataProperty ;
              rdfs:domain :Wave ;
              rdfs:range xsd:int ;
              rdfs:comment "The quantity of shipments processed in a wave" .


###  https://w3id.org/latuli/ontology/m3#qttTasks
:qttTasks rdf:type owl:DatatypeProperty ;
          rdfs:subPropertyOf owl:topDataProperty ;
          rdfs:domain :Wave ;
          rdfs:range xsd:int ;
          rdfs:comment "The quantity of tasks processed in a wave" .


###  https://w3id.org/latuli/ontology/m3#qttTrailers
:qttTrailers rdf:type owl:DatatypeProperty ;
             rdfs:subPropertyOf owl:topDataProperty ;
             rdfs:domain :Wave ;
             rdfs:range xsd:int ;
             rdfs:comment "The quantity of trailers processed in a wave" .


###  https://w3id.org/latuli/ontology/m3#quantity
:quantity rdf:type owl:DatatypeProperty ;
          rdfs:subPropertyOf owl:topDataProperty ;
          rdfs:domain :ShipmentItem ;
          rdfs:range xsd:int ;
          rdfs:comment "The quantity of individual items in a trade item" .


###  https://w3id.org/latuli/ontology/m3#receiverHashCode
:receiverHashCode rdf:type owl:DatatypeProperty ;
                  rdfs:range xsd:string ;
                  rdfs:comment "A hashcode which represents a receiver party using a numeric value" .


###  https://w3id.org/latuli/ontology/m3#reconstructedScanOn
:reconstructedScanOn rdf:type owl:DatatypeProperty ;
                     rdfs:subPropertyOf owl:topDataProperty ;
                     rdfs:domain :XDocLoadingUnit ;
                     rdfs:range xsd:dateTime ;
                     rdfs:comment "Timestamp for when an XDocLoadingUnit (cross-dock loading unit) is being reconstructed." .


###  https://w3id.org/latuli/ontology/m3#reconstructionLane
:reconstructionLane rdf:type owl:DatatypeProperty ;
                    rdfs:subPropertyOf owl:topDataProperty ;
                    rdfs:range xsd:string ;
                    rdfs:comment "A lane or section in a terminal or hub used for the reconstruction of goods" .


###  https://w3id.org/latuli/ontology/m3#reconstructionLocation
:reconstructionLocation rdf:type owl:DatatypeProperty ;
                        rdfs:range xsd:string ;
                        rdfs:comment "A location in which a reconstruction takes place." .


###  https://w3id.org/latuli/ontology/m3#reconstructionTypeId
:reconstructionTypeId rdf:type owl:DatatypeProperty ;
                      rdfs:range xsd:string ;
                      rdfs:comment "The type of reconstruction performed. Values are either loose cartons (LooseCarton), recon pallet (ReconPallet), or recon parcel (ReconParcel)." .


###  https://w3id.org/latuli/ontology/m3#releasedOn
:releasedOn rdf:type owl:DatatypeProperty ;
            rdfs:subPropertyOf owl:topDataProperty ;
            rdfs:range xsd:dateTime ;
            rdfs:comment "Timestamp for when a wave is released." .


###  https://w3id.org/latuli/ontology/m3#salesOrder
:salesOrder rdf:type owl:DatatypeProperty ;
            rdfs:subPropertyOf owl:topDataProperty ;
            rdfs:range xsd:string ;
            rdfs:comment "A reference to a sales order associated with a trade item" .


###  https://w3id.org/latuli/ontology/m3#shipmentId
:shipmentId rdf:type owl:DatatypeProperty ;
            rdfs:range xsd:string ;
            rdfs:comment "A unique identifier for a shipment." .


###  https://w3id.org/latuli/ontology/m3#shippedOn
:shippedOn rdf:type owl:DatatypeProperty ;
           rdfs:subPropertyOf owl:topDataProperty ;
           rdfs:domain :Shipment ;
           rdfs:range xsd:dateTime ;
           rdfs:comment "Timestamp for when a shipment is sent from a shipper." ;
           <http://www.w3.org/2004/02/skos/core#prefLabel> "shippedOn"@nb .


###  https://w3id.org/latuli/ontology/m3#shipperHashCode
:shipperHashCode rdf:type owl:DatatypeProperty ;
                 rdfs:range xsd:string ;
                 rdfs:comment "A hashcode which represents a shipper party using a numeric value" .


###  https://w3id.org/latuli/ontology/m3#splitShipment
:splitShipment rdf:type owl:DatatypeProperty ;
               rdfs:subPropertyOf owl:topDataProperty ;
               rdfs:range xsd:int ;
               rdfs:comment "A flag that defines whether a shipment has been split or not." .


###  https://w3id.org/latuli/ontology/m3#status
:status rdf:type owl:DatatypeProperty ;
        rdfs:subPropertyOf owl:topDataProperty ;
        rdfs:range xsd:string ;
        rdfs:comment "The status of a wave." .


###  https://w3id.org/latuli/ontology/m3#supplierProductDescription
:supplierProductDescription rdf:type owl:DatatypeProperty ;
                            rdfs:subPropertyOf owl:topDataProperty ;
                            rdfs:range xsd:string ;
                            rdfs:comment "A description of a trade item by the supplier." .


###  https://w3id.org/latuli/ontology/m3#supplierProductId
:supplierProductId rdf:type owl:DatatypeProperty ;
                   rdfs:subPropertyOf owl:topDataProperty ;
                   rdfs:range xsd:string ;
                   rdfs:comment "The identifier of a trade item used by the supplier." .


###  https://w3id.org/latuli/ontology/m3#supplierQuantity
:supplierQuantity rdf:type owl:DatatypeProperty ;
                  rdfs:subPropertyOf owl:topDataProperty ;
                  rdfs:range xsd:decimal ;
                  rdfs:comment "The quantity of trade items as provided by the supplier." .


###  https://w3id.org/latuli/ontology/m3#taskClosedOn
:taskClosedOn rdf:type owl:DatatypeProperty ;
              rdfs:subPropertyOf owl:topDataProperty ;
              rdfs:domain :Consignment ;
              rdfs:range xsd:dateTime ;
              rdfs:comment "Timestamp for when a consignment task is closed." .


###  https://w3id.org/latuli/ontology/m3#taskDescription
:taskDescription rdf:type owl:DatatypeProperty ;
                 rdfs:subPropertyOf owl:topDataProperty ;
                 rdfs:range xsd:string ;
                 rdfs:comment "A description of a reconstruction task related to a consignment. Examples are Reconstruct by Address, Reconstruct by Product or Reconstruct by Order." .


###  https://w3id.org/latuli/ontology/m3#taskId
:taskId rdf:type owl:DatatypeProperty ;
        rdfs:subPropertyOf owl:topDataProperty ;
        rdfs:range xsd:string ;
        rdfs:comment "An identifier that describes the reconstruction task related to a consignment." .


###  https://w3id.org/latuli/ontology/m3#totalConsignmentVolume
:totalConsignmentVolume rdf:type owl:DatatypeProperty ;
                        rdfs:subPropertyOf owl:topDataProperty ;
                        rdfs:domain :Consignment ;
                        rdfs:range xsd:decimal ;
                        rdfs:comment "The total volume of a consignment." .


###  https://w3id.org/latuli/ontology/m3#totalConsignmentWeight
:totalConsignmentWeight rdf:type owl:DatatypeProperty ;
                        rdfs:subPropertyOf owl:topDataProperty ;
                        rdfs:domain :Consignment ;
                        rdfs:range xsd:decimal ;
                        rdfs:comment "The total weight of a consignment." .


###  https://w3id.org/latuli/ontology/m3#transportId
:transportId rdf:type owl:DatatypeProperty ;
             rdfs:subPropertyOf owl:topDataProperty ;
             rdfs:range xsd:string ;
             rdfs:comment "A unique identifier for a transport." .


###  https://w3id.org/latuli/ontology/m3#transportName
:transportName rdf:type owl:DatatypeProperty ;
               rdfs:range xsd:string ;
               rdfs:comment "The name of a transport. Examples are TJUE042ZU2 and 528776." .


###  https://w3id.org/latuli/ontology/m3#transportType
:transportType rdf:type owl:DatatypeProperty ;
               rdfs:subPropertyOf owl:topDataProperty ;
               rdfs:domain :Transport ;
               rdfs:range xsd:string ;
               rdfs:comment "A flag that defines whether a transport is inbound (IN) or outbound (OUT)" .


###  https://w3id.org/latuli/ontology/m3#volume
:volume rdf:type owl:DatatypeProperty ;
        rdfs:subPropertyOf owl:topDataProperty ;
        rdfs:range xsd:decimal ;
        rdfs:comment "The volume of an xDocLoadingUnit (cross-dock loading unit)." .


###  https://w3id.org/latuli/ontology/m3#waveClosedOn
:waveClosedOn rdf:type owl:DatatypeProperty ;
              rdfs:range xsd:dateTime ;
              rdfs:comment "Timestamp for when a wave is closed." .


###  https://w3id.org/latuli/ontology/m3#waveEndProcessingOn
:waveEndProcessingOn rdf:type owl:DatatypeProperty ;
                     rdfs:subPropertyOf owl:topDataProperty ;
                     rdfs:domain :Wave ;
                     rdfs:range xsd:dateTime ;
                     rdfs:comment "Timestamp for when a wave process is ended." .


###  https://w3id.org/latuli/ontology/m3#waveId
:waveId rdf:type owl:DatatypeProperty ;
        rdfs:range xsd:string ;
        rdfs:comment "A unique identifier for a wave." .


###  https://w3id.org/latuli/ontology/m3#wavePlannedOn
:wavePlannedOn rdf:type owl:DatatypeProperty ;
               rdfs:range xsd:dateTime ;
               rdfs:comment "Timestamp for when a wave has been planned." .


###  https://w3id.org/latuli/ontology/m3#waveReleasedOn
:waveReleasedOn rdf:type owl:DatatypeProperty ;
                rdfs:range xsd:dateTime ;
                rdfs:comment "Timestamp for when a wave has been released to the floor." .


###  https://w3id.org/latuli/ontology/m3#waveStartProcessingOn
:waveStartProcessingOn rdf:type owl:DatatypeProperty ;
                       rdfs:subPropertyOf owl:topDataProperty ;
                       rdfs:domain :Wave ;
                       rdfs:range xsd:dateTime ;
                       rdfs:comment "Timestamp for when a wave process is started." .


###  https://w3id.org/latuli/ontology/m3#weight
:weight rdf:type owl:DatatypeProperty ;
        rdfs:subPropertyOf owl:topDataProperty ;
        rdfs:range xsd:decimal ;
        rdfs:comment "The weight of an xDocLoadingUnit (cross-dock loading unit)." .


#################################################################
#    Classes
#################################################################

###  http://www.opengis.net/ont/geosparql#Feature
<http://www.opengis.net/ont/geosparql#Feature> rdf:type owl:Class ;
                                               rdfs:subClassOf <http://www.opengis.net/ont/geosparql#SpatialObject> ;
                                               owl:disjointWith <http://www.opengis.net/ont/geosparql#Geometry> ;
                                               <http://purl.org/dc/elements/1.1/contributor> "Matthew Perry" ;
                                               <http://purl.org/dc/elements/1.1/creator> "OGC GeoSPARQL 1.0 Standard Working Group" ;
                                               <http://purl.org/dc/elements/1.1/date> "2011-06-16"^^xsd:date ;
                                               <http://purl.org/dc/elements/1.1/description> """
      This class represents the top-level feature type. This class is 
      equivalent to GFI_Feature defined in ISO 19156:2011, and it is 
      superclass of all feature types.
    """@en ;
                                               rdfs:comment """
      This class represents the top-level feature type. This class is 
      equivalent to GFI_Feature defined in ISO 19156:2011, and it is 
      superclass of all feature types.
    """@en ;
                                               rdfs:isDefinedBy <http://www.opengis.net/ont/geosparql> ,
                                                                <http://www.opengis.net/spec/geosparql/1.0> ;
                                               rdfs:label "Feature"@en ;
                                               <http://www.w3.org/2004/02/skos/core#definition> """
      This class represents the top-level feature type. This class is 
      equivalent to GFI_Feature defined in ISO 19156:2011, and it is 
      superclass of all feature types.
    """@en ;
                                               <http://www.w3.org/2004/02/skos/core#prefLabel> "Feature"@en .


###  http://www.opengis.net/ont/geosparql#Geometry
<http://www.opengis.net/ont/geosparql#Geometry> rdf:type owl:Class ;
                                                rdfs:subClassOf <http://www.opengis.net/ont/geosparql#SpatialObject> ;
                                                <http://purl.org/dc/elements/1.1/contributor> "Matthew Perry" ;
                                                <http://purl.org/dc/elements/1.1/creator> "OGC GeoSPARQL 1.0 Standard Working Group" ;
                                                <http://purl.org/dc/elements/1.1/date> "2011-06-16"^^xsd:date ;
                                                <http://purl.org/dc/elements/1.1/description> """
      The class represents the top-level geometry type. This class is 
      equivalent to the UML class GM_Object defined in ISO 19107, and 
      it is superclass of all geometry types.
    """@en ;
                                                rdfs:comment """
      The class represents the top-level geometry type. This class is 
      equivalent to the UML class GM_Object defined in ISO 19107, and 
      it is superclass of all geometry types.
    """@en ;
                                                rdfs:isDefinedBy <http://www.opengis.net/ont/geosparql> ,
                                                                 <http://www.opengis.net/spec/geosparql/1.0> ;
                                                rdfs:label "Geometry"@en ;
                                                <http://www.w3.org/2004/02/skos/core#definition> """
      The class represents the top-level geometry type. This class is 
      equivalent to the UML class GM_Object defined in ISO 19107, and 
      it is superclass of all geometry types.
    """@en ;
                                                <http://www.w3.org/2004/02/skos/core#prefLabel> "Geometry"@en .


###  http://www.opengis.net/ont/geosparql#SpatialObject
<http://www.opengis.net/ont/geosparql#SpatialObject> rdf:type owl:Class ;
                                                     <http://purl.org/dc/elements/1.1/contributor> "Matthew Perry" ;
                                                     <http://purl.org/dc/elements/1.1/creator> "OGC GeoSPARQL 1.0 Standard Working Group" ;
                                                     <http://purl.org/dc/elements/1.1/date> "2011-06-16"^^xsd:date ;
                                                     <http://purl.org/dc/elements/1.1/description> """
      The class spatial-object represents everything that can have 
      a spatial representation. It is superclass of feature and geometry.
    """@en ;
                                                     rdfs:comment """
      The class spatial-object represents everything that can have 
      a spatial representation. It is superclass of feature and geometry.
    """@en ;
                                                     rdfs:isDefinedBy <http://www.opengis.net/ont/geosparql> ,
                                                                      <http://www.opengis.net/spec/geosparql/1.0> ;
                                                     rdfs:label "SpatialObject"@en ;
                                                     <http://www.w3.org/2004/02/skos/core#definition> """
      The class spatial-object represents everything that can have 
      a spatial representation. It is superclass of feature and geometry.
    """@en ;
                                                     <http://www.w3.org/2004/02/skos/core#prefLabel> "SpatialObject"@en .


###  https://w3id.org/latuli/ontology/m3#Carrier
:Carrier rdf:type owl:Class ;
         rdfs:subClassOf :Party ;
         rdfs:comment "A company, which physically transports goods from one place to another." .


###  https://w3id.org/latuli/ontology/m3#Consignee
:Consignee rdf:type owl:Class ;
           rdfs:subClassOf :Party ;
           rdfs:comment "In a consignment view / scenario, the entity who will receive the physical shipment." .


###  https://w3id.org/latuli/ontology/m3#Consignment
:Consignment rdf:type owl:Class ;
             rdfs:subClassOf [ rdf:type owl:Restriction ;
                               owl:onProperty :hasCarrierParty ;
                               owl:someValuesFrom :Carrier
                             ] ,
                             [ rdf:type owl:Restriction ;
                               owl:onProperty :hasConsigneeParty ;
                               owl:someValuesFrom :Consignee
                             ] ,
                             [ rdf:type owl:Restriction ;
                               owl:onProperty :hasConsignorParty ;
                               owl:someValuesFrom :Consignor
                             ] ,
                             [ rdf:type owl:Restriction ;
                               owl:onProperty :hasHubParty ;
                               owl:someValuesFrom :Party
                             ] ,
                             [ rdf:type owl:Restriction ;
                               owl:onProperty :includesTransport ;
                               owl:someValuesFrom :Transport
                             ] ,
                             [ rdf:type owl:Restriction ;
                               owl:onProperty :processedByWave ;
                               owl:someValuesFrom :Wave
                             ] ;
             rdfs:comment "A consignment is a logical grouping of goods (one or more physical entities) that is intended to be transported as a whole from a consignor to a consignee by a carrier or freight forwarder via one or more modes of transport, subject to one single transport contract." .


###  https://w3id.org/latuli/ontology/m3#Consignor
:Consignor rdf:type owl:Class ;
           rdfs:subClassOf :Party ;
           rdfs:comment "In a consignment view / scenario, the entity who will ship the physical shipment." .


###  https://w3id.org/latuli/ontology/m3#DangerousGoods
:DangerousGoods rdf:type owl:Class ;
                rdfs:subClassOf [ rdf:type owl:Restriction ;
                                  owl:onProperty :belongsToShipment ;
                                  owl:someValuesFrom :Shipment
                                ] ,
                                [ rdf:type owl:Restriction ;
                                  owl:onProperty :hasLoadingUnit ;
                                  owl:someValuesFrom :LoadingUnit
                                ] ,
                                [ rdf:type owl:Restriction ;
                                  owl:onProperty :relatesToTradeItem ;
                                  owl:someValuesFrom :TradeItem
                                ] .


###  https://w3id.org/latuli/ontology/m3#HubReconstructionLocation
:HubReconstructionLocation rdf:type owl:Class ;
                           owl:equivalentClass :Terminal ;
                           rdfs:subClassOf [ rdf:type owl:Restriction ;
                                             owl:onProperty :hasParty ;
                                             owl:someValuesFrom :Party
                                           ] ;
                           rdfs:comment "The location where a reconstruction of goods takes place." .


###  https://w3id.org/latuli/ontology/m3#LoadingUnit
:LoadingUnit rdf:type owl:Class ;
             rdfs:comment "A logistic unit is a unit of any composition made up for transport and or storage which has to be managed throughout the supply chain." .


###  https://w3id.org/latuli/ontology/m3#Party
:Party rdf:type owl:Class ;
       rdfs:comment "A person or group of people constituting a particular side in a contract or legal action." .


###  https://w3id.org/latuli/ontology/m3#Receiver
:Receiver rdf:type owl:Class ;
          rdfs:subClassOf :Party ;
          rdfs:comment "In a shipment scenario, a party who engages in receiving goods." .


###  https://w3id.org/latuli/ontology/m3#Shipment
:Shipment rdf:type owl:Class ;
          rdfs:subClassOf [ rdf:type owl:Restriction ;
                            owl:onProperty :hasReceiverParty ;
                            owl:someValuesFrom :Receiver
                          ] ,
                          [ rdf:type owl:Restriction ;
                            owl:onProperty :hasShipperParty ;
                            owl:someValuesFrom :Shipper
                          ] ;
          rdfs:comment "A shipment is an identifiable collection of one or more Trade Items available to be transported together from the shipper (Original Consignor/Shipper), to the receiver (Final/Ultimate Consignee). Typically the shipment is the entity communicated between trading partners in the Despatch and Receiving Advice." .


###  https://w3id.org/latuli/ontology/m3#ShipmentItem
:ShipmentItem rdf:type owl:Class ;
              rdfs:subClassOf [ rdf:type owl:Restriction ;
                                owl:onProperty :belongsToShipment ;
                                owl:someValuesFrom :Shipment
                              ] ,
                              [ rdf:type owl:Restriction ;
                                owl:onProperty :hasLoadingUnit ;
                                owl:someValuesFrom :LoadingUnit
                              ] ;
              rdfs:comment "A shipment is an identifiable collection of one or more Trade Items available to be transported together from the shipper (Original Consignor/Shipper), to the receiver (Final/Ultimate Consignee). Typically the shipment is the entity communicated between trading partners in the Despatch and Receiving Advice." .


###  https://w3id.org/latuli/ontology/m3#Shipper
:Shipper rdf:type owl:Class ;
         rdfs:subClassOf :Party ;
         rdfs:comment "In a shipment scenario, a party who engages in shipping goods." .


###  https://w3id.org/latuli/ontology/m3#Terminal
:Terminal rdf:type owl:Class .


###  https://w3id.org/latuli/ontology/m3#TerminalOperator
:TerminalOperator rdf:type owl:Class ;
                  rdfs:subClassOf :Party ;
                  rdfs:comment "Terminal operator means a person who by ownership or contractual agreement is charged with the responsibility for, or physical control over, and operation of a logistics terminal." .


###  https://w3id.org/latuli/ontology/m3#TradeItem
:TradeItem rdf:type owl:Class ;
           rdfs:subClassOf [ rdf:type owl:Restriction ;
                             owl:onProperty :belongsToShipment ;
                             owl:someValuesFrom :Shipment
                           ] ,
                           [ rdf:type owl:Restriction ;
                             owl:onProperty :hasLoadingUnit ;
                             owl:someValuesFrom :LoadingUnit
                           ] ;
           rdfs:comment "A trade item is any item (product or service) upon which there is a need to retrieve pre-defined information and that may be priced, or ordered, or invoiced at any point in any supply chain." .


###  https://w3id.org/latuli/ontology/m3#Transport
:Transport rdf:type owl:Class ;
           rdfs:comment "Transport is the act of moving goods and materials from one location to another" .


###  https://w3id.org/latuli/ontology/m3#Wave
:Wave rdf:type owl:Class ;
      rdfs:subClassOf [ rdf:type owl:Restriction ;
                        owl:onProperty :hasHubParty ;
                        owl:someValuesFrom :Party
                      ] ;
      rdfs:comment "A wave is a planning event that involves allocating a specific inventory or storage zone, and employees to pick items from those sections." .


###  https://w3id.org/latuli/ontology/m3#XDocLoadingUnit
:XDocLoadingUnit rdf:type owl:Class ;
                 rdfs:subClassOf [ rdf:type owl:Restriction ;
                                   owl:onProperty :hasCarrierParty ;
                                   owl:someValuesFrom :Carrier
                                 ] ,
                                 [ rdf:type owl:Restriction ;
                                   owl:onProperty :hasConsigneeParty ;
                                   owl:someValuesFrom :Consignee
                                 ] ,
                                 [ rdf:type owl:Restriction ;
                                   owl:onProperty :hasConsignorParty ;
                                   owl:someValuesFrom :Consignor
                                 ] ,
                                 [ rdf:type owl:Restriction ;
                                   owl:onProperty :hasHubReconstructionParty ;
                                   owl:someValuesFrom :Party
                                 ] ,
                                 [ rdf:type owl:Restriction ;
                                   owl:onProperty :hasInboundConsignment ;
                                   owl:someValuesFrom :Consignment
                                 ] ,
                                 [ rdf:type owl:Restriction ;
                                   owl:onProperty :hasInboundParentLoadingUnit ;
                                   owl:someValuesFrom :LoadingUnit
                                 ] ,
                                 [ rdf:type owl:Restriction ;
                                   owl:onProperty :hasLoadingUnit ;
                                   owl:someValuesFrom :LoadingUnit
                                 ] ,
                                 [ rdf:type owl:Restriction ;
                                   owl:onProperty :hasOutboundConsignment ;
                                   owl:someValuesFrom :Consignment
                                 ] ,
                                 [ rdf:type owl:Restriction ;
                                   owl:onProperty :hasOutboundParentLoadingUnit ;
                                   owl:someValuesFrom :LoadingUnit
                                 ] ,
                                 [ rdf:type owl:Restriction ;
                                   owl:onProperty :hasParty ;
                                   owl:someValuesFrom :Party
                                 ] ,
                                 [ rdf:type owl:Restriction ;
                                   owl:onProperty :hasReceiverParty ;
                                   owl:someValuesFrom :Receiver
                                 ] ,
                                 [ rdf:type owl:Restriction ;
                                   owl:onProperty :hasShipperParty ;
                                   owl:someValuesFrom :Shipper
                                 ] ,
                                 [ rdf:type owl:Restriction ;
                                   owl:onProperty :processedByWave ;
                                   owl:someValuesFrom :Wave
                                 ] ;
                 rdfs:comment "A loading unit which is received through an inbound dock and then transferred across the dock to an outbound transportation dock." .


###  Generated by the OWL API (version 5.1.14) https://github.com/owlcs/owlapi/
